Revert "move to `Std.Extensional`"
This reverts commit 58e9af35329a3c88e7257016a38f5da95eeccaf7.

src/Std/Data/ExtDHashMap/Basic.lean
@@ -9,10 +9,10 @@ import Std.Data.DHashMap.Lemmas
 /-!
 # Extensional dependent hash maps
 
-This file develops the type `Std.Extensional.DHashMap` of extensional dependent hash maps.
+This file develops the type `Std.ExtDHashMap` of extensional dependent hash maps.
 
-Lemmas about the operations on `Std.Extensional.DHashMap` are available in the
-module `Std.Data.DHashMap.ExtensionalLemmas`.
+Lemmas about the operations on `Std.ExtDHashMap` are available in the
+module `Std.Data.ExtDHashMap.Lemmas`.
 -/
 
 set_option linter.missingDocs true
@@ -26,7 +26,7 @@ variable {_ : BEq α} {_ : Hashable α} {_ : EquivBEq α} {_ : LawfulHashable α
 
 open scoped Std.DHashMap
 
-namespace Std.Extensional
+namespace Std
 
 /--
 Extensional dependent hash maps.
@@ -45,50 +45,50 @@ must be an equivalence relation and `a == b` must imply `hash a = hash b` (see a
 `EquivBEq` and `LawfulHashable` typeclasses). Both of these conditions are automatic if the BEq
 instance is lawful, i.e., if `a == b` implies `a = b`.
 
-In contrast to regular dependent hash maps, `Std.Extensional.DHashMap` offers several
-extensionality lemmas and therefore has more lemmas about equality of hash maps. This however
-also makes it lose the ability to iterate freely over the hash map.
+In contrast to regular dependent hash maps, `Std.ExtDHashMap` offers several extensionality lemmas
+and therefore has more lemmas about equality of hash maps. This however also makes it lose the
+ability to iterate freely over the hash map.
 
 These hash maps contain a bundled well-formedness invariant, which means that they cannot
 be used in nested inductive types. For these use cases, `Std.DHashMap.Raw` and
 `Std.DHashMap.Raw.WF` unbundle the invariant from the hash map. When in doubt, prefer
 `DHashMap` over `DHashMap.Raw`.
 -/
-def DHashMap (α : Type u) (β : α → Type v) [BEq α] [Hashable α] [EquivBEq α] [LawfulHashable α] :=
+def ExtDHashMap (α : Type u) (β : α → Type v) [BEq α] [Hashable α] [EquivBEq α] [LawfulHashable α] :=
   Quotient (DHashMap.isSetoid α β)
 
-namespace DHashMap
+namespace ExtDHashMap
 
-@[inline, inherit_doc Std.DHashMap.emptyWithCapacity]
+@[inline, inherit_doc DHashMap.emptyWithCapacity]
 def emptyWithCapacity [BEq α] [Hashable α] [EquivBEq α] [LawfulHashable α]
-    (capacity := 8) : DHashMap α β :=
-  Quotient.mk' (Std.DHashMap.emptyWithCapacity capacity)
+    (capacity := 8) : ExtDHashMap α β :=
+  Quotient.mk' (DHashMap.emptyWithCapacity capacity)
 
-instance [BEq α] [Hashable α] [EquivBEq α] [LawfulHashable α] : EmptyCollection (DHashMap α β) where
+instance [BEq α] [Hashable α] [EquivBEq α] [LawfulHashable α] : EmptyCollection (ExtDHashMap α β) where
   emptyCollection := emptyWithCapacity
 
 instance [BEq α] [Hashable α] [EquivBEq α] [LawfulHashable α] : Inhabited (DHashMap α β) where
   default := ∅
 
-@[inline, inherit_doc Std.DHashMap.insert] def insert (m : DHashMap α β) (a : α)
-    (b : β a) : DHashMap α β :=
+@[inline, inherit_doc DHashMap.insert] def insert (m : ExtDHashMap α β) (a : α)
+    (b : β a) : ExtDHashMap α β :=
   m.lift (fun m => Quotient.mk' (m.insert a b))
     (fun m m' (h : m ~m m') => Quotient.sound (h.insert a b))
 
-instance : Singleton ((a : α) × β a) (DHashMap α β) := ⟨fun ⟨a, b⟩ => (∅ : DHashMap α β).insert a b⟩
+instance : Singleton ((a : α) × β a) (ExtDHashMap α β) := ⟨fun ⟨a, b⟩ => (∅ : ExtDHashMap α β).insert a b⟩
 
-instance : Insert ((a : α) × β a) (DHashMap α β) := ⟨fun ⟨a, b⟩ s => s.insert a b⟩
+instance : Insert ((a : α) × β a) (ExtDHashMap α β) := ⟨fun ⟨a, b⟩ s => s.insert a b⟩
 
-instance : LawfulSingleton ((a : α) × β a) (DHashMap α β) :=
+instance : LawfulSingleton ((a : α) × β a) (ExtDHashMap α β) :=
   ⟨fun _ => rfl⟩
 
-@[inline, inherit_doc Std.DHashMap.insertIfNew] def insertIfNew (m : DHashMap α β)
-    (a : α) (b : β a) : DHashMap α β :=
+@[inline, inherit_doc DHashMap.insertIfNew] def insertIfNew (m : ExtDHashMap α β)
+    (a : α) (b : β a) : ExtDHashMap α β :=
   m.lift (fun m => Quotient.mk' (m.insertIfNew a b))
     (fun m m' (h : m ~m m') => Quotient.sound (h.insertIfNew a b))
 
-@[inline, inherit_doc Std.DHashMap.containsThenInsert] def containsThenInsert
-    (m : DHashMap α β) (a : α) (b : β a) : Bool × DHashMap α β :=
+@[inline, inherit_doc DHashMap.containsThenInsert] def containsThenInsert
+    (m : ExtDHashMap α β) (a : α) (b : β a) : Bool × ExtDHashMap α β :=
   m.lift (fun m => let m' := m.containsThenInsert a b; ⟨m'.1, Quotient.mk' m'.2⟩)
     (fun m m' (h : m ~m m') =>
       Prod.ext
@@ -96,8 +96,8 @@ instance : LawfulSingleton ((a : α) × β a) (DHashMap α β) :=
         (Quotient.sound <|
           m.containsThenInsert_snd.symm ▸ m'.containsThenInsert_snd.symm ▸ h.insert a b))
 
-@[inline, inherit_doc Std.DHashMap.containsThenInsertIfNew] def containsThenInsertIfNew
-    (m : DHashMap α β) (a : α) (b : β a) : Bool × DHashMap α β :=
+@[inline, inherit_doc DHashMap.containsThenInsert] def containsThenInsertIfNew
+    (m : ExtDHashMap α β) (a : α) (b : β a) : Bool × ExtDHashMap α β :=
   m.lift (fun m => let m' := m.containsThenInsertIfNew a b; ⟨m'.1, Quotient.mk' m'.2⟩)
     (fun m m' (h : m ~m m') =>
       Prod.ext
@@ -105,8 +105,8 @@ instance : LawfulSingleton ((a : α) × β a) (DHashMap α β) :=
         (Quotient.sound <|
           m.containsThenInsertIfNew_snd.symm ▸ m'.containsThenInsertIfNew_snd.symm ▸ h.insertIfNew a b))
 
-@[inline, inherit_doc Std.DHashMap.getThenInsertIfNew?] def getThenInsertIfNew? [LawfulBEq α]
-    (m : DHashMap α β) (a : α) (b : β a) : Option (β a) × DHashMap α β :=
+@[inline, inherit_doc DHashMap.getThenInsertIfNew?] def getThenInsertIfNew? [LawfulBEq α]
+    (m : ExtDHashMap α β) (a : α) (b : β a) : Option (β a) × ExtDHashMap α β :=
   m.lift (fun m => let m' := m.getThenInsertIfNew? a b; ⟨m'.1, Quotient.mk' m'.2⟩)
     (fun m m' (h : m ~m m') =>
       Prod.ext
@@ -114,35 +114,35 @@ instance : LawfulSingleton ((a : α) × β a) (DHashMap α β) :=
         (Quotient.sound <|
           m.getThenInsertIfNew?_snd.symm ▸ m'.getThenInsertIfNew?_snd.symm ▸ h.insertIfNew a b))
 
-@[inline, inherit_doc Std.DHashMap.get?] def get? [LawfulBEq α] (m : DHashMap α β)
+@[inline, inherit_doc DHashMap.get?] def get? [LawfulBEq α] (m : ExtDHashMap α β)
     (a : α) : Option (β a) :=
   m.lift (fun m => m.get? a) (fun m m' (h : m ~m m') => h.get?_eq)
 
-@[inline, inherit_doc Std.DHashMap.contains] def contains (m : DHashMap α β) (a : α) :
+@[inline, inherit_doc DHashMap.contains] def contains (m : ExtDHashMap α β) (a : α) :
     Bool :=
   m.lift (fun m => m.contains a) (fun m m' (h : m ~m m') => h.contains_eq)
 
-instance : Membership α (DHashMap α β) where
+instance : Membership α (ExtDHashMap α β) where
   mem m a := m.contains a
 
-instance {m : DHashMap α β} {a : α} : Decidable (a ∈ m) :=
+instance {m : ExtDHashMap α β} {a : α} : Decidable (a ∈ m) :=
   inferInstanceAs <| Decidable (m.contains a)
 
-@[inline, inherit_doc Std.DHashMap.get] def get [LawfulBEq α] (m : DHashMap α β) (a : α)
+@[inline, inherit_doc DHashMap.get] def get [LawfulBEq α] (m : ExtDHashMap α β) (a : α)
     (h : a ∈ m) : β a :=
   m.pliftOn (fun m h' => m.get a (h' ▸ h :))
     (fun m m' _ _ (h : m ~m m') => h.get_eq _)
 
-@[inline, inherit_doc Std.DHashMap.get!] def get! [LawfulBEq α] (m : DHashMap α β)
+@[inline, inherit_doc DHashMap.get!] def get! [LawfulBEq α] (m : ExtDHashMap α β)
     (a : α) [Inhabited (β a)] : β a :=
   m.lift (fun m => m.get! a) (fun m m' (h : m ~m m') => h.get!_eq)
 
-@[inline, inherit_doc Std.DHashMap.getD] def getD [LawfulBEq α] (m : DHashMap α β)
+@[inline, inherit_doc DHashMap.getD] def getD [LawfulBEq α] (m : ExtDHashMap α β)
     (a : α) (fallback : β a) : β a :=
   m.lift (fun m => m.getD a fallback) (fun m m' (h : m ~m m') => h.getD_eq)
 
-@[inline, inherit_doc Std.DHashMap.erase] def erase (m : DHashMap α β) (a : α) :
-    DHashMap α β :=
+@[inline, inherit_doc DHashMap.erase] def erase (m : ExtDHashMap α β) (a : α) :
+    ExtDHashMap α β :=
   m.lift (fun m => Quotient.mk' (m.erase a))
     (fun m m' (h : m ~m m') => Quotient.sound (h.erase a))
 
@@ -150,97 +150,97 @@ namespace Const
 
 variable {β : Type v}
 
-@[inline, inherit_doc Std.DHashMap.Const.get?] def get?
-    (m : DHashMap α (fun _ => β)) (a : α) : Option β :=
-  m.lift (fun m => Std.DHashMap.Const.get? m a)
+@[inline, inherit_doc DHashMap.Const.get?] def get?
+    (m : ExtDHashMap α (fun _ => β)) (a : α) : Option β :=
+  m.lift (fun m => DHashMap.Const.get? m a)
     (fun m m' (h : m ~m m') => h.constGet?_eq)
 
-@[inline, inherit_doc Std.DHashMap.Const.get] def get
-    (m : DHashMap α (fun _ => β)) (a : α) (h : a ∈ m) : β :=
-  m.pliftOn (fun m h' => Std.DHashMap.Const.get m a (h' ▸ h :))
+@[inline, inherit_doc DHashMap.Const.get] def get
+    (m : ExtDHashMap α (fun _ => β)) (a : α) (h : a ∈ m) : β :=
+  m.pliftOn (fun m h' => DHashMap.Const.get m a (h' ▸ h :))
     (fun m m' _ _ (h : m ~m m') => h.constGet_eq _)
 
-@[inline, inherit_doc Std.DHashMap.Const.getD] def getD
-    (m : DHashMap α (fun _ => β)) (a : α) (fallback : β) : β :=
-  m.lift (fun m => Std.DHashMap.Const.getD m a fallback)
+@[inline, inherit_doc DHashMap.Const.getD] def getD
+    (m : ExtDHashMap α (fun _ => β)) (a : α) (fallback : β) : β :=
+  m.lift (fun m => DHashMap.Const.getD m a fallback)
     (fun m m' (h : m ~m m') => h.constGetD_eq)
 
-@[inline, inherit_doc Std.DHashMap.Const.get!] def get! [Inhabited β]
-    (m : DHashMap α (fun _ => β)) (a : α) : β :=
-  m.lift (fun m => Std.DHashMap.Const.get! m a)
+@[inline, inherit_doc DHashMap.Const.get!] def get! [Inhabited β]
+    (m : ExtDHashMap α (fun _ => β)) (a : α) : β :=
+  m.lift (fun m => DHashMap.Const.get! m a)
     (fun m m' (h : m ~m m') => h.constGet!_eq)
 
-@[inline, inherit_doc Std.DHashMap.Const.getThenInsertIfNew?] def getThenInsertIfNew?
-    (m : DHashMap α (fun _ => β)) (a : α) (b : β) :
-    Option β × DHashMap α (fun _ => β) :=
+@[inline, inherit_doc DHashMap.Const.getThenInsertIfNew?] def getThenInsertIfNew?
+    (m : ExtDHashMap α (fun _ => β)) (a : α) (b : β) :
+    Option β × ExtDHashMap α (fun _ => β) :=
   m.lift (fun m =>
-      let m' := Std.DHashMap.Const.getThenInsertIfNew? m a b
+      let m' := DHashMap.Const.getThenInsertIfNew? m a b
       ⟨m'.1, Quotient.mk' m'.2⟩)
     (fun m m' (h : m ~m m') =>
       Prod.ext
-        (Std.DHashMap.Const.getThenInsertIfNew?_fst.symm ▸
-          Std.DHashMap.Const.getThenInsertIfNew?_fst.symm ▸ h.constGet?_eq)
+        (DHashMap.Const.getThenInsertIfNew?_fst.symm ▸
+          DHashMap.Const.getThenInsertIfNew?_fst.symm ▸ h.constGet?_eq)
         (Quotient.sound <|
-          Std.DHashMap.Const.getThenInsertIfNew?_snd.symm ▸
-          Std.DHashMap.Const.getThenInsertIfNew?_snd.symm ▸ h.insertIfNew a b))
+          DHashMap.Const.getThenInsertIfNew?_snd.symm ▸
+          DHashMap.Const.getThenInsertIfNew?_snd.symm ▸ h.insertIfNew a b))
 
 end Const
 
-@[inline, inherit_doc Std.DHashMap.getKey?] def getKey? (m : DHashMap α β) (a : α) : Option α :=
+@[inline, inherit_doc DHashMap.getKey?] def getKey? (m : ExtDHashMap α β) (a : α) : Option α :=
   m.lift (fun m => m.getKey? a) (fun m m' (h : m ~m m') => h.getKey?_eq)
 
-@[inline, inherit_doc Std.DHashMap.getKey] def getKey (m : DHashMap α β) (a : α) (h : a ∈ m) : α :=
+@[inline, inherit_doc DHashMap.getKey] def getKey (m : ExtDHashMap α β) (a : α) (h : a ∈ m) : α :=
   m.pliftOn (fun m h' => m.getKey a (h' ▸ h :))
     (fun m m' _ _ (h : m ~m m') => h.getKey_eq _)
 
-@[inline, inherit_doc Std.DHashMap.getKey!] def getKey! [Inhabited α] (m : DHashMap α β) (a : α) : α :=
+@[inline, inherit_doc DHashMap.getKey!] def getKey! [Inhabited α] (m : ExtDHashMap α β) (a : α) : α :=
   m.lift (fun m => m.getKey! a) (fun m m' (h : m ~m m') => h.getKey!_eq)
 
-@[inline, inherit_doc Std.DHashMap.getKeyD] def getKeyD (m : DHashMap α β) (a : α) (fallback : α) : α :=
+@[inline, inherit_doc DHashMap.getKeyD] def getKeyD (m : ExtDHashMap α β) (a : α) (fallback : α) : α :=
   m.lift (fun m => m.getKeyD a fallback)
     (fun m m' (h : m ~m m') => h.getKeyD_eq)
 
-@[inline, inherit_doc Std.DHashMap.size] def size (m : DHashMap α β) : Nat :=
+@[inline, inherit_doc DHashMap.size] def size (m : ExtDHashMap α β) : Nat :=
   m.lift (fun m => m.size) (fun m m' (h : m ~m m') => h.size_eq)
 
-@[inline, inherit_doc Std.DHashMap.isEmpty] def isEmpty (m : DHashMap α β) : Bool :=
+@[inline, inherit_doc DHashMap.isEmpty] def isEmpty (m : ExtDHashMap α β) : Bool :=
   m.lift (fun m => m.isEmpty) (fun m m' (h : m ~m m') => h.isEmpty_eq)
 
 -- TODO: add fold similar to `Finset.fold`
 
-@[inline, inherit_doc Std.DHashMap.filter] def filter (f : (a : α) → β a → Bool)
-    (m : DHashMap α β) : DHashMap α β :=
+@[inline, inherit_doc DHashMap.filter] def filter (f : (a : α) → β a → Bool)
+    (m : ExtDHashMap α β) : ExtDHashMap α β :=
   m.lift (fun m => Quotient.mk' (m.filter f))
     (fun m m' (h : m ~m m') => Quotient.sound (h.filter f))
 
-@[inline, inherit_doc Std.DHashMap.map] def map (f : (a : α) → β a → γ a)
-    (m : DHashMap α β) : DHashMap α γ :=
+@[inline, inherit_doc DHashMap.map] def map (f : (a : α) → β a → γ a)
+    (m : ExtDHashMap α β) : ExtDHashMap α γ :=
   m.lift (fun m => Quotient.mk' (m.map f))
     (fun m m' (h : m ~m m') => Quotient.sound (h.map f))
 
-@[inline, inherit_doc Std.DHashMap.filterMap] def filterMap (f : (a : α) → β a → Option (γ a))
-    (m : DHashMap α β) : DHashMap α γ :=
+@[inline, inherit_doc DHashMap.filterMap] def filterMap (f : (a : α) → β a → Option (γ a))
+    (m : ExtDHashMap α β) : ExtDHashMap α γ :=
   m.lift (fun m => Quotient.mk' (m.filterMap f))
     (fun m m' (h : m ~m m') => Quotient.sound (h.filterMap f))
 
-@[inline, inherit_doc Std.DHashMap.modify] def modify [LawfulBEq α] (m : DHashMap α β)
-    (a : α) (f : β a → β a) : DHashMap α β :=
+@[inline, inherit_doc DHashMap.modify] def modify [LawfulBEq α] (m : ExtDHashMap α β)
+    (a : α) (f : β a → β a) : ExtDHashMap α β :=
   m.lift (fun m => Quotient.mk' (m.modify a f))
     (fun m m' (h : m ~m m') => Quotient.sound (h.modify a f))
 
-@[inline, inherit_doc Std.DHashMap.Const.modify] def Const.modify {β : Type v} (m : DHashMap α (fun _ => β))
-    (a : α) (f : β → β) : DHashMap α (fun _ => β) :=
-  m.lift (fun m => Quotient.mk' (Std.DHashMap.Const.modify m a f))
+@[inline, inherit_doc DHashMap.modify] def Const.modify {β : Type v} (m : ExtDHashMap α (fun _ => β))
+    (a : α) (f : β → β) : ExtDHashMap α (fun _ => β) :=
+  m.lift (fun m => Quotient.mk' (DHashMap.Const.modify m a f))
     (fun m m' (h : m ~m m') => Quotient.sound (h.constModify a f))
 
-@[inline, inherit_doc Std.DHashMap.alter] def alter [LawfulBEq α] (m : DHashMap α β)
-    (a : α) (f : Option (β a) → Option (β a)) : DHashMap α β :=
+@[inline, inherit_doc DHashMap.alter] def alter [LawfulBEq α] (m : ExtDHashMap α β)
+    (a : α) (f : Option (β a) → Option (β a)) : ExtDHashMap α β :=
   m.lift (fun m => Quotient.mk' (m.alter a f))
     (fun m m' (h : m ~m m') => Quotient.sound (h.alter a f))
 
-@[inline, inherit_doc Std.DHashMap.Const.alter] def Const.alter {β : Type v} (m : DHashMap α (fun _ => β))
-    (a : α) (f : Option β → Option β) : DHashMap α (fun _ => β) :=
-  m.lift (fun m => Quotient.mk' (Std.DHashMap.Const.alter m a f))
+@[inline, inherit_doc DHashMap.alter] def Const.alter {β : Type v} (m : ExtDHashMap α (fun _ => β))
+    (a : α) (f : Option β → Option β) : ExtDHashMap α (fun _ => β) :=
+  m.lift (fun m => Quotient.mk' (DHashMap.Const.alter m a f))
     (fun m m' (h : m ~m m') => Quotient.sound (h.constAlter a f))
 
 /-
@@ -248,27 +248,27 @@ Note: We can't use the existing functions because weird (noncomputable) `ForIn` 
 can break congruence. The subtype is still used to provide the `insertMany_ind` theorem.
 -/
 
-@[inline, inherit_doc Std.DHashMap.insertMany] def insertMany {ρ : Type w}
-    [ForIn Id ρ ((a : α) × β a)] (m : DHashMap α β) (l : ρ) : DHashMap α β := Id.run do
-  let mut m : { x // ∀ P : DHashMap α β → Prop,
+@[inline, inherit_doc DHashMap.insertMany] def insertMany {ρ : Type w}
+    [ForIn Id ρ ((a : α) × β a)] (m : ExtDHashMap α β) (l : ρ) : ExtDHashMap α β := Id.run do
+  let mut m : { x // ∀ P : ExtDHashMap α β → Prop,
     P m → (∀ {m a b}, P m → P (m.insert a b)) → P x } := ⟨m, fun _ h _ => h⟩
   for ⟨a, b⟩ in l do
     m := ⟨m.1.insert a b, fun _ init step => step (m.2 _ init step)⟩
   return m.1
 
-@[inline, inherit_doc Std.DHashMap.Const.insertMany] def Const.insertMany {β : Type v} {ρ : Type w}
-    [ForIn Id ρ (α × β)] (m : DHashMap α (fun _ => β))
-    (l : ρ) : DHashMap α (fun _ => β) := Id.run do
-  let mut m : { x // ∀ P : DHashMap α (fun _ => β) → Prop,
+@[inline, inherit_doc DHashMap.Const.insertMany] def Const.insertMany {β : Type v} {ρ : Type w}
+    [ForIn Id ρ (α × β)] (m : ExtDHashMap α (fun _ => β))
+    (l : ρ) : ExtDHashMap α (fun _ => β) := Id.run do
+  let mut m : { x // ∀ P : ExtDHashMap α (fun _ => β) → Prop,
     P m → (∀ {m a b}, P m → P (m.insert a b)) → P x } := ⟨m, fun _ h _ => h⟩
   for (a, b) in l do
     m := ⟨m.1.insert a b, fun _ init step => step (m.2 _ init step)⟩
   return m.1
 
-@[inline, inherit_doc Std.DHashMap.Const.insertManyIfNewUnit] def Const.insertManyIfNewUnit {ρ : Type w}
-    [ForIn Id ρ α] (m : DHashMap α (fun _ => Unit))
-    (l : ρ) : DHashMap α (fun _ => Unit) := Id.run do
-  let mut m : { x // ∀ P : DHashMap α (fun _ => Unit) → Prop,
+@[inline, inherit_doc DHashMap.Const.insertManyIfNewUnit] def Const.insertManyIfNewUnit {ρ : Type w}
+    [ForIn Id ρ α] (m : ExtDHashMap α (fun _ => Unit))
+    (l : ρ) : ExtDHashMap α (fun _ => Unit) := Id.run do
+  let mut m : { x // ∀ P : ExtDHashMap α (fun _ => Unit) → Prop,
     P m → (∀ {m a}, P m → P (m.insertIfNew a ())) → P x } := ⟨m, fun _ h _ => h⟩
   for a in l do
     m := ⟨m.1.insertIfNew a (), fun _ init step => step (m.2 _ init step)⟩
@@ -280,21 +280,21 @@ can break congruence. The subtype is still used to provide the `insertMany_ind` 
 Note: we could use `ofList` here but we want the connection of `ofList` and `insertMany`.
 -/
 
-@[inline, inherit_doc Std.DHashMap.ofList] def ofList
+@[inline, inherit_doc DHashMap.ofList] def ofList
     [BEq α] [Hashable α] [EquivBEq α] [LawfulHashable α] (l : List ((a : α) × β a)) :
-    DHashMap α β :=
+    ExtDHashMap α β :=
   insertMany ∅ l
 
-@[inline, inherit_doc Std.DHashMap.Const.ofList] def Const.ofList {β : Type v}
+@[inline, inherit_doc DHashMap.Const.ofList] def Const.ofList {β : Type v}
     [BEq α] [Hashable α] [EquivBEq α] [LawfulHashable α] (l : List (α × β)) :
-    DHashMap α (fun _ => β) :=
+    ExtDHashMap α (fun _ => β) :=
   Const.insertMany ∅ l
 
-@[inline, inherit_doc Std.DHashMap.Const.unitOfList] def Const.unitOfList
+@[inline, inherit_doc DHashMap.Const.unitOfList] def Const.unitOfList
     [BEq α] [Hashable α] [EquivBEq α] [LawfulHashable α] (l : List α) :
-    DHashMap α (fun _ => Unit) :=
+    ExtDHashMap α (fun _ => Unit) :=
   Const.insertManyIfNewUnit ∅ l
 
-end DHashMap
+end ExtDHashMap
 
-end Std.Extensional
+end Std
