src/Std/Data/ExtDHashMap/Lemmas.lean
@@ -4,12 +4,12 @@ Released under Apache 2.0 license as described in the file LICENSE.
 Authors: Robin Arnez
 -/
 prelude
-import Std.Data.DHashMap.Extensional
+import Std.Data.ExtDHashMap.Basic
 
 /-!
 # Extensional dependent hash map lemmas
 
-This file contains lemmas about `Std.Extensional.DHashMap`.
+This file contains lemmas about `Std.ExtDHashMap`.
 -/
 
 set_option linter.missingDocs true
@@ -20,9 +20,9 @@ universe u v w w'
 variable {α : Type u} {_ : BEq α} {_ : Hashable α} {_ : EquivBEq α} {_ : LawfulHashable α}
 variable {β : α → Type v} {γ : α → Type w}
 
-namespace Std.Extensional.DHashMap
+namespace Std.ExtDHashMap
 
-variable {m : DHashMap α β}
+variable {m : ExtDHashMap α β}
 
 @[simp]
 theorem isEmpty_iff : m.isEmpty ↔ m = ∅ := by
@@ -38,83 +38,83 @@ theorem isEmpty_eq_false_iff : m.isEmpty = false ↔ ¬m = ∅ :=
 theorem empty_eq : ∅ = m ↔ m = ∅ := eq_comm
 
 @[simp]
-theorem emptyWithCapacity_eq {c} : (emptyWithCapacity c : DHashMap α β) = ∅ :=
-  isEmpty_iff.mp Std.DHashMap.isEmpty_emptyWithCapacity
+theorem emptyWithCapacity_eq {c} : (emptyWithCapacity c : ExtDHashMap α β) = ∅ :=
+  isEmpty_iff.mp DHashMap.isEmpty_emptyWithCapacity
 
 @[simp]
 theorem not_insert_eq_empty {k : α} {v : β k} :
     ¬m.insert k v = ∅ :=
-  m.inductionOn fun _ => isEmpty_eq_false_iff.mp Std.DHashMap.isEmpty_insert
+  m.inductionOn fun _ => isEmpty_eq_false_iff.mp DHashMap.isEmpty_insert
 
 theorem mem_iff_contains {a : α} : a ∈ m ↔ m.contains a :=
   Iff.rfl
 
 theorem contains_congr {a b : α} (hab : a == b) : m.contains a = m.contains b :=
-  m.inductionOn fun _ => Std.DHashMap.contains_congr hab
+  m.inductionOn fun _ => DHashMap.contains_congr hab
 
 theorem mem_congr {a b : α} (hab : a == b) : a ∈ m ↔ b ∈ m :=
-  m.inductionOn fun _ => Std.DHashMap.mem_congr hab
+  m.inductionOn fun _ => DHashMap.mem_congr hab
 
 @[simp]
-theorem contains_empty {a : α} : (∅ : Std.DHashMap α β).contains a = false :=
-  Std.DHashMap.contains_empty
+theorem contains_empty {a : α} : (∅ : DHashMap α β).contains a = false :=
+  DHashMap.contains_empty
 
 @[simp]
-theorem not_mem_empty {a : α} : ¬a ∈ (∅ : Std.DHashMap α β) :=
-  Std.DHashMap.not_mem_empty
+theorem not_mem_empty {a : α} : ¬a ∈ (∅ : DHashMap α β) :=
+  DHashMap.not_mem_empty
 
 theorem eq_empty_iff_forall_contains : m = ∅ ↔ ∀ a, m.contains a = false :=
-  isEmpty_iff.symm.trans <| m.inductionOn fun _ => Std.DHashMap.isEmpty_iff_forall_contains
+  isEmpty_iff.symm.trans <| m.inductionOn fun _ => DHashMap.isEmpty_iff_forall_contains
 
 theorem eq_empty_iff_forall_not_mem : m = ∅ ↔ ∀ a, ¬a ∈ m :=
-  isEmpty_iff.symm.trans <| m.inductionOn fun _ => Std.DHashMap.isEmpty_iff_forall_not_mem
+  isEmpty_iff.symm.trans <| m.inductionOn fun _ => DHashMap.isEmpty_iff_forall_not_mem
 
 @[simp] theorem insert_eq_insert {p : (a : α) × β a} : Insert.insert p m = m.insert p.1 p.2 := rfl
 
 @[simp] theorem singleton_eq_insert {p : (a : α) × β a} :
-    Singleton.singleton p = (∅ : Std.DHashMap α β).insert p.1 p.2 :=
+    Singleton.singleton p = (∅ : DHashMap α β).insert p.1 p.2 :=
   rfl
 
 @[simp]
 theorem contains_insert {k a : α} {v : β k} :
     (m.insert k v).contains a = (k == a || m.contains a) :=
-  m.inductionOn fun _ => Std.DHashMap.contains_insert
+  m.inductionOn fun _ => DHashMap.contains_insert
 
 @[simp]
 theorem mem_insert {k a : α} {v : β k} : a ∈ m.insert k v ↔ k == a ∨ a ∈ m :=
-  m.inductionOn fun _ => Std.DHashMap.mem_insert
+  m.inductionOn fun _ => DHashMap.mem_insert
 
 theorem contains_of_contains_insert {k a : α} {v : β k} :
     (m.insert k v).contains a → (k == a) = false → m.contains a :=
-  m.inductionOn fun _ => Std.DHashMap.contains_of_contains_insert
+  m.inductionOn fun _ => DHashMap.contains_of_contains_insert
 
 theorem mem_of_mem_insert {k a : α} {v : β k} : a ∈ m.insert k v → (k == a) = false → a ∈ m :=
-  m.inductionOn fun _ => Std.DHashMap.mem_of_mem_insert
+  m.inductionOn fun _ => DHashMap.mem_of_mem_insert
 
 theorem contains_insert_self {k : α} {v : β k} : (m.insert k v).contains k := by simp
 
 theorem mem_insert_self {k : α} {v : β k} : k ∈ m.insert k v := by simp
 
 @[simp]
-theorem size_empty : (∅ : DHashMap α β).size = 0 := rfl
+theorem size_empty : (∅ : ExtDHashMap α β).size = 0 := rfl
 
 theorem eq_empty_iff_size_eq_zero : m = ∅ ↔ m.size = 0 :=
   isEmpty_iff.symm.trans <| m.inductionOn fun _ =>
-    (Bool.eq_iff_iff.mp Std.DHashMap.isEmpty_eq_size_eq_zero).trans beq_iff_eq
+    (Bool.eq_iff_iff.mp DHashMap.isEmpty_eq_size_eq_zero).trans beq_iff_eq
 
 theorem size_insert {k : α} {v : β k} :
     (m.insert k v).size = if k ∈ m then m.size else m.size + 1 :=
-  m.inductionOn fun _ => Std.DHashMap.size_insert
+  m.inductionOn fun _ => DHashMap.size_insert
 
 theorem size_le_size_insert {k : α} {v : β k} : m.size ≤ (m.insert k v).size :=
-  m.inductionOn fun _ => Std.DHashMap.size_le_size_insert
+  m.inductionOn fun _ => DHashMap.size_le_size_insert
 
 theorem size_insert_le {k : α} {v : β k} : (m.insert k v).size ≤ m.size + 1 :=
-  m.inductionOn fun _ => Std.DHashMap.size_insert_le
+  m.inductionOn fun _ => DHashMap.size_insert_le
 
 @[simp]
-theorem erase_empty {k : α} : (∅ : DHashMap α β).erase k = ∅ :=
-  congrArg Quotient.mk' Std.DHashMap.erase_empty
+theorem erase_empty {k : α} : (∅ : ExtDHashMap α β).erase k = ∅ :=
+  congrArg Quotient.mk' DHashMap.erase_empty
 
 @[simp]
 theorem erase_eq_empty_iff {k : α} : m.erase k = ∅ ↔ m = ∅ ∨ m.size = 1 ∧ k ∈ m := by
@@ -122,13 +122,13 @@ theorem erase_eq_empty_iff {k : α} : m.erase k = ∅ ↔ m = ∅ ∨ m.size = 1
   rcases m with ⟨m⟩
   rw [← isEmpty_iff]
   dsimp only [erase, isEmpty, Quotient.mk', Quotient.mk, Quotient.lift]
-  simp only [Std.DHashMap.isEmpty_erase, Bool.or_eq_true, Bool.and_eq_true, beq_iff_eq]
+  simp only [DHashMap.isEmpty_erase, Bool.or_eq_true, Bool.and_eq_true, beq_iff_eq]
   rfl
 
 @[simp]
 theorem contains_erase {k a : α} :
     (m.erase k).contains a = (!(k == a) && m.contains a) :=
-  m.inductionOn fun _ => Std.DHashMap.contains_erase
+  m.inductionOn fun _ => DHashMap.contains_erase
 
 @[simp]
 theorem mem_erase {k a : α} :
@@ -137,117 +137,117 @@ theorem mem_erase {k a : α} :
 
 theorem contains_of_contains_erase {k a : α} :
     (m.erase k).contains a → m.contains a :=
-  m.inductionOn fun _ => Std.DHashMap.contains_of_contains_erase
+  m.inductionOn fun _ => DHashMap.contains_of_contains_erase
 
 theorem mem_of_mem_erase {k a : α} : a ∈ m.erase k → a ∈ m := by
   simp
 
 theorem size_erase {k : α} :
     (m.erase k).size = if k ∈ m then m.size - 1 else m.size :=
-  m.inductionOn fun _ => Std.DHashMap.size_erase
+  m.inductionOn fun _ => DHashMap.size_erase
 
 theorem size_erase_le {k : α} : (m.erase k).size ≤ m.size :=
-  m.inductionOn fun _ => Std.DHashMap.size_erase_le
+  m.inductionOn fun _ => DHashMap.size_erase_le
 
 theorem size_le_size_erase {k : α} :
     m.size ≤ (m.erase k).size + 1 :=
-  m.inductionOn fun _ => Std.DHashMap.size_le_size_erase
+  m.inductionOn fun _ => DHashMap.size_le_size_erase
 
 @[simp]
 theorem containsThenInsert_fst {k : α} {v : β k} : (m.containsThenInsert k v).1 = m.contains k :=
-  m.inductionOn fun _ => Std.DHashMap.containsThenInsert_fst
+  m.inductionOn fun _ => DHashMap.containsThenInsert_fst
 
 @[simp]
 theorem containsThenInsert_snd {k : α} {v : β k} : (m.containsThenInsert k v).2 = m.insert k v :=
-  m.inductionOn fun _ => congrArg Quotient.mk' Std.DHashMap.containsThenInsert_snd
+  m.inductionOn fun _ => congrArg Quotient.mk' DHashMap.containsThenInsert_snd
 
 @[simp]
 theorem containsThenInsertIfNew_fst {k : α} {v : β k} :
     (m.containsThenInsertIfNew k v).1 = m.contains k :=
-  m.inductionOn fun _ => Std.DHashMap.containsThenInsertIfNew_fst
+  m.inductionOn fun _ => DHashMap.containsThenInsertIfNew_fst
 
 @[simp]
 theorem containsThenInsertIfNew_snd {k : α} {v : β k} :
     (m.containsThenInsertIfNew k v).2 = m.insertIfNew k v :=
-  m.inductionOn fun _ => congrArg Quotient.mk' Std.DHashMap.containsThenInsertIfNew_snd
+  m.inductionOn fun _ => congrArg Quotient.mk' DHashMap.containsThenInsertIfNew_snd
 
 @[simp]
-theorem get?_empty [LawfulBEq α] {a : α} : (∅ : DHashMap α β).get? a = none :=
-  Std.DHashMap.get?_empty
+theorem get?_empty [LawfulBEq α] {a : α} : (∅ : ExtDHashMap α β).get? a = none :=
+  DHashMap.get?_empty
 
 theorem get?_insert [LawfulBEq α] {a k : α} {v : β k} : (m.insert k v).get? a =
     if h : k == a then some (cast (congrArg β (eq_of_beq h)) v) else m.get? a :=
-  m.inductionOn fun _ => Std.DHashMap.get?_insert
+  m.inductionOn fun _ => DHashMap.get?_insert
 
 @[simp]
 theorem get?_insert_self [LawfulBEq α] {k : α} {v : β k} : (m.insert k v).get? k = some v :=
-  m.inductionOn fun _ => Std.DHashMap.get?_insert_self
+  m.inductionOn fun _ => DHashMap.get?_insert_self
 
 theorem contains_eq_isSome_get? [LawfulBEq α] {a : α} : m.contains a = (m.get? a).isSome :=
-  m.inductionOn fun _ => Std.DHashMap.contains_eq_isSome_get?
+  m.inductionOn fun _ => DHashMap.contains_eq_isSome_get?
 
 theorem mem_iff_isSome_get? [LawfulBEq α] {a : α} : a ∈ m ↔ (m.get? a).isSome :=
-  m.inductionOn fun _ => Std.DHashMap.mem_iff_isSome_get?
+  m.inductionOn fun _ => DHashMap.mem_iff_isSome_get?
 
 theorem get?_eq_none_of_contains_eq_false [LawfulBEq α] {a : α} :
     m.contains a = false → m.get? a = none :=
-  m.inductionOn fun _ => Std.DHashMap.get?_eq_none_of_contains_eq_false
+  m.inductionOn fun _ => DHashMap.get?_eq_none_of_contains_eq_false
 
 theorem get?_eq_none [LawfulBEq α] {a : α} : ¬a ∈ m → m.get? a = none := by
   simpa [mem_iff_contains] using get?_eq_none_of_contains_eq_false
 
 theorem get?_erase [LawfulBEq α] {k a : α} :
     (m.erase k).get? a = if k == a then none else m.get? a :=
-  m.inductionOn fun _ => Std.DHashMap.get?_erase
+  m.inductionOn fun _ => DHashMap.get?_erase
 
 @[simp]
 theorem get?_erase_self [LawfulBEq α] {k : α} : (m.erase k).get? k = none :=
-  m.inductionOn fun _ => Std.DHashMap.get?_erase_self
+  m.inductionOn fun _ => DHashMap.get?_erase_self
 
 namespace Const
 
-variable {β : Type v} {m : DHashMap α (fun _ => β)}
+variable {β : Type v} {m : ExtDHashMap α (fun _ => β)}
 
 @[simp]
-theorem get?_empty {a : α} : get? (∅ : DHashMap α (fun _ => β)) a = none :=
-  Std.DHashMap.Const.get?_empty
+theorem get?_empty {a : α} : get? (∅ : ExtDHashMap α (fun _ => β)) a = none :=
+  DHashMap.Const.get?_empty
 
 theorem get?_insert {k a : α} {v : β} :
     get? (m.insert k v) a = if k == a then some v else get? m a :=
-  m.inductionOn fun _ => Std.DHashMap.Const.get?_insert
+  m.inductionOn fun _ => DHashMap.Const.get?_insert
 
 @[simp]
 theorem get?_insert_self {k : α} {v : β} :
     get? (m.insert k v) k = some v :=
-  m.inductionOn fun _ => Std.DHashMap.Const.get?_insert_self
+  m.inductionOn fun _ => DHashMap.Const.get?_insert_self
 
 theorem contains_eq_isSome_get? {a : α} :
     m.contains a = (get? m a).isSome :=
-  m.inductionOn fun _ => Std.DHashMap.Const.contains_eq_isSome_get?
+  m.inductionOn fun _ => DHashMap.Const.contains_eq_isSome_get?
 
 theorem mem_iff_isSome_get? {a : α} : a ∈ m ↔ (get? m a).isSome :=
-  m.inductionOn fun _ => Std.DHashMap.Const.mem_iff_isSome_get?
+  m.inductionOn fun _ => DHashMap.Const.mem_iff_isSome_get?
 
 theorem get?_eq_none_of_contains_eq_false {a : α} :
     m.contains a = false → get? m a = none :=
-  m.inductionOn fun _ => Std.DHashMap.Const.get?_eq_none_of_contains_eq_false
+  m.inductionOn fun _ => DHashMap.Const.get?_eq_none_of_contains_eq_false
 
 theorem get?_eq_none {a : α} : ¬a ∈ m → get? m a = none := by
   simpa [mem_iff_contains] using get?_eq_none_of_contains_eq_false
 
 theorem get?_erase {k a : α} :
     Const.get? (m.erase k) a = if k == a then none else get? m a :=
-  m.inductionOn fun _ => Std.DHashMap.Const.get?_erase
+  m.inductionOn fun _ => DHashMap.Const.get?_erase
 
 @[simp]
 theorem get?_erase_self {k : α} : get? (m.erase k) k = none :=
-  m.inductionOn fun _ => Std.DHashMap.Const.get?_erase_self
+  m.inductionOn fun _ => DHashMap.Const.get?_erase_self
 
 theorem get?_eq_get? [LawfulBEq α] {a : α} : get? m a = m.get? a :=
-  m.inductionOn fun _ => Std.DHashMap.Const.get?_eq_get?
+  m.inductionOn fun _ => DHashMap.Const.get?_eq_get?
 
 theorem get?_congr {a b : α} (hab : a == b) : get? m a = get? m b :=
-  m.inductionOn fun _ => Std.DHashMap.Const.get?_congr hab
+  m.inductionOn fun _ => DHashMap.Const.get?_congr hab
 
 end Const
 
@@ -257,348 +257,348 @@ theorem get_insert [LawfulBEq α] {k a : α} {v : β k} {h₁} :
         cast (congrArg β (eq_of_beq h₂)) v
       else
         m.get a (mem_of_mem_insert h₁ (Bool.eq_false_iff.2 h₂)) :=
-  m.inductionOn (fun _ _ => Std.DHashMap.get_insert) h₁
+  m.inductionOn (fun _ _ => DHashMap.get_insert) h₁
 
 @[simp]
 theorem get_insert_self [LawfulBEq α] {k : α} {v : β k} :
     (m.insert k v).get k mem_insert_self = v :=
-  m.inductionOn fun _ => Std.DHashMap.get_insert_self
+  m.inductionOn fun _ => DHashMap.get_insert_self
 
 @[simp]
 theorem get_erase [LawfulBEq α] {k a : α} {h'} :
     (m.erase k).get a h' = m.get a (mem_of_mem_erase h') :=
-  m.inductionOn (fun _ _ => Std.DHashMap.get_erase) h'
+  m.inductionOn (fun _ _ => DHashMap.get_erase) h'
 
 theorem get?_eq_some_get [LawfulBEq α] {a : α} (h) : m.get? a = some (m.get a h) :=
-  m.inductionOn (fun _ h => Std.DHashMap.get?_eq_some_get h) h
+  m.inductionOn (fun _ h => DHashMap.get?_eq_some_get h) h
 
 theorem get_eq_get_get? [LawfulBEq α] {a : α} {h} :
     m.get a h = (m.get? a).get (mem_iff_isSome_get?.mp h) :=
-  m.inductionOn (fun _ _ => Std.DHashMap.get_eq_get_get?) h
+  m.inductionOn (fun _ _ => DHashMap.get_eq_get_get?) h
 
 theorem get_get? [LawfulBEq α] {a : α} {h} :
     (m.get? a).get h = m.get a (mem_iff_isSome_get?.mpr h) :=
-  m.inductionOn (fun _ _ => Std.DHashMap.get_get?) h
+  m.inductionOn (fun _ _ => DHashMap.get_get?) h
 
 namespace Const
 
-variable {β : Type v} {m : DHashMap α (fun _ => β)}
+variable {β : Type v} {m : ExtDHashMap α (fun _ => β)}
 
 theorem get_insert {k a : α} {v : β} {h₁} :
     get (m.insert k v) a h₁ =
       if h₂ : k == a then v else get m a (mem_of_mem_insert h₁ (Bool.eq_false_iff.2 h₂)) :=
-  m.inductionOn (fun _ _ => Std.DHashMap.Const.get_insert) h₁
+  m.inductionOn (fun _ _ => DHashMap.Const.get_insert) h₁
 
 @[simp]
 theorem get_insert_self {k : α} {v : β} :
     get (m.insert k v) k mem_insert_self = v :=
-  m.inductionOn fun _ => Std.DHashMap.Const.get_insert_self
+  m.inductionOn fun _ => DHashMap.Const.get_insert_self
 
 @[simp]
 theorem get_erase {k a : α} {h'} :
     get (m.erase k) a h' = get m a (mem_of_mem_erase h') :=
-  m.inductionOn (fun _ _ => Std.DHashMap.Const.get_erase) h'
+  m.inductionOn (fun _ _ => DHashMap.Const.get_erase) h'
 
 theorem get?_eq_some_get {a : α} (h) :
     get? m a = some (get m a h) :=
-  m.inductionOn (fun _ h => Std.DHashMap.Const.get?_eq_some_get h) h
+  m.inductionOn (fun _ h => DHashMap.Const.get?_eq_some_get h) h
 
 theorem get_eq_get_get? {a : α} {h} :
     get m a h = (get? m a).get (mem_iff_isSome_get?.mp h) :=
-  m.inductionOn (fun _ _ => Std.DHashMap.Const.get_eq_get_get?) h
+  m.inductionOn (fun _ _ => DHashMap.Const.get_eq_get_get?) h
 
 theorem get_get? {a : α} {h} :
     (get? m a).get h = get m a (mem_iff_isSome_get?.mpr h) :=
-  m.inductionOn (fun _ _ => Std.DHashMap.Const.get_get?) h
+  m.inductionOn (fun _ _ => DHashMap.Const.get_get?) h
 
 theorem get_eq_get [LawfulBEq α] {a : α} {h} : get m a h = m.get a h :=
-  m.inductionOn (fun _ _ => Std.DHashMap.Const.get_eq_get) h
+  m.inductionOn (fun _ _ => DHashMap.Const.get_eq_get) h
 
 theorem get_congr {a b : α} (hab : a == b) {h'} :
     get m a h' = get m b ((mem_congr hab).1 h') :=
-  m.inductionOn (fun _ hab _ => Std.DHashMap.Const.get_congr hab) hab h'
+  m.inductionOn (fun _ hab _ => DHashMap.Const.get_congr hab) hab h'
 
 end Const
 
 @[simp]
 theorem get!_empty [LawfulBEq α] {a : α} [Inhabited (β a)] :
-    (∅ : DHashMap α β).get! a = default :=
-  Std.DHashMap.get!_empty
+    (∅ : ExtDHashMap α β).get! a = default :=
+  DHashMap.get!_empty
 
 theorem get!_insert [LawfulBEq α] {k a : α} [Inhabited (β a)] {v : β k} :
     (m.insert k v).get! a =
       if h : k == a then cast (congrArg β (eq_of_beq h)) v else m.get! a :=
-  m.inductionOn fun _ => Std.DHashMap.get!_insert
+  m.inductionOn fun _ => DHashMap.get!_insert
 
 @[simp]
 theorem get!_insert_self [LawfulBEq α] {a : α} [Inhabited (β a)] {b : β a} :
     (m.insert a b).get! a = b :=
-  m.inductionOn fun _ => Std.DHashMap.get!_insert_self
+  m.inductionOn fun _ => DHashMap.get!_insert_self
 
 theorem get!_eq_default_of_contains_eq_false [LawfulBEq α] {a : α} [Inhabited (β a)] :
     m.contains a = false → m.get! a = default :=
-  m.inductionOn fun _ => Std.DHashMap.get!_eq_default_of_contains_eq_false
+  m.inductionOn fun _ => DHashMap.get!_eq_default_of_contains_eq_false
 
 theorem get!_eq_default [LawfulBEq α] {a : α} [Inhabited (β a)] :
     ¬a ∈ m → m.get! a = default :=
-  m.inductionOn fun _ => Std.DHashMap.get!_eq_default
+  m.inductionOn fun _ => DHashMap.get!_eq_default
 
 theorem get!_erase [LawfulBEq α] {k a : α} [Inhabited (β a)] :
     (m.erase k).get! a = if k == a then default else m.get! a :=
-  m.inductionOn fun _ => Std.DHashMap.get!_erase
+  m.inductionOn fun _ => DHashMap.get!_erase
 
 @[simp]
 theorem get!_erase_self [LawfulBEq α] {k : α} [Inhabited (β k)] :
     (m.erase k).get! k = default :=
-  m.inductionOn fun _ => Std.DHashMap.get!_erase_self
+  m.inductionOn fun _ => DHashMap.get!_erase_self
 
 theorem get?_eq_some_get!_of_contains [LawfulBEq α] {a : α} [Inhabited (β a)] :
     m.contains a = true → m.get? a = some (m.get! a) :=
-  m.inductionOn fun _ => Std.DHashMap.get?_eq_some_get!_of_contains
+  m.inductionOn fun _ => DHashMap.get?_eq_some_get!_of_contains
 
 theorem get?_eq_some_get! [LawfulBEq α] {a : α} [Inhabited (β a)] :
     a ∈ m → m.get? a = some (m.get! a) :=
-  m.inductionOn fun _ => Std.DHashMap.get?_eq_some_get!
+  m.inductionOn fun _ => DHashMap.get?_eq_some_get!
 
 theorem get!_eq_get!_get? [LawfulBEq α] {a : α} [Inhabited (β a)] :
     m.get! a = (m.get? a).get! :=
-  m.inductionOn fun _ => Std.DHashMap.get!_eq_get!_get?
+  m.inductionOn fun _ => DHashMap.get!_eq_get!_get?
 
 theorem get_eq_get! [LawfulBEq α] {a : α} [Inhabited (β a)] {h} :
     m.get a h = m.get! a :=
-  m.inductionOn (fun _ _ => Std.DHashMap.get_eq_get!) h
+  m.inductionOn (fun _ _ => DHashMap.get_eq_get!) h
 
 namespace Const
 
-variable {β : Type v} {m : DHashMap α (fun _ => β)}
+variable {β : Type v} {m : ExtDHashMap α (fun _ => β)}
 
 @[simp]
-theorem get!_empty [Inhabited β] {a : α} : get! (∅ : DHashMap α (fun _ => β)) a = default :=
-  Std.DHashMap.Const.get!_empty
+theorem get!_empty [Inhabited β] {a : α} : get! (∅ : ExtDHashMap α (fun _ => β)) a = default :=
+  DHashMap.Const.get!_empty
 
 theorem get!_insert [Inhabited β] {k a : α} {v : β} :
     get! (m.insert k v) a = if k == a then v else get! m a :=
-  m.inductionOn fun _ => Std.DHashMap.Const.get!_insert
+  m.inductionOn fun _ => DHashMap.Const.get!_insert
 
 @[simp]
 theorem get!_insert_self [Inhabited β] {k : α} {v : β} :
     get! (m.insert k v) k = v :=
-  m.inductionOn fun _ => Std.DHashMap.Const.get!_insert_self
+  m.inductionOn fun _ => DHashMap.Const.get!_insert_self
 
 theorem get!_eq_default_of_contains_eq_false [Inhabited β] {a : α} :
     m.contains a = false → get! m a = default :=
-  m.inductionOn fun _ => Std.DHashMap.Const.get!_eq_default_of_contains_eq_false
+  m.inductionOn fun _ => DHashMap.Const.get!_eq_default_of_contains_eq_false
 
 theorem get!_eq_default [Inhabited β] {a : α} :
     ¬a ∈ m → get! m a = default :=
-  m.inductionOn fun _ => Std.DHashMap.Const.get!_eq_default
+  m.inductionOn fun _ => DHashMap.Const.get!_eq_default
 
 theorem get!_erase [Inhabited β] {k a : α} :
     get! (m.erase k) a = if k == a then default else get! m a :=
-  m.inductionOn fun _ => Std.DHashMap.Const.get!_erase
+  m.inductionOn fun _ => DHashMap.Const.get!_erase
 
 @[simp]
 theorem get!_erase_self [Inhabited β] {k : α} :
     get! (m.erase k) k = default :=
-  m.inductionOn fun _ => Std.DHashMap.Const.get!_erase_self
+  m.inductionOn fun _ => DHashMap.Const.get!_erase_self
 
 theorem get?_eq_some_get!_of_contains [Inhabited β] {a : α} :
     m.contains a = true → get? m a = some (get! m a) :=
-  m.inductionOn fun _ => Std.DHashMap.Const.get?_eq_some_get!_of_contains
+  m.inductionOn fun _ => DHashMap.Const.get?_eq_some_get!_of_contains
 
 theorem get?_eq_some_get! [Inhabited β] {a : α} :
     a ∈ m → get? m a = some (get! m a) :=
-  m.inductionOn fun _ => Std.DHashMap.Const.get?_eq_some_get!
+  m.inductionOn fun _ => DHashMap.Const.get?_eq_some_get!
 
 theorem get!_eq_get!_get? [Inhabited β] {a : α} :
     get! m a = (get? m a).get! :=
-  m.inductionOn fun _ => Std.DHashMap.Const.get!_eq_get!_get?
+  m.inductionOn fun _ => DHashMap.Const.get!_eq_get!_get?
 
 theorem get_eq_get! [Inhabited β] {a : α} {h} :
     get m a h = get! m a :=
-  m.inductionOn (fun _ _ => Std.DHashMap.Const.get_eq_get!) h
+  m.inductionOn (fun _ _ => DHashMap.Const.get_eq_get!) h
 
 theorem get!_eq_get! [LawfulBEq α] [Inhabited β] {a : α} :
     get! m a = m.get! a :=
-  m.inductionOn fun _ => Std.DHashMap.Const.get!_eq_get!
+  m.inductionOn fun _ => DHashMap.Const.get!_eq_get!
 
 theorem get!_congr [Inhabited β] {a b : α} (hab : a == b) :
     get! m a = get! m b :=
-  m.inductionOn (fun _ hab => Std.DHashMap.Const.get!_congr hab) hab
+  m.inductionOn (fun _ hab => DHashMap.Const.get!_congr hab) hab
 
 end Const
 
 @[simp]
 theorem getD_empty [LawfulBEq α] {a : α} {fallback : β a} :
-    (∅ : DHashMap α β).getD a fallback = fallback :=
-  Std.DHashMap.getD_empty
+    (∅ : ExtDHashMap α β).getD a fallback = fallback :=
+  DHashMap.getD_empty
 
 theorem getD_insert [LawfulBEq α] {k a : α} {fallback : β a} {v : β k} :
     (m.insert k v).getD a fallback =
       if h : k == a then cast (congrArg β (eq_of_beq h)) v else m.getD a fallback :=
-  m.inductionOn fun _ => Std.DHashMap.getD_insert
+  m.inductionOn fun _ => DHashMap.getD_insert
 
 @[simp]
 theorem getD_insert_self [LawfulBEq α] {k : α} {fallback v : β k} :
     (m.insert k v).getD k fallback = v :=
-  m.inductionOn fun _ => Std.DHashMap.getD_insert_self
+  m.inductionOn fun _ => DHashMap.getD_insert_self
 
 theorem getD_eq_fallback_of_contains_eq_false [LawfulBEq α] {a : α} {fallback : β a} :
     m.contains a = false → m.getD a fallback = fallback :=
-  m.inductionOn fun _ => Std.DHashMap.getD_eq_fallback_of_contains_eq_false
+  m.inductionOn fun _ => DHashMap.getD_eq_fallback_of_contains_eq_false
 
 theorem getD_eq_fallback [LawfulBEq α] {a : α} {fallback : β a} :
     ¬a ∈ m → m.getD a fallback = fallback :=
-  m.inductionOn fun _ => Std.DHashMap.getD_eq_fallback
+  m.inductionOn fun _ => DHashMap.getD_eq_fallback
 
 theorem getD_erase [LawfulBEq α] {k a : α} {fallback : β a} :
     (m.erase k).getD a fallback = if k == a then fallback else m.getD a fallback :=
-  m.inductionOn fun _ => Std.DHashMap.getD_erase
+  m.inductionOn fun _ => DHashMap.getD_erase
 
 @[simp]
 theorem getD_erase_self [LawfulBEq α] {k : α} {fallback : β k} :
     (m.erase k).getD k fallback = fallback :=
-  m.inductionOn fun _ => Std.DHashMap.getD_erase_self
+  m.inductionOn fun _ => DHashMap.getD_erase_self
 
 theorem get?_eq_some_getD_of_contains [LawfulBEq α] {a : α} {fallback : β a} :
     m.contains a = true → m.get? a = some (m.getD a fallback) :=
-  m.inductionOn fun _ => Std.DHashMap.get?_eq_some_getD_of_contains
+  m.inductionOn fun _ => DHashMap.get?_eq_some_getD_of_contains
 
 theorem get?_eq_some_getD [LawfulBEq α] {a : α} {fallback : β a} :
     a ∈ m → m.get? a = some (m.getD a fallback) :=
-  m.inductionOn fun _ => Std.DHashMap.get?_eq_some_getD
+  m.inductionOn fun _ => DHashMap.get?_eq_some_getD
 
 theorem getD_eq_getD_get? [LawfulBEq α] {a : α} {fallback : β a} :
     m.getD a fallback = (m.get? a).getD fallback :=
-  m.inductionOn fun _ => Std.DHashMap.getD_eq_getD_get?
+  m.inductionOn fun _ => DHashMap.getD_eq_getD_get?
 
 theorem get_eq_getD [LawfulBEq α] {a : α} {fallback : β a} {h} :
     m.get a h = m.getD a fallback :=
-  m.inductionOn (fun _ _ => Std.DHashMap.get_eq_getD) h
+  m.inductionOn (fun _ _ => DHashMap.get_eq_getD) h
 
 theorem get!_eq_getD_default [LawfulBEq α] {a : α} [Inhabited (β a)] :
     m.get! a = m.getD a default :=
-  m.inductionOn fun _ => Std.DHashMap.get!_eq_getD_default
+  m.inductionOn fun _ => DHashMap.get!_eq_getD_default
 
 namespace Const
 
-variable {β : Type v} {m : DHashMap α (fun _ => β)}
+variable {β : Type v} {m : ExtDHashMap α (fun _ => β)}
 
 @[simp]
 theorem getD_empty {a : α} {fallback : β} :
-    getD (∅ : DHashMap α (fun _ => β)) a fallback = fallback :=
-  Std.DHashMap.Const.getD_empty
+    getD (∅ : ExtDHashMap α (fun _ => β)) a fallback = fallback :=
+  DHashMap.Const.getD_empty
 
 theorem getD_insert {k a : α} {fallback v : β} :
     getD (m.insert k v) a fallback = if k == a then v else getD m a fallback :=
-  m.inductionOn fun _ => Std.DHashMap.Const.getD_insert
+  m.inductionOn fun _ => DHashMap.Const.getD_insert
 
 @[simp]
 theorem getD_insert_self {k : α} {fallback v : β} :
    getD (m.insert k v) k fallback = v :=
-  m.inductionOn fun _ => Std.DHashMap.Const.getD_insert_self
+  m.inductionOn fun _ => DHashMap.Const.getD_insert_self
 
 theorem getD_eq_fallback_of_contains_eq_false {a : α}
     {fallback : β} : m.contains a = false → getD m a fallback = fallback :=
-  m.inductionOn fun _ => Std.DHashMap.Const.getD_eq_fallback_of_contains_eq_false
+  m.inductionOn fun _ => DHashMap.Const.getD_eq_fallback_of_contains_eq_false
 
 theorem getD_eq_fallback {a : α} {fallback : β} :
     ¬a ∈ m → getD m a fallback = fallback :=
-  m.inductionOn fun _ => Std.DHashMap.Const.getD_eq_fallback
+  m.inductionOn fun _ => DHashMap.Const.getD_eq_fallback
 
 theorem getD_erase {k a : α} {fallback : β} :
     getD (m.erase k) a fallback = if k == a then fallback else getD m a fallback :=
-  m.inductionOn fun _ => Std.DHashMap.Const.getD_erase
+  m.inductionOn fun _ => DHashMap.Const.getD_erase
 
 @[simp]
 theorem getD_erase_self {k : α} {fallback : β} :
     getD (m.erase k) k fallback = fallback :=
-  m.inductionOn fun _ => Std.DHashMap.Const.getD_erase_self
+  m.inductionOn fun _ => DHashMap.Const.getD_erase_self
 
 theorem get?_eq_some_getD_of_contains {a : α} {fallback : β} :
     m.contains a = true → get? m a = some (getD m a fallback) :=
-  m.inductionOn fun _ => Std.DHashMap.Const.get?_eq_some_getD_of_contains
+  m.inductionOn fun _ => DHashMap.Const.get?_eq_some_getD_of_contains
 
 theorem get?_eq_some_getD {a : α} {fallback : β} :
     a ∈ m → get? m a = some (getD m a fallback) :=
-  m.inductionOn fun _ => Std.DHashMap.Const.get?_eq_some_getD
+  m.inductionOn fun _ => DHashMap.Const.get?_eq_some_getD
 
 theorem getD_eq_getD_get? {a : α} {fallback : β} :
     getD m a fallback = (get? m a).getD fallback :=
-  m.inductionOn fun _ => Std.DHashMap.Const.getD_eq_getD_get?
+  m.inductionOn fun _ => DHashMap.Const.getD_eq_getD_get?
 
 theorem get_eq_getD {a : α} {fallback : β} {h} :
     get m a h = getD m a fallback :=
-  m.inductionOn (fun _ _ => Std.DHashMap.Const.get_eq_getD) h
+  m.inductionOn (fun _ _ => DHashMap.Const.get_eq_getD) h
 
 theorem get!_eq_getD_default [Inhabited β] {a : α} :
     get! m a = getD m a default :=
-  m.inductionOn fun _ => Std.DHashMap.Const.get!_eq_getD_default
+  m.inductionOn fun _ => DHashMap.Const.get!_eq_getD_default
 
 theorem getD_eq_getD [LawfulBEq α] {a : α} {fallback : β} :
     getD m a fallback = m.getD a fallback :=
-  m.inductionOn fun _ => Std.DHashMap.Const.getD_eq_getD
+  m.inductionOn fun _ => DHashMap.Const.getD_eq_getD
 
 theorem getD_congr {a b : α} {fallback : β} (hab : a == b) :
     getD m a fallback = getD m b fallback :=
-  m.inductionOn (fun _ hab => Std.DHashMap.Const.getD_congr hab) hab
+  m.inductionOn (fun _ hab => DHashMap.Const.getD_congr hab) hab
 
 end Const
 
 @[simp]
-theorem getKey?_empty {a : α} : (∅ : DHashMap α β).getKey? a = none :=
-  Std.DHashMap.getKey?_empty
+theorem getKey?_empty {a : α} : (∅ : ExtDHashMap α β).getKey? a = none :=
+  DHashMap.getKey?_empty
 
 theorem getKey?_insert {a k : α} {v : β k} :
     (m.insert k v).getKey? a = if k == a then some k else m.getKey? a :=
-  m.inductionOn fun _ => Std.DHashMap.getKey?_insert
+  m.inductionOn fun _ => DHashMap.getKey?_insert
 
 @[simp]
 theorem getKey?_insert_self {k : α} {v : β k} :
     (m.insert k v).getKey? k = some k :=
-  m.inductionOn fun _ => Std.DHashMap.getKey?_insert_self
+  m.inductionOn fun _ => DHashMap.getKey?_insert_self
 
 theorem contains_eq_isSome_getKey? {a : α} :
     m.contains a = (m.getKey? a).isSome :=
-  m.inductionOn fun _ => Std.DHashMap.contains_eq_isSome_getKey?
+  m.inductionOn fun _ => DHashMap.contains_eq_isSome_getKey?
 
 theorem mem_iff_isSome_getKey? {a : α} :
     a ∈ m ↔ (m.getKey? a).isSome :=
-  m.inductionOn fun _ => Std.DHashMap.mem_iff_isSome_getKey?
+  m.inductionOn fun _ => DHashMap.mem_iff_isSome_getKey?
 
 theorem mem_of_getKey?_eq_some {k k' : α}
     (h : m.getKey? k = some k') : k' ∈ m :=
-  m.inductionOn (fun _ h => Std.DHashMap.mem_of_getKey?_eq_some h) h
+  m.inductionOn (fun _ h => DHashMap.mem_of_getKey?_eq_some h) h
 
 theorem getKey?_eq_none_of_contains_eq_false {a : α} :
     m.contains a = false → m.getKey? a = none :=
-  m.inductionOn fun _ => Std.DHashMap.getKey?_eq_none_of_contains_eq_false
+  m.inductionOn fun _ => DHashMap.getKey?_eq_none_of_contains_eq_false
 
 theorem getKey?_eq_none {a : α} : ¬a ∈ m → m.getKey? a = none :=
-  m.inductionOn fun _ => Std.DHashMap.getKey?_eq_none
+  m.inductionOn fun _ => DHashMap.getKey?_eq_none
 
 theorem getKey?_erase {k a : α} :
     (m.erase k).getKey? a = if k == a then none else m.getKey? a :=
-  m.inductionOn fun _ => Std.DHashMap.getKey?_erase
+  m.inductionOn fun _ => DHashMap.getKey?_erase
 
 @[simp]
 theorem getKey?_erase_self {k : α} : (m.erase k).getKey? k = none :=
-  m.inductionOn fun _ => Std.DHashMap.getKey?_erase_self
+  m.inductionOn fun _ => DHashMap.getKey?_erase_self
 
 theorem getKey?_beq {k : α} :
     (m.getKey? k).all (· == k) :=
-  m.inductionOn fun _ => Std.DHashMap.getKey?_beq
+  m.inductionOn fun _ => DHashMap.getKey?_beq
 
 theorem getKey?_congr {k k' : α} (h : k == k') :
     m.getKey? k = m.getKey? k' :=
-  m.inductionOn (fun _ h => Std.DHashMap.getKey?_congr h) h
+  m.inductionOn (fun _ h => DHashMap.getKey?_congr h) h
 
 theorem getKey?_eq_some_of_contains [LawfulBEq α] {k : α} (h : m.contains k) :
     m.getKey? k = some k :=
-  m.inductionOn (fun _ h => Std.DHashMap.getKey?_eq_some_of_contains h) h
+  m.inductionOn (fun _ h => DHashMap.getKey?_eq_some_of_contains h) h
 
 theorem getKey?_eq_some [LawfulBEq α] {k : α} (h : k ∈ m) : m.getKey? k = some k :=
-  m.inductionOn (fun _ h => Std.DHashMap.getKey?_eq_some h) h
+  m.inductionOn (fun _ h => DHashMap.getKey?_eq_some h) h
 
 theorem getKey_insert {k a : α} {v : β k} {h₁} :
     (m.insert k v).getKey a h₁ =
@@ -606,304 +606,304 @@ theorem getKey_insert {k a : α} {v : β k} {h₁} :
         k
       else
         m.getKey a (mem_of_mem_insert h₁ (Bool.eq_false_iff.2 h₂)) :=
-  m.inductionOn (fun _ _ => Std.DHashMap.getKey_insert) h₁
+  m.inductionOn (fun _ _ => DHashMap.getKey_insert) h₁
 
 @[simp]
 theorem getKey_insert_self {k : α} {v : β k} :
     (m.insert k v).getKey k mem_insert_self = k :=
-  m.inductionOn fun _ => Std.DHashMap.getKey_insert_self
+  m.inductionOn fun _ => DHashMap.getKey_insert_self
 
 @[simp]
 theorem getKey_erase {k a : α} {h'} :
     (m.erase k).getKey a h' = m.getKey a (mem_of_mem_erase h') :=
-  m.inductionOn (fun _ _ => Std.DHashMap.getKey_erase) h'
+  m.inductionOn (fun _ _ => DHashMap.getKey_erase) h'
 
 theorem getKey?_eq_some_getKey {a : α} (h) :
     m.getKey? a = some (m.getKey a h) :=
-  m.inductionOn (fun _ h => Std.DHashMap.getKey?_eq_some_getKey h) h
+  m.inductionOn (fun _ h => DHashMap.getKey?_eq_some_getKey h) h
 
 theorem getKey_eq_get_getKey? {a : α} {h} :
     m.getKey a h = (m.getKey? a).get (mem_iff_isSome_getKey?.mp h) :=
-  m.inductionOn (fun _ _ => Std.DHashMap.getKey_eq_get_getKey?) h
+  m.inductionOn (fun _ _ => DHashMap.getKey_eq_get_getKey?) h
 
 theorem get_getKey? {a : α} {h} :
     (m.getKey? a).get h = m.getKey a (mem_iff_isSome_getKey?.mpr h) :=
-  m.inductionOn (fun _ _ => Std.DHashMap.get_getKey?) h
+  m.inductionOn (fun _ _ => DHashMap.get_getKey?) h
 
 theorem getKey_beq {k : α} (h : k ∈ m) : m.getKey k h == k :=
-  m.inductionOn (fun _ h => Std.DHashMap.getKey_beq h) h
+  m.inductionOn (fun _ h => DHashMap.getKey_beq h) h
 
 theorem getKey_congr {k₁ k₂ : α} (h : k₁ == k₂)
     (h₁ : k₁ ∈ m) : m.getKey k₁ h₁ = m.getKey k₂ ((mem_congr h).mp h₁) :=
-  m.inductionOn (fun _ h h₁ => Std.DHashMap.getKey_congr h h₁) h h₁
+  m.inductionOn (fun _ h h₁ => DHashMap.getKey_congr h h₁) h h₁
 
 theorem getKey_eq [LawfulBEq α] {k : α} (h : k ∈ m) : m.getKey k h = k :=
-  m.inductionOn (fun _ h => Std.DHashMap.getKey_eq h) h
+  m.inductionOn (fun _ h => DHashMap.getKey_eq h) h
 
 @[simp]
 theorem getKey!_empty [Inhabited α] {a : α} :
-    (∅ : DHashMap α β).getKey! a = default :=
-  Std.DHashMap.getKey!_empty
+    (∅ : ExtDHashMap α β).getKey! a = default :=
+  DHashMap.getKey!_empty
 
 theorem getKey!_insert [Inhabited α] {k a : α} {v : β k} :
     (m.insert k v).getKey! a =
       if k == a then k else m.getKey! a :=
-  m.inductionOn fun _ => Std.DHashMap.getKey!_insert
+  m.inductionOn fun _ => DHashMap.getKey!_insert
 
 @[simp]
 theorem getKey!_insert_self [Inhabited α] {a : α} {b : β a} :
     (m.insert a b).getKey! a = a :=
-  m.inductionOn fun _ => Std.DHashMap.getKey!_insert_self
+  m.inductionOn fun _ => DHashMap.getKey!_insert_self
 
 theorem getKey!_eq_default_of_contains_eq_false [Inhabited α]
     {a : α} :
     m.contains a = false → m.getKey! a = default :=
-  m.inductionOn fun _ => Std.DHashMap.getKey!_eq_default_of_contains_eq_false
+  m.inductionOn fun _ => DHashMap.getKey!_eq_default_of_contains_eq_false
 
 theorem getKey!_eq_default [Inhabited α] {a : α} :
     ¬a ∈ m → m.getKey! a = default :=
-  m.inductionOn fun _ => Std.DHashMap.getKey!_eq_default
+  m.inductionOn fun _ => DHashMap.getKey!_eq_default
 
 theorem getKey!_erase [Inhabited α] {k a : α} :
     (m.erase k).getKey! a = if k == a then default else m.getKey! a :=
-  m.inductionOn fun _ => Std.DHashMap.getKey!_erase
+  m.inductionOn fun _ => DHashMap.getKey!_erase
 
 @[simp]
 theorem getKey!_erase_self [Inhabited α] {k : α} :
     (m.erase k).getKey! k = default :=
-  m.inductionOn fun _ => Std.DHashMap.getKey!_erase_self
+  m.inductionOn fun _ => DHashMap.getKey!_erase_self
 
 theorem getKey?_eq_some_getKey!_of_contains [Inhabited α] {a : α} :
     m.contains a = true → m.getKey? a = some (m.getKey! a) :=
-  m.inductionOn fun _ => Std.DHashMap.getKey?_eq_some_getKey!_of_contains
+  m.inductionOn fun _ => DHashMap.getKey?_eq_some_getKey!_of_contains
 
 theorem getKey?_eq_some_getKey! [Inhabited α] {a : α} :
     a ∈ m → m.getKey? a = some (m.getKey! a) :=
-  m.inductionOn fun _ => Std.DHashMap.getKey?_eq_some_getKey!
+  m.inductionOn fun _ => DHashMap.getKey?_eq_some_getKey!
 
 theorem getKey!_eq_get!_getKey? [Inhabited α] {a : α} :
     m.getKey! a = (m.getKey? a).get! :=
-  m.inductionOn fun _ => Std.DHashMap.getKey!_eq_get!_getKey?
+  m.inductionOn fun _ => DHashMap.getKey!_eq_get!_getKey?
 
 theorem getKey_eq_getKey! [Inhabited α] {a : α} {h} :
     m.getKey a h = m.getKey! a :=
-  m.inductionOn (fun _ _ => Std.DHashMap.getKey_eq_getKey!) h
+  m.inductionOn (fun _ _ => DHashMap.getKey_eq_getKey!) h
 
 theorem getKey!_congr [Inhabited α] {k k' : α} (h : k == k') :
     m.getKey! k = m.getKey! k' :=
-  m.inductionOn (fun _ h => Std.DHashMap.getKey!_congr h) h
+  m.inductionOn (fun _ h => DHashMap.getKey!_congr h) h
 
 theorem getKey!_eq_of_contains [LawfulBEq α] [Inhabited α] {k : α} (h : m.contains k) :
     m.getKey! k = k :=
-  m.inductionOn (fun _ h => Std.DHashMap.getKey!_eq_of_contains h) h
+  m.inductionOn (fun _ h => DHashMap.getKey!_eq_of_contains h) h
 
 theorem getKey!_eq_of_mem [LawfulBEq α] [Inhabited α] {k : α} (h : k ∈ m) : m.getKey! k = k :=
-  m.inductionOn (fun _ h => Std.DHashMap.getKey!_eq_of_mem h) h
+  m.inductionOn (fun _ h => DHashMap.getKey!_eq_of_mem h) h
 
 @[simp]
 theorem getKeyD_empty {a fallback : α} :
-    (∅ : DHashMap α β).getKeyD a fallback = fallback :=
-  Std.DHashMap.getKeyD_empty
+    (∅ : ExtDHashMap α β).getKeyD a fallback = fallback :=
+  DHashMap.getKeyD_empty
 
 theorem getKeyD_insert {k a fallback : α} {v : β k} :
     (m.insert k v).getKeyD a fallback =
       if k == a then k else m.getKeyD a fallback :=
-  m.inductionOn fun _ => Std.DHashMap.getKeyD_insert
+  m.inductionOn fun _ => DHashMap.getKeyD_insert
 
 @[simp]
 theorem getKeyD_insert_self {k fallback : α} {v : β k} :
     (m.insert k v).getKeyD k fallback = k :=
-  m.inductionOn fun _ => Std.DHashMap.getKeyD_insert_self
+  m.inductionOn fun _ => DHashMap.getKeyD_insert_self
 
 theorem getKeyD_eq_fallback_of_contains_eq_false {a : α}
     {fallback : α} :
     m.contains a = false → m.getKeyD a fallback = fallback :=
-  m.inductionOn fun _ => Std.DHashMap.getKeyD_eq_fallback_of_contains_eq_false
+  m.inductionOn fun _ => DHashMap.getKeyD_eq_fallback_of_contains_eq_false
 
 theorem getKeyD_eq_fallback {a fallback : α} :
     ¬a ∈ m → m.getKeyD a fallback = fallback :=
-  m.inductionOn fun _ => Std.DHashMap.getKeyD_eq_fallback
+  m.inductionOn fun _ => DHashMap.getKeyD_eq_fallback
 
 theorem getKeyD_erase {k a fallback : α} :
     (m.erase k).getKeyD a fallback = if k == a then fallback else m.getKeyD a fallback :=
-  m.inductionOn fun _ => Std.DHashMap.getKeyD_erase
+  m.inductionOn fun _ => DHashMap.getKeyD_erase
 
 @[simp]
 theorem getKeyD_erase_self {k fallback : α} :
     (m.erase k).getKeyD k fallback = fallback :=
-  m.inductionOn fun _ => Std.DHashMap.getKeyD_erase_self
+  m.inductionOn fun _ => DHashMap.getKeyD_erase_self
 
 theorem getKey?_eq_some_getKeyD_of_contains {a fallback : α} :
     m.contains a = true → m.getKey? a = some (m.getKeyD a fallback) :=
-  m.inductionOn fun _ => Std.DHashMap.getKey?_eq_some_getKeyD_of_contains
+  m.inductionOn fun _ => DHashMap.getKey?_eq_some_getKeyD_of_contains
 
 theorem getKey?_eq_some_getKeyD {a fallback : α} :
     a ∈ m → m.getKey? a = some (m.getKeyD a fallback) :=
-  m.inductionOn fun _ => Std.DHashMap.getKey?_eq_some_getKeyD
+  m.inductionOn fun _ => DHashMap.getKey?_eq_some_getKeyD
 
 theorem getKeyD_eq_getD_getKey? {a fallback : α} :
     m.getKeyD a fallback = (m.getKey? a).getD fallback :=
-  m.inductionOn fun _ => Std.DHashMap.getKeyD_eq_getD_getKey?
+  m.inductionOn fun _ => DHashMap.getKeyD_eq_getD_getKey?
 
 theorem getKey_eq_getKeyD {a fallback : α} {h} :
     m.getKey a h = m.getKeyD a fallback :=
-  m.inductionOn (fun _ _ => Std.DHashMap.getKey_eq_getKeyD) h
+  m.inductionOn (fun _ _ => DHashMap.getKey_eq_getKeyD) h
 
 theorem getKey!_eq_getKeyD_default [Inhabited α] {a : α} :
     m.getKey! a = m.getKeyD a default :=
-  m.inductionOn fun _ => Std.DHashMap.getKey!_eq_getKeyD_default
+  m.inductionOn fun _ => DHashMap.getKey!_eq_getKeyD_default
 
 theorem getKeyD_congr {k k' fallback : α}
     (h : k == k') : m.getKeyD k fallback = m.getKeyD k' fallback :=
-  m.inductionOn (fun _ h => Std.DHashMap.getKeyD_congr h) h
+  m.inductionOn (fun _ h => DHashMap.getKeyD_congr h) h
 
 theorem getKeyD_eq_of_contains [LawfulBEq α] {k fallback : α} (h : m.contains k) :
     m.getKeyD k fallback = k :=
-  m.inductionOn (fun _ h => Std.DHashMap.getKeyD_eq_of_contains h) h
+  m.inductionOn (fun _ h => DHashMap.getKeyD_eq_of_contains h) h
 
 theorem getKeyD_eq_of_mem [LawfulBEq α] {k fallback : α} (h : k ∈ m) :
     m.getKeyD k fallback = k :=
-  m.inductionOn (fun _ h => Std.DHashMap.getKeyD_eq_of_mem h) h
+  m.inductionOn (fun _ h => DHashMap.getKeyD_eq_of_mem h) h
 
 @[simp]
 theorem not_insertIfNew_eq_empty {k : α} {v : β k} :
     ¬m.insertIfNew k v = ∅ :=
-  isEmpty_eq_false_iff.mp <| m.inductionOn fun _ => Std.DHashMap.isEmpty_insertIfNew
+  isEmpty_eq_false_iff.mp <| m.inductionOn fun _ => DHashMap.isEmpty_insertIfNew
 
 @[simp]
 theorem contains_insertIfNew {k a : α} {v : β k} :
     (m.insertIfNew k v).contains a = (k == a || m.contains a) :=
-  m.inductionOn fun _ => Std.DHashMap.contains_insertIfNew
+  m.inductionOn fun _ => DHashMap.contains_insertIfNew
 
 @[simp]
 theorem mem_insertIfNew {k a : α} {v : β k} :
     a ∈ m.insertIfNew k v ↔ k == a ∨ a ∈ m :=
-  m.inductionOn fun _ => Std.DHashMap.mem_insertIfNew
+  m.inductionOn fun _ => DHashMap.mem_insertIfNew
 
 theorem contains_insertIfNew_self {k : α} {v : β k} :
     (m.insertIfNew k v).contains k :=
-  m.inductionOn fun _ => Std.DHashMap.contains_insertIfNew_self
+  m.inductionOn fun _ => DHashMap.contains_insertIfNew_self
 
 theorem mem_insertIfNew_self {k : α} {v : β k} :
     k ∈ m.insertIfNew k v :=
-  m.inductionOn fun _ => Std.DHashMap.mem_insertIfNew_self
+  m.inductionOn fun _ => DHashMap.mem_insertIfNew_self
 
 theorem contains_of_contains_insertIfNew {k a : α} {v : β k} :
     (m.insertIfNew k v).contains a → (k == a) = false → m.contains a :=
-  m.inductionOn fun _ => Std.DHashMap.contains_of_contains_insertIfNew
+  m.inductionOn fun _ => DHashMap.contains_of_contains_insertIfNew
 
 theorem mem_of_mem_insertIfNew {k a : α} {v : β k} :
     a ∈ m.insertIfNew k v → (k == a) = false → a ∈ m :=
-  m.inductionOn fun _ => Std.DHashMap.mem_of_mem_insertIfNew
+  m.inductionOn fun _ => DHashMap.mem_of_mem_insertIfNew
 
 /-- This is a restatement of `contains_of_contains_insertIfNew` that is written to exactly match the proof
 obligation in the statement of `get_insertIfNew`. -/
 theorem contains_of_contains_insertIfNew' {k a : α} {v : β k} :
     (m.insertIfNew k v).contains a → ¬((k == a) ∧ m.contains k = false) → m.contains a :=
-  m.inductionOn fun _ => Std.DHashMap.contains_of_contains_insertIfNew'
+  m.inductionOn fun _ => DHashMap.contains_of_contains_insertIfNew'
 
 /-- This is a restatement of `mem_of_mem_insertIfNew` that is written to exactly match the proof obligation
 in the statement of `get_insertIfNew`. -/
 theorem mem_of_mem_insertIfNew' {k a : α} {v : β k} :
     a ∈ m.insertIfNew k v → ¬((k == a) ∧ ¬k ∈ m) → a ∈ m :=
-  m.inductionOn fun _ => Std.DHashMap.mem_of_mem_insertIfNew'
+  m.inductionOn fun _ => DHashMap.mem_of_mem_insertIfNew'
 
 theorem size_insertIfNew {k : α} {v : β k} :
     (m.insertIfNew k v).size = if k ∈ m then m.size else m.size + 1 :=
-  m.inductionOn fun _ => Std.DHashMap.size_insertIfNew
+  m.inductionOn fun _ => DHashMap.size_insertIfNew
 
 theorem size_le_size_insertIfNew {k : α} {v : β k} :
     m.size ≤ (m.insertIfNew k v).size :=
-  m.inductionOn fun _ => Std.DHashMap.size_le_size_insertIfNew
+  m.inductionOn fun _ => DHashMap.size_le_size_insertIfNew
 
 theorem size_insertIfNew_le {k : α} {v : β k} :
     (m.insertIfNew k v).size ≤ m.size + 1 :=
-  m.inductionOn fun _ => Std.DHashMap.size_insertIfNew_le
+  m.inductionOn fun _ => DHashMap.size_insertIfNew_le
 
 theorem get?_insertIfNew [LawfulBEq α] {k a : α} {v : β k} : (m.insertIfNew k v).get? a =
     if h : k == a ∧ ¬k ∈ m then some (cast (congrArg β (eq_of_beq h.1)) v) else m.get? a :=
-  m.inductionOn fun _ => Std.DHashMap.get?_insertIfNew
+  m.inductionOn fun _ => DHashMap.get?_insertIfNew
 
 theorem get_insertIfNew [LawfulBEq α] {k a : α} {v : β k} {h₁} : (m.insertIfNew k v).get a h₁ =
     if h₂ : k == a ∧ ¬k ∈ m then cast (congrArg β (eq_of_beq h₂.1)) v else m.get a
       (mem_of_mem_insertIfNew' h₁ h₂) :=
-  m.inductionOn (fun _ _ => Std.DHashMap.get_insertIfNew) h₁
+  m.inductionOn (fun _ _ => DHashMap.get_insertIfNew) h₁
 
 theorem get!_insertIfNew [LawfulBEq α] {k a : α} [Inhabited (β a)] {v : β k} :
     (m.insertIfNew k v).get! a =
       if h : k == a ∧ ¬k ∈ m then cast (congrArg β (eq_of_beq h.1)) v else m.get! a :=
-  m.inductionOn fun _ => Std.DHashMap.get!_insertIfNew
+  m.inductionOn fun _ => DHashMap.get!_insertIfNew
 
 theorem getD_insertIfNew [LawfulBEq α] {k a : α} {fallback : β a} {v : β k} :
     (m.insertIfNew k v).getD a fallback =
       if h : k == a ∧ ¬k ∈ m then cast (congrArg β (eq_of_beq h.1)) v
       else m.getD a fallback :=
-  m.inductionOn fun _ => Std.DHashMap.getD_insertIfNew
+  m.inductionOn fun _ => DHashMap.getD_insertIfNew
 
 namespace Const
 
-variable {β : Type v} {m : DHashMap α (fun _ => β)}
+variable {β : Type v} {m : ExtDHashMap α (fun _ => β)}
 
 theorem get?_insertIfNew {k a : α} {v : β} :
     get? (m.insertIfNew k v) a = if k == a ∧ ¬k ∈ m then some v else get? m a :=
-  m.inductionOn fun _ => Std.DHashMap.Const.get?_insertIfNew
+  m.inductionOn fun _ => DHashMap.Const.get?_insertIfNew
 
 theorem get_insertIfNew {k a : α} {v : β} {h₁} :
     get (m.insertIfNew k v) a h₁ =
       if h₂ : k == a ∧ ¬k ∈ m then v else get m a (mem_of_mem_insertIfNew' h₁ h₂) :=
-  m.inductionOn (fun _ _ => Std.DHashMap.Const.get_insertIfNew) h₁
+  m.inductionOn (fun _ _ => DHashMap.Const.get_insertIfNew) h₁
 
 theorem get!_insertIfNew [Inhabited β] {k a : α} {v : β} :
     get! (m.insertIfNew k v) a = if k == a ∧ ¬k ∈ m then v else get! m a :=
-  m.inductionOn fun _ => Std.DHashMap.Const.get!_insertIfNew
+  m.inductionOn fun _ => DHashMap.Const.get!_insertIfNew
 
 theorem getD_insertIfNew {k a : α} {fallback v : β} :
     getD (m.insertIfNew k v) a fallback =
       if k == a ∧ ¬k ∈ m then v else getD m a fallback :=
-  m.inductionOn fun _ => Std.DHashMap.Const.getD_insertIfNew
+  m.inductionOn fun _ => DHashMap.Const.getD_insertIfNew
 
 end Const
 
 theorem getKey?_insertIfNew {k a : α} {v : β k} :
     getKey? (m.insertIfNew k v) a = if k == a ∧ ¬k ∈ m then some k else getKey? m a :=
-  m.inductionOn fun _ => Std.DHashMap.getKey?_insertIfNew
+  m.inductionOn fun _ => DHashMap.getKey?_insertIfNew
 
 theorem getKey_insertIfNew {k a : α} {v : β k} {h₁} :
     getKey (m.insertIfNew k v) a h₁ =
       if h₂ : k == a ∧ ¬k ∈ m then k else getKey m a (mem_of_mem_insertIfNew' h₁ h₂) :=
-  m.inductionOn (fun _ _ => Std.DHashMap.getKey_insertIfNew) h₁
+  m.inductionOn (fun _ _ => DHashMap.getKey_insertIfNew) h₁
 
 theorem getKey!_insertIfNew [Inhabited α] {k a : α} {v : β k} :
     getKey! (m.insertIfNew k v) a = if k == a ∧ ¬k ∈ m then k else getKey! m a :=
-  m.inductionOn fun _ => Std.DHashMap.getKey!_insertIfNew
+  m.inductionOn fun _ => DHashMap.getKey!_insertIfNew
 
 theorem getKeyD_insertIfNew {k a fallback : α} {v : β k} :
     getKeyD (m.insertIfNew k v) a fallback =
       if k == a ∧ ¬k ∈ m then k else getKeyD m a fallback :=
-  m.inductionOn fun _ => Std.DHashMap.getKeyD_insertIfNew
+  m.inductionOn fun _ => DHashMap.getKeyD_insertIfNew
 
 @[simp]
 theorem getThenInsertIfNew?_fst [LawfulBEq α] {k : α} {v : β k} :
     (m.getThenInsertIfNew? k v).1 = m.get? k :=
-  m.inductionOn fun _ => Std.DHashMap.getThenInsertIfNew?_fst
+  m.inductionOn fun _ => DHashMap.getThenInsertIfNew?_fst
 
 @[simp]
 theorem getThenInsertIfNew?_snd [LawfulBEq α] {k : α} {v : β k} :
     (m.getThenInsertIfNew? k v).2 = m.insertIfNew k v :=
-  m.inductionOn fun _ => congrArg Quotient.mk' Std.DHashMap.getThenInsertIfNew?_snd
+  m.inductionOn fun _ => congrArg Quotient.mk' DHashMap.getThenInsertIfNew?_snd
 
 namespace Const
 
-variable {β : Type v} {m : DHashMap α (fun _ => β)}
+variable {β : Type v} {m : ExtDHashMap α (fun _ => β)}
 
 @[simp]
 theorem getThenInsertIfNew?_fst {k : α} {v : β} : (getThenInsertIfNew? m k v).1 = get? m k :=
-  m.inductionOn fun _ => Std.DHashMap.Const.getThenInsertIfNew?_fst
+  m.inductionOn fun _ => DHashMap.Const.getThenInsertIfNew?_fst
 
 @[simp]
 theorem getThenInsertIfNew?_snd {k : α} {v : β} :
     (getThenInsertIfNew? m k v).2 = m.insertIfNew k v :=
-  m.inductionOn fun _ => congrArg Quotient.mk' Std.DHashMap.Const.getThenInsertIfNew?_snd
+  m.inductionOn fun _ => congrArg Quotient.mk' DHashMap.Const.getThenInsertIfNew?_snd
 
 end Const
 
@@ -927,18 +927,18 @@ theorem insertMany_cons {l : List ((a : α) × β a)} {p : (a : α) × β a} :
   exact (List.foldl_hom (f := Subtype.val) fun x y => rfl).symm
   exact (List.foldl_hom (f := Subtype.val) fun x y => rfl).symm
 
-private theorem insertMany_list_mk {m : Std.DHashMap α β} {l : List ((a : α) × β a)} :
-    (DHashMap.insertMany (Quotient.mk _ m) l : DHashMap α β) = Quotient.mk _ (m.insertMany l) := by
+private theorem insertMany_list_mk {m : DHashMap α β} {l : List ((a : α) × β a)} :
+    (ExtDHashMap.insertMany (Quotient.mk _ m) l : ExtDHashMap α β) = Quotient.mk _ (m.insertMany l) := by
   simp only [Quotient.mk]
   induction l generalizing m with
   | nil => rfl
   | cons x l ih =>
     rcases x with ⟨k, v⟩
-    simp only [insertMany_cons, Std.DHashMap.insertMany_cons, insert,
+    simp only [insertMany_cons, DHashMap.insertMany_cons, insert,
       Quotient.mk', Quotient.mk, Quotient.lift, ih]
 
 @[elab_as_elim]
-theorem insertMany_ind {motive : DHashMap α β → Prop} (m : DHashMap α β) (l : ρ)
+theorem insertMany_ind {motive : ExtDHashMap α β → Prop} (m : ExtDHashMap α β) (l : ρ)
     (init : motive m) (insert : ∀ m a b, motive m → motive (m.insert a b)) :
     motive (m.insertMany l) := by
   change motive (Subtype.val ?my_mvar)
@@ -950,7 +950,7 @@ theorem contains_insertMany_list
     (m.insertMany l).contains k = (m.contains k || (l.map Sigma.fst).contains k) := by
   refine m.inductionOn fun _ => ?_
   simp only [insertMany_list_mk]
-  exact Std.DHashMap.contains_insertMany_list
+  exact DHashMap.contains_insertMany_list
 
 @[simp]
 theorem mem_insertMany_list
@@ -958,7 +958,7 @@ theorem mem_insertMany_list
     k ∈ m.insertMany l ↔ k ∈ m ∨ (l.map Sigma.fst).contains k := by
   refine m.inductionOn fun _ => ?_
   simp only [insertMany_list_mk]
-  exact Std.DHashMap.mem_insertMany_list
+  exact DHashMap.mem_insertMany_list
 
 theorem mem_of_mem_insertMany_list
     {l : List ((a : α) × β a)} {k : α} (mem : k ∈ m.insertMany l)
@@ -966,7 +966,7 @@ theorem mem_of_mem_insertMany_list
     k ∈ m := by
   refine m.inductionOn (fun _ mem contains_eq_false => ?_) mem contains_eq_false
   simp only [insertMany_list_mk] at mem
-  exact Std.DHashMap.mem_of_mem_insertMany_list mem contains_eq_false
+  exact DHashMap.mem_of_mem_insertMany_list mem contains_eq_false
 
 theorem mem_insertMany_of_mem {l : ρ} {k : α} (h' : k ∈ m) : k ∈ m.insertMany l :=
   insertMany_ind m l h' fun _ _ _ h => mem_insert.mpr (.inr h)
@@ -977,7 +977,7 @@ theorem get?_insertMany_list_of_contains_eq_false [LawfulBEq α]
     (m.insertMany l).get? k = m.get? k := by
   refine m.inductionOn (fun _ contains_eq_false => ?_) contains_eq_false
   simp only [insertMany_list_mk]
-  exact Std.DHashMap.get?_insertMany_list_of_contains_eq_false contains_eq_false
+  exact DHashMap.get?_insertMany_list_of_contains_eq_false contains_eq_false
 
 theorem get?_insertMany_list_of_mem [LawfulBEq α]
     {l : List ((a : α) × β a)} {k k' : α} (k_beq : k == k') {v : β k}
@@ -986,7 +986,7 @@ theorem get?_insertMany_list_of_mem [LawfulBEq α]
     (m.insertMany l).get? k' = some (cast (by congr; apply LawfulBEq.eq_of_beq k_beq) v) := by
   refine m.inductionOn (fun _ k_beq distinct mem => ?_) k_beq distinct mem
   simp only [insertMany_list_mk]
-  exact Std.DHashMap.get?_insertMany_list_of_mem k_beq distinct mem
+  exact DHashMap.get?_insertMany_list_of_mem k_beq distinct mem
 
 theorem get_insertMany_list_of_contains_eq_false [LawfulBEq α]
     {l : List ((a : α) × β a)} {k : α}
@@ -996,7 +996,7 @@ theorem get_insertMany_list_of_contains_eq_false [LawfulBEq α]
       m.get k (mem_of_mem_insertMany_list h contains_eq_false) := by
   refine m.inductionOn (fun _ contains_eq_false _ => ?_) contains_eq_false h
   simp only [insertMany_list_mk]
-  exact Std.DHashMap.get_insertMany_list_of_contains_eq_false contains_eq_false
+  exact DHashMap.get_insertMany_list_of_contains_eq_false contains_eq_false
 
 theorem get_insertMany_list_of_mem [LawfulBEq α]
     {l : List ((a : α) × β a)} {k k' : α} (k_beq : k == k') {v : β k}
@@ -1006,7 +1006,7 @@ theorem get_insertMany_list_of_mem [LawfulBEq α]
     (m.insertMany l).get k' h = cast (by congr; apply LawfulBEq.eq_of_beq k_beq) v := by
   refine m.inductionOn (fun _ k_beq distinct mem _ => ?_) k_beq distinct mem h
   simp only [insertMany_list_mk]
-  exact Std.DHashMap.get_insertMany_list_of_mem k_beq distinct mem
+  exact DHashMap.get_insertMany_list_of_mem k_beq distinct mem
 
 theorem get!_insertMany_list_of_contains_eq_false [LawfulBEq α]
     {l : List ((a : α) × β a)} {k : α} [Inhabited (β k)]
@@ -1014,7 +1014,7 @@ theorem get!_insertMany_list_of_contains_eq_false [LawfulBEq α]
     (m.insertMany l).get! k = m.get! k := by
   refine m.inductionOn (fun _ contains_eq_false => ?_) contains_eq_false
   simp only [insertMany_list_mk]
-  exact Std.DHashMap.get!_insertMany_list_of_contains_eq_false contains_eq_false
+  exact DHashMap.get!_insertMany_list_of_contains_eq_false contains_eq_false
 
 theorem get!_insertMany_list_of_mem [LawfulBEq α]
     {l : List ((a : α) × β a)} {k k' : α} (k_beq : k == k') {v : β k} [Inhabited (β k')]
@@ -1023,7 +1023,7 @@ theorem get!_insertMany_list_of_mem [LawfulBEq α]
     (m.insertMany l).get! k' = cast (by congr; apply LawfulBEq.eq_of_beq k_beq) v := by
   refine m.inductionOn (fun _ k_beq distinct mem => ?_) k_beq distinct mem
   simp only [insertMany_list_mk]
-  exact Std.DHashMap.get!_insertMany_list_of_mem k_beq distinct mem
+  exact DHashMap.get!_insertMany_list_of_mem k_beq distinct mem
 
 theorem getD_insertMany_list_of_contains_eq_false [LawfulBEq α]
     {l : List ((a : α) × β a)} {k : α} {fallback : β k}
@@ -1031,7 +1031,7 @@ theorem getD_insertMany_list_of_contains_eq_false [LawfulBEq α]
     (m.insertMany l).getD k fallback = m.getD k fallback := by
   refine m.inductionOn (fun _ contains_eq_false => ?_) contains_eq_false
   simp only [insertMany_list_mk]
-  exact Std.DHashMap.getD_insertMany_list_of_contains_eq_false contains_eq_false
+  exact DHashMap.getD_insertMany_list_of_contains_eq_false contains_eq_false
 
 theorem getD_insertMany_list_of_mem [LawfulBEq α]
     {l : List ((a : α) × β a)} {k k' : α} (k_beq : k == k') {v : β k} {fallback : β k'}
@@ -1040,7 +1040,7 @@ theorem getD_insertMany_list_of_mem [LawfulBEq α]
     (m.insertMany l).getD k' fallback = cast (by congr; apply LawfulBEq.eq_of_beq k_beq) v := by
   refine m.inductionOn (fun _ k_beq distinct mem => ?_) k_beq distinct mem
   simp only [insertMany_list_mk]
-  exact Std.DHashMap.getD_insertMany_list_of_mem k_beq distinct mem
+  exact DHashMap.getD_insertMany_list_of_mem k_beq distinct mem
 
 theorem getKey?_insertMany_list_of_contains_eq_false
     {l : List ((a : α) × β a)} {k : α}
@@ -1048,7 +1048,7 @@ theorem getKey?_insertMany_list_of_contains_eq_false
     (m.insertMany l).getKey? k = m.getKey? k := by
   refine m.inductionOn (fun _ contains_eq_false => ?_) contains_eq_false
   simp only [insertMany_list_mk]
-  exact Std.DHashMap.getKey?_insertMany_list_of_contains_eq_false contains_eq_false
+  exact DHashMap.getKey?_insertMany_list_of_contains_eq_false contains_eq_false
 
 theorem getKey?_insertMany_list_of_mem
     {l : List ((a : α) × β a)}
@@ -1058,7 +1058,7 @@ theorem getKey?_insertMany_list_of_mem
     (m.insertMany l).getKey? k' = some k := by
   refine m.inductionOn (fun _ k_beq distinct mem => ?_) k_beq distinct mem
   simp only [insertMany_list_mk]
-  exact Std.DHashMap.getKey?_insertMany_list_of_mem k_beq distinct mem
+  exact DHashMap.getKey?_insertMany_list_of_mem k_beq distinct mem
 
 theorem getKey_insertMany_list_of_contains_eq_false
     {l : List ((a : α) × β a)} {k : α}
@@ -1068,7 +1068,7 @@ theorem getKey_insertMany_list_of_contains_eq_false
       m.getKey k (mem_of_mem_insertMany_list h contains_eq_false) := by
   refine m.inductionOn (fun _ contains_eq_false _ => ?_) contains_eq_false h
   simp only [insertMany_list_mk]
-  exact Std.DHashMap.getKey_insertMany_list_of_contains_eq_false contains_eq_false
+  exact DHashMap.getKey_insertMany_list_of_contains_eq_false contains_eq_false
 
 theorem getKey_insertMany_list_of_mem
     {l : List ((a : α) × β a)}
@@ -1079,7 +1079,7 @@ theorem getKey_insertMany_list_of_mem
     (m.insertMany l).getKey k' h = k := by
   refine m.inductionOn (fun _ k_beq distinct mem _ => ?_) k_beq distinct mem h
   simp only [insertMany_list_mk]
-  exact Std.DHashMap.getKey_insertMany_list_of_mem k_beq distinct mem
+  exact DHashMap.getKey_insertMany_list_of_mem k_beq distinct mem
 
 theorem getKey!_insertMany_list_of_contains_eq_false [Inhabited α]
     {l : List ((a : α) × β a)} {k : α}
@@ -1087,7 +1087,7 @@ theorem getKey!_insertMany_list_of_contains_eq_false [Inhabited α]
     (m.insertMany l).getKey! k = m.getKey! k := by
   refine m.inductionOn (fun _ contains_eq_false => ?_) contains_eq_false
   simp only [insertMany_list_mk]
-  exact Std.DHashMap.getKey!_insertMany_list_of_contains_eq_false contains_eq_false
+  exact DHashMap.getKey!_insertMany_list_of_contains_eq_false contains_eq_false
 
 theorem getKey!_insertMany_list_of_mem [Inhabited α]
     {l : List ((a : α) × β a)}
@@ -1097,7 +1097,7 @@ theorem getKey!_insertMany_list_of_mem [Inhabited α]
     (m.insertMany l).getKey! k' = k := by
   refine m.inductionOn (fun _ k_beq distinct mem => ?_) k_beq distinct mem
   simp only [insertMany_list_mk]
-  exact Std.DHashMap.getKey!_insertMany_list_of_mem k_beq distinct mem
+  exact DHashMap.getKey!_insertMany_list_of_mem k_beq distinct mem
 
 theorem getKeyD_insertMany_list_of_contains_eq_false
     {l : List ((a : α) × β a)} {k fallback : α}
@@ -1105,7 +1105,7 @@ theorem getKeyD_insertMany_list_of_contains_eq_false
     (m.insertMany l).getKeyD k fallback = m.getKeyD k fallback := by
   refine m.inductionOn (fun _ contains_eq_false => ?_) contains_eq_false
   simp only [insertMany_list_mk]
-  exact Std.DHashMap.getKeyD_insertMany_list_of_contains_eq_false contains_eq_false
+  exact DHashMap.getKeyD_insertMany_list_of_contains_eq_false contains_eq_false
 
 theorem getKeyD_insertMany_list_of_mem
     {l : List ((a : α) × β a)}
@@ -1115,7 +1115,7 @@ theorem getKeyD_insertMany_list_of_mem
     (m.insertMany l).getKeyD k' fallback = k := by
   refine m.inductionOn (fun _ k_beq distinct mem => ?_) k_beq distinct mem
   simp only [insertMany_list_mk]
-  exact Std.DHashMap.getKeyD_insertMany_list_of_mem k_beq distinct mem
+  exact DHashMap.getKeyD_insertMany_list_of_mem k_beq distinct mem
 
 theorem size_insertMany_list
     {l : List ((a : α) × β a)} (distinct : l.Pairwise (fun a b => (a.1 == b.1) = false)) :
@@ -1123,14 +1123,14 @@ theorem size_insertMany_list
       (m.insertMany l).size = m.size + l.length := by
   refine m.inductionOn (fun _ distinct => ?_) distinct
   simp only [insertMany_list_mk]
-  exact Std.DHashMap.size_insertMany_list distinct
+  exact DHashMap.size_insertMany_list distinct
 
 theorem size_le_size_insertMany_list
     {l : List ((a : α) × β a)} :
     m.size ≤ (m.insertMany l).size := by
   refine m.inductionOn fun _ => ?_
   simp only [insertMany_list_mk]
-  exact Std.DHashMap.size_le_size_insertMany_list
+  exact DHashMap.size_le_size_insertMany_list
 
 theorem size_le_size_insertMany {l : ρ} : m.size ≤ (m.insertMany l).size :=
   insertMany_ind m l (Nat.le_refl _) fun _ _ _ h => Nat.le_trans h size_le_size_insert
@@ -1140,7 +1140,7 @@ theorem size_insertMany_list_le
     (m.insertMany l).size ≤ m.size + l.length := by
   refine m.inductionOn fun _ => ?_
   simp only [insertMany_list_mk]
-  exact Std.DHashMap.size_insertMany_list_le
+  exact DHashMap.size_insertMany_list_le
 
 @[simp]
 theorem insertMany_list_eq_empty_iff {l : List ((a : α) × β a)} :
@@ -1148,7 +1148,7 @@ theorem insertMany_list_eq_empty_iff {l : List ((a : α) × β a)} :
   refine m.inductionOn fun _ => ?_
   simp only [insertMany_list_mk, ← isEmpty_iff, ← List.isEmpty_iff,
     Bool.coe_iff_coe, ← Bool.and_eq_true]
-  exact Std.DHashMap.isEmpty_insertMany_list
+  exact DHashMap.isEmpty_insertMany_list
 
 theorem eq_empty_of_insertMany_eq_empty {l : ρ} :
     m.insertMany l = ∅ → m = ∅ :=
@@ -1156,7 +1156,7 @@ theorem eq_empty_of_insertMany_eq_empty {l : ρ} :
 
 namespace Const
 
-variable {β : Type v} {m : DHashMap α (fun _ => β)}
+variable {β : Type v} {m : ExtDHashMap α (fun _ => β)}
 variable {ρ : Type w} [ForIn Id ρ (α × β)]
 
 @[simp]
@@ -1176,20 +1176,20 @@ theorem insertMany_cons {l : List (α × β)} {p : α × β} :
   exact (List.foldl_hom (f := Subtype.val) fun x y => rfl).symm
   exact (List.foldl_hom (f := Subtype.val) fun x y => rfl).symm
 
-private theorem insertMany_list_mk {m : Std.DHashMap α fun _ => β} {l : List (α × β)} :
-    (insertMany (Quotient.mk _ m) l : DHashMap α fun _ => β) =
-      Quotient.mk _ (Std.DHashMap.Const.insertMany m l) := by
+private theorem insertMany_list_mk {m : DHashMap α fun _ => β} {l : List (α × β)} :
+    (insertMany (Quotient.mk _ m) l : ExtDHashMap α fun _ => β) =
+      Quotient.mk _ (DHashMap.Const.insertMany m l) := by
   simp only [Quotient.mk]
   induction l generalizing m with
   | nil => rfl
   | cons x l ih =>
     rcases x with ⟨k, v⟩
-    simp only [insertMany_cons, Std.DHashMap.Const.insertMany_cons, insert,
+    simp only [insertMany_cons, DHashMap.Const.insertMany_cons, insert,
       Quotient.mk', Quotient.mk, Quotient.lift, ih]
 
 @[elab_as_elim]
-theorem insertMany_ind {motive : DHashMap α (fun _ => β) → Prop}
-    (m : DHashMap α fun _ => β) (l : ρ)
+theorem insertMany_ind {motive : ExtDHashMap α (fun _ => β) → Prop}
+    (m : ExtDHashMap α fun _ => β) (l : ρ)
     (init : motive m) (insert : ∀ m a b, motive m → motive (m.insert a b)) :
     motive (insertMany m l) := by
   change motive (Subtype.val ?my_mvar)
@@ -1201,7 +1201,7 @@ theorem contains_insertMany_list
     (Const.insertMany m l).contains k = (m.contains k || (l.map Prod.fst).contains k) := by
   refine m.inductionOn fun _ => ?_
   simp only [insertMany_list_mk]
-  exact Std.DHashMap.Const.contains_insertMany_list
+  exact DHashMap.Const.contains_insertMany_list
 
 @[simp]
 theorem mem_insertMany_list
@@ -1209,7 +1209,7 @@ theorem mem_insertMany_list
     k ∈ insertMany m l ↔ k ∈ m ∨ (l.map Prod.fst).contains k := by
   refine m.inductionOn fun _ => ?_
   simp only [insertMany_list_mk]
-  exact Std.DHashMap.Const.mem_insertMany_list
+  exact DHashMap.Const.mem_insertMany_list
 
 theorem mem_of_mem_insertMany_list
     {l : List (α × β)} {k : α} (mem : k ∈ insertMany m l)
@@ -1217,7 +1217,7 @@ theorem mem_of_mem_insertMany_list
     k ∈ m := by
   refine m.inductionOn (fun _ mem contains_eq_false => ?_) mem contains_eq_false
   simp only [insertMany_list_mk] at mem
-  exact Std.DHashMap.Const.mem_of_mem_insertMany_list mem contains_eq_false
+  exact DHashMap.Const.mem_of_mem_insertMany_list mem contains_eq_false
 
 theorem mem_insertMany_of_mem {l : ρ} {k : α} (h' : k ∈ m) : k ∈ insertMany m l :=
   insertMany_ind m l h' fun _ _ _ h => mem_insert.mpr (.inr h)
@@ -1228,7 +1228,7 @@ theorem getKey?_insertMany_list_of_contains_eq_false
     (insertMany m l).getKey? k = m.getKey? k := by
   refine m.inductionOn (fun _ contains_eq_false => ?_) contains_eq_false
   simp only [insertMany_list_mk]
-  exact Std.DHashMap.Const.getKey?_insertMany_list_of_contains_eq_false contains_eq_false
+  exact DHashMap.Const.getKey?_insertMany_list_of_contains_eq_false contains_eq_false
 
 theorem getKey?_insertMany_list_of_mem
     {l : List (α × β)}
@@ -1238,7 +1238,7 @@ theorem getKey?_insertMany_list_of_mem
     (insertMany m l).getKey? k' = some k := by
   refine m.inductionOn (fun _ k_beq distinct mem => ?_) k_beq distinct mem
   simp only [insertMany_list_mk]
-  exact Std.DHashMap.Const.getKey?_insertMany_list_of_mem k_beq distinct mem
+  exact DHashMap.Const.getKey?_insertMany_list_of_mem k_beq distinct mem
 
 theorem getKey_insertMany_list_of_contains_eq_false
     {l : List (α × β)} {k : α}
@@ -1248,7 +1248,7 @@ theorem getKey_insertMany_list_of_contains_eq_false
       m.getKey k (mem_of_mem_insertMany_list h contains_eq_false) := by
   refine m.inductionOn (fun _ contains_eq_false _ => ?_) contains_eq_false h
   simp only [insertMany_list_mk]
-  exact Std.DHashMap.Const.getKey_insertMany_list_of_contains_eq_false contains_eq_false
+  exact DHashMap.Const.getKey_insertMany_list_of_contains_eq_false contains_eq_false
 
 theorem getKey_insertMany_list_of_mem
     {l : List (α × β)}
@@ -1259,7 +1259,7 @@ theorem getKey_insertMany_list_of_mem
     (insertMany m l).getKey k' h = k := by
   refine m.inductionOn (fun _ k_beq distinct mem _ => ?_) k_beq distinct mem h
   simp only [insertMany_list_mk]
-  exact Std.DHashMap.Const.getKey_insertMany_list_of_mem k_beq distinct mem
+  exact DHashMap.Const.getKey_insertMany_list_of_mem k_beq distinct mem
 
 theorem getKey!_insertMany_list_of_contains_eq_false [Inhabited α]
     {l : List (α × β)} {k : α}
@@ -1267,7 +1267,7 @@ theorem getKey!_insertMany_list_of_contains_eq_false [Inhabited α]
     (insertMany m l).getKey! k = m.getKey! k := by
   refine m.inductionOn (fun _ contains_eq_false => ?_) contains_eq_false
   simp only [insertMany_list_mk]
-  exact Std.DHashMap.Const.getKey!_insertMany_list_of_contains_eq_false contains_eq_false
+  exact DHashMap.Const.getKey!_insertMany_list_of_contains_eq_false contains_eq_false
 
 theorem getKey!_insertMany_list_of_mem [Inhabited α]
     {l : List (α × β)}
@@ -1277,7 +1277,7 @@ theorem getKey!_insertMany_list_of_mem [Inhabited α]
     (insertMany m l).getKey! k' = k := by
   refine m.inductionOn (fun _ k_beq distinct mem => ?_) k_beq distinct mem
   simp only [insertMany_list_mk]
-  exact Std.DHashMap.Const.getKey!_insertMany_list_of_mem k_beq distinct mem
+  exact DHashMap.Const.getKey!_insertMany_list_of_mem k_beq distinct mem
 
 theorem getKeyD_insertMany_list_of_contains_eq_false
     {l : List (α × β)} {k fallback : α}
@@ -1285,7 +1285,7 @@ theorem getKeyD_insertMany_list_of_contains_eq_false
     (insertMany m l).getKeyD k fallback = m.getKeyD k fallback := by
   refine m.inductionOn (fun _ contains_eq_false => ?_) contains_eq_false
   simp only [insertMany_list_mk]
-  exact Std.DHashMap.Const.getKeyD_insertMany_list_of_contains_eq_false contains_eq_false
+  exact DHashMap.Const.getKeyD_insertMany_list_of_contains_eq_false contains_eq_false
 
 theorem getKeyD_insertMany_list_of_mem
     {l : List (α × β)}
@@ -1295,7 +1295,7 @@ theorem getKeyD_insertMany_list_of_mem
     (insertMany m l).getKeyD k' fallback = k := by
   refine m.inductionOn (fun _ k_beq distinct mem => ?_) k_beq distinct mem
   simp only [insertMany_list_mk]
-  exact Std.DHashMap.Const.getKeyD_insertMany_list_of_mem k_beq distinct mem
+  exact DHashMap.Const.getKeyD_insertMany_list_of_mem k_beq distinct mem
 
 theorem size_insertMany_list
     {l : List (α × β)}
@@ -1304,14 +1304,14 @@ theorem size_insertMany_list
       (insertMany m l).size = m.size + l.length := by
   refine m.inductionOn (fun _ distinct => ?_) distinct
   simp only [insertMany_list_mk]
-  exact Std.DHashMap.Const.size_insertMany_list distinct
+  exact DHashMap.Const.size_insertMany_list distinct
 
 theorem size_le_size_insertMany_list
     {l : List (α × β)} :
     m.size ≤ (insertMany m l).size := by
   refine m.inductionOn fun _ => ?_
   simp only [insertMany_list_mk]
-  exact Std.DHashMap.Const.size_le_size_insertMany_list
+  exact DHashMap.Const.size_le_size_insertMany_list
 
 theorem size_le_size_insertMany {l : ρ} : m.size ≤ (insertMany m l).size :=
   insertMany_ind m l (Nat.le_refl _) fun _ _ _ h => Nat.le_trans h size_le_size_insert
@@ -1321,7 +1321,7 @@ theorem size_insertMany_list_le
     (insertMany m l).size ≤ m.size + l.length := by
   refine m.inductionOn fun _ => ?_
   simp only [insertMany_list_mk]
-  exact Std.DHashMap.Const.size_insertMany_list_le
+  exact DHashMap.Const.size_insertMany_list_le
 
 @[simp]
 theorem insertMany_list_eq_empty_iff {l : List (α × β)} :
@@ -1329,7 +1329,7 @@ theorem insertMany_list_eq_empty_iff {l : List (α × β)} :
   refine m.inductionOn fun _ => ?_
   simp only [insertMany_list_mk, ← isEmpty_iff, ← List.isEmpty_iff,
     Bool.coe_iff_coe, ← Bool.and_eq_true]
-  exact Std.DHashMap.Const.isEmpty_insertMany_list
+  exact DHashMap.Const.isEmpty_insertMany_list
 
 theorem eq_empty_of_insertMany_eq_empty {l : ρ} : insertMany m l = ∅ → m = ∅ :=
   insertMany_ind m l id fun _ _ _ _ h => absurd h not_insert_eq_empty
@@ -1340,7 +1340,7 @@ theorem get?_insertMany_list_of_contains_eq_false
     get? (insertMany m l) k = get? m k := by
   refine m.inductionOn (fun _ contains_eq_false => ?_) contains_eq_false
   simp only [insertMany_list_mk]
-  exact Std.DHashMap.Const.get?_insertMany_list_of_contains_eq_false contains_eq_false
+  exact DHashMap.Const.get?_insertMany_list_of_contains_eq_false contains_eq_false
 
 theorem get?_insertMany_list_of_mem
     {l : List (α × β)} {k k' : α} (k_beq : k == k') {v : β}
@@ -1348,7 +1348,7 @@ theorem get?_insertMany_list_of_mem
     get? (insertMany m l) k' = v := by
   refine m.inductionOn (fun _ k_beq distinct mem => ?_) k_beq distinct mem
   simp only [insertMany_list_mk]
-  exact Std.DHashMap.Const.get?_insertMany_list_of_mem k_beq distinct mem
+  exact DHashMap.Const.get?_insertMany_list_of_mem k_beq distinct mem
 
 theorem get_insertMany_list_of_contains_eq_false
     {l : List (α × β)} {k : α}
@@ -1357,7 +1357,7 @@ theorem get_insertMany_list_of_contains_eq_false
     get (insertMany m l) k h = get m k (mem_of_mem_insertMany_list h contains_eq_false) := by
   refine m.inductionOn (fun _ contains_eq_false _ => ?_) contains_eq_false h
   simp only [insertMany_list_mk]
-  exact Std.DHashMap.Const.get_insertMany_list_of_contains_eq_false contains_eq_false
+  exact DHashMap.Const.get_insertMany_list_of_contains_eq_false contains_eq_false
 
 theorem get_insertMany_list_of_mem
     {l : List (α × β)} {k k' : α} (k_beq : k == k') {v : β}
@@ -1365,7 +1365,7 @@ theorem get_insertMany_list_of_mem
     get (insertMany m l) k' h = v := by
   refine m.inductionOn (fun _ k_beq distinct mem _ => ?_) k_beq distinct mem h
   simp only [insertMany_list_mk]
-  exact Std.DHashMap.Const.get_insertMany_list_of_mem k_beq distinct mem
+  exact DHashMap.Const.get_insertMany_list_of_mem k_beq distinct mem
 
 theorem get!_insertMany_list_of_contains_eq_false
     [Inhabited β] {l : List (α × β)} {k : α}
@@ -1373,7 +1373,7 @@ theorem get!_insertMany_list_of_contains_eq_false
     get! (insertMany m l) k = get! m k := by
   refine m.inductionOn (fun _ contains_eq_false => ?_) contains_eq_false
   simp only [insertMany_list_mk]
-  exact Std.DHashMap.Const.get!_insertMany_list_of_contains_eq_false contains_eq_false
+  exact DHashMap.Const.get!_insertMany_list_of_contains_eq_false contains_eq_false
 
 theorem get!_insertMany_list_of_mem [Inhabited β]
     {l : List (α × β)} {k k' : α} (k_beq : k == k') {v : β}
@@ -1381,7 +1381,7 @@ theorem get!_insertMany_list_of_mem [Inhabited β]
     get! (insertMany m l) k' = v := by
   refine m.inductionOn (fun _ k_beq distinct mem => ?_) k_beq distinct mem
   simp only [insertMany_list_mk]
-  exact Std.DHashMap.Const.get!_insertMany_list_of_mem k_beq distinct mem
+  exact DHashMap.Const.get!_insertMany_list_of_mem k_beq distinct mem
 
 theorem getD_insertMany_list_of_contains_eq_false
     {l : List (α × β)} {k : α} {fallback : β}
@@ -1389,7 +1389,7 @@ theorem getD_insertMany_list_of_contains_eq_false
     getD (insertMany m l) k fallback = getD m k fallback := by
   refine m.inductionOn (fun _ contains_eq_false => ?_) contains_eq_false
   simp only [insertMany_list_mk]
-  exact Std.DHashMap.Const.getD_insertMany_list_of_contains_eq_false contains_eq_false
+  exact DHashMap.Const.getD_insertMany_list_of_contains_eq_false contains_eq_false
 
 theorem getD_insertMany_list_of_mem
     {l : List (α × β)} {k k' : α} (k_beq : k == k') {v fallback : β}
@@ -1397,9 +1397,9 @@ theorem getD_insertMany_list_of_mem
     getD (insertMany m l) k' fallback = v := by
   refine m.inductionOn (fun _ k_beq distinct mem => ?_) k_beq distinct mem
   simp only [insertMany_list_mk]
-  exact Std.DHashMap.Const.getD_insertMany_list_of_mem k_beq distinct mem
+  exact DHashMap.Const.getD_insertMany_list_of_mem k_beq distinct mem
 
-variable {m : DHashMap α (fun _ => Unit)}
+variable {m : ExtDHashMap α (fun _ => Unit)}
 variable {ρ : Type w} [ForIn Id ρ α]
 
 @[simp]
@@ -1419,19 +1419,19 @@ theorem insertManyIfNewUnit_cons {l : List α} {k : α} :
   exact (List.foldl_hom (f := Subtype.val) fun x y => rfl).symm
   exact (List.foldl_hom (f := Subtype.val) fun x y => rfl).symm
 
-private theorem insertManyIfNewUnit_list_mk {m : Std.DHashMap α fun _ => Unit} {l : List α} :
-    (insertManyIfNewUnit (Quotient.mk _ m) l : DHashMap α fun _ => Unit) =
-      Quotient.mk _ (Std.DHashMap.Const.insertManyIfNewUnit m l) := by
+private theorem insertManyIfNewUnit_list_mk {m : DHashMap α fun _ => Unit} {l : List α} :
+    (insertManyIfNewUnit (Quotient.mk _ m) l : ExtDHashMap α fun _ => Unit) =
+      Quotient.mk _ (DHashMap.Const.insertManyIfNewUnit m l) := by
   simp only [Quotient.mk]
   induction l generalizing m with
   | nil => rfl
   | cons x l ih =>
-    simp only [insertManyIfNewUnit_cons, Std.DHashMap.Const.insertManyIfNewUnit_cons, insertIfNew,
+    simp only [insertManyIfNewUnit_cons, DHashMap.Const.insertManyIfNewUnit_cons, insertIfNew,
       Quotient.mk', Quotient.mk, Quotient.lift, ih]
 
 @[elab_as_elim]
-theorem insertManyIfNewUnit_ind {motive : DHashMap α (fun _ => Unit) → Prop}
-    (m : DHashMap α fun _ => Unit) (l : ρ)
+theorem insertManyIfNewUnit_ind {motive : ExtDHashMap α (fun _ => Unit) → Prop}
+    (m : ExtDHashMap α fun _ => Unit) (l : ρ)
     (init : motive m) (insert : ∀ m a, motive m → motive (m.insertIfNew a ())) :
     motive (insertManyIfNewUnit m l) := by
   change motive (Subtype.val ?my_mvar)
@@ -1443,7 +1443,7 @@ theorem contains_insertManyIfNewUnit_list
     (insertManyIfNewUnit m l).contains k = (m.contains k || l.contains k) := by
   refine m.inductionOn fun _ => ?_
   simp only [insertManyIfNewUnit_list_mk]
-  exact Std.DHashMap.Const.contains_insertManyIfNewUnit_list
+  exact DHashMap.Const.contains_insertManyIfNewUnit_list
 
 @[simp]
 theorem mem_insertManyIfNewUnit_list
@@ -1451,14 +1451,14 @@ theorem mem_insertManyIfNewUnit_list
     k ∈ insertManyIfNewUnit m l ↔ k ∈ m ∨ l.contains k := by
   refine m.inductionOn fun _ => ?_
   simp only [insertManyIfNewUnit_list_mk]
-  exact Std.DHashMap.Const.mem_insertManyIfNewUnit_list
+  exact DHashMap.Const.mem_insertManyIfNewUnit_list
 
 theorem mem_of_mem_insertManyIfNewUnit_list
     {l : List α} {k : α} (contains_eq_false : l.contains k = false) :
     k ∈ insertManyIfNewUnit m l → k ∈ m := by
   refine m.inductionOn (fun _ contains_eq_false => ?_) contains_eq_false
   simp only [insertManyIfNewUnit_list_mk]
-  exact Std.DHashMap.Const.mem_of_mem_insertManyIfNewUnit_list contains_eq_false
+  exact DHashMap.Const.mem_of_mem_insertManyIfNewUnit_list contains_eq_false
 
 theorem mem_insertManyIfNewUnit_of_mem {l : ρ} {k : α} (h : k ∈ m) :
     k ∈ insertManyIfNewUnit m l :=
@@ -1470,7 +1470,7 @@ theorem getKey?_insertManyIfNewUnit_list_of_not_mem_of_contains_eq_false
     getKey? (insertManyIfNewUnit m l) k = none := by
   refine m.inductionOn (fun _ not_mem contains_eq_false => ?_) not_mem contains_eq_false
   simp only [insertManyIfNewUnit_list_mk]
-  exact Std.DHashMap.Const.getKey?_insertManyIfNewUnit_list_of_not_mem_of_contains_eq_false not_mem contains_eq_false
+  exact DHashMap.Const.getKey?_insertManyIfNewUnit_list_of_not_mem_of_contains_eq_false not_mem contains_eq_false
 
 theorem getKey?_insertManyIfNewUnit_list_of_not_mem_of_mem
     {l : List α} {k k' : α} (k_beq : k == k')
@@ -1479,14 +1479,14 @@ theorem getKey?_insertManyIfNewUnit_list_of_not_mem_of_mem
     getKey? (insertManyIfNewUnit m l) k' = some k := by
   refine m.inductionOn (fun _ k_beq not_mem distinct mem => ?_) k_beq not_mem distinct mem
   simp only [insertManyIfNewUnit_list_mk]
-  exact Std.DHashMap.Const.getKey?_insertManyIfNewUnit_list_of_not_mem_of_mem k_beq not_mem distinct mem
+  exact DHashMap.Const.getKey?_insertManyIfNewUnit_list_of_not_mem_of_mem k_beq not_mem distinct mem
 
 theorem getKey?_insertManyIfNewUnit_list_of_mem
     {l : List α} {k : α} (h' : k ∈ m) :
     getKey? (insertManyIfNewUnit m l) k = getKey? m k := by
   refine m.inductionOn (fun _ h' => ?_) h'
   simp only [insertManyIfNewUnit_list_mk]
-  exact Std.DHashMap.Const.getKey?_insertManyIfNewUnit_list_of_mem h'
+  exact DHashMap.Const.getKey?_insertManyIfNewUnit_list_of_mem h'
 
 theorem getKey_insertManyIfNewUnit_list_of_not_mem_of_mem
     {l : List α}
@@ -1496,14 +1496,14 @@ theorem getKey_insertManyIfNewUnit_list_of_not_mem_of_mem
     getKey (insertManyIfNewUnit m l) k' h = k := by
   refine m.inductionOn (fun _ k_beq not_mem distinct mem _ => ?_) k_beq not_mem distinct mem h
   simp only [insertManyIfNewUnit_list_mk]
-  exact Std.DHashMap.Const.getKey_insertManyIfNewUnit_list_of_not_mem_of_mem k_beq not_mem distinct mem
+  exact DHashMap.Const.getKey_insertManyIfNewUnit_list_of_not_mem_of_mem k_beq not_mem distinct mem
 
 theorem getKey_insertManyIfNewUnit_list_of_mem
     {l : List α} {k : α} (mem : k ∈ m) {h} :
     getKey (insertManyIfNewUnit m l) k h = getKey m k mem := by
   refine m.inductionOn (fun _ mem _ => ?_) mem h
   simp only [insertManyIfNewUnit_list_mk]
-  exact Std.DHashMap.Const.getKey_insertManyIfNewUnit_list_of_mem mem
+  exact DHashMap.Const.getKey_insertManyIfNewUnit_list_of_mem mem
 
 theorem getKey!_insertManyIfNewUnit_list_of_not_mem_of_contains_eq_false
     [Inhabited α] {l : List α} {k : α}
@@ -1511,7 +1511,7 @@ theorem getKey!_insertManyIfNewUnit_list_of_not_mem_of_contains_eq_false
     getKey! (insertManyIfNewUnit m l) k = default := by
   refine m.inductionOn (fun _ not_mem contains_eq_false => ?_) not_mem contains_eq_false
   simp only [insertManyIfNewUnit_list_mk]
-  exact Std.DHashMap.Const.getKey!_insertManyIfNewUnit_list_of_not_mem_of_contains_eq_false not_mem contains_eq_false
+  exact DHashMap.Const.getKey!_insertManyIfNewUnit_list_of_not_mem_of_contains_eq_false not_mem contains_eq_false
 
 theorem getKey!_insertManyIfNewUnit_list_of_not_mem_of_mem
     [Inhabited α] {l : List α} {k k' : α} (k_beq : k == k')
@@ -1520,14 +1520,14 @@ theorem getKey!_insertManyIfNewUnit_list_of_not_mem_of_mem
     getKey! (insertManyIfNewUnit m l) k' = k := by
   refine m.inductionOn (fun _ k_beq not_mem distinct mem => ?_) k_beq not_mem distinct mem
   simp only [insertManyIfNewUnit_list_mk]
-  exact Std.DHashMap.Const.getKey!_insertManyIfNewUnit_list_of_not_mem_of_mem k_beq not_mem distinct mem
+  exact DHashMap.Const.getKey!_insertManyIfNewUnit_list_of_not_mem_of_mem k_beq not_mem distinct mem
 
 theorem getKey!_insertManyIfNewUnit_list_of_mem
     [Inhabited α] {l : List α} {k : α} (mem : k ∈ m) :
     getKey! (insertManyIfNewUnit m l) k = getKey! m k := by
   refine m.inductionOn (fun _ mem => ?_) mem
   simp only [insertManyIfNewUnit_list_mk]
-  exact Std.DHashMap.Const.getKey!_insertManyIfNewUnit_list_of_mem mem
+  exact DHashMap.Const.getKey!_insertManyIfNewUnit_list_of_mem mem
 
 theorem getKeyD_insertManyIfNewUnit_list_of_not_mem_of_contains_eq_false
     {l : List α} {k fallback : α}
@@ -1535,7 +1535,7 @@ theorem getKeyD_insertManyIfNewUnit_list_of_not_mem_of_contains_eq_false
     getKeyD (insertManyIfNewUnit m l) k fallback = fallback := by
   refine m.inductionOn (fun _ not_mem contains_eq_false => ?_) not_mem contains_eq_false
   simp only [insertManyIfNewUnit_list_mk]
-  exact Std.DHashMap.Const.getKeyD_insertManyIfNewUnit_list_of_not_mem_of_contains_eq_false not_mem contains_eq_false
+  exact DHashMap.Const.getKeyD_insertManyIfNewUnit_list_of_not_mem_of_contains_eq_false not_mem contains_eq_false
 
 theorem getKeyD_insertManyIfNewUnit_list_of_not_mem_of_mem
     {l : List α} {k k' fallback : α} (k_beq : k == k')
@@ -1544,14 +1544,14 @@ theorem getKeyD_insertManyIfNewUnit_list_of_not_mem_of_mem
     getKeyD (insertManyIfNewUnit m l) k' fallback = k := by
   refine m.inductionOn (fun _ k_beq not_mem distinct mem => ?_) k_beq not_mem distinct mem
   simp only [insertManyIfNewUnit_list_mk]
-  exact Std.DHashMap.Const.getKeyD_insertManyIfNewUnit_list_of_not_mem_of_mem k_beq not_mem distinct mem
+  exact DHashMap.Const.getKeyD_insertManyIfNewUnit_list_of_not_mem_of_mem k_beq not_mem distinct mem
 
 theorem getKeyD_insertManyIfNewUnit_list_of_mem
     {l : List α} {k fallback : α} (mem : k ∈ m) :
     getKeyD (insertManyIfNewUnit m l) k fallback = getKeyD m k fallback := by
   refine m.inductionOn (fun _ mem => ?_) mem
   simp only [insertManyIfNewUnit_list_mk]
-  exact Std.DHashMap.Const.getKeyD_insertManyIfNewUnit_list_of_mem mem
+  exact DHashMap.Const.getKeyD_insertManyIfNewUnit_list_of_mem mem
 
 theorem size_insertManyIfNewUnit_list
     {l : List α}
@@ -1560,14 +1560,14 @@ theorem size_insertManyIfNewUnit_list
       (insertManyIfNewUnit m l).size = m.size + l.length := by
   refine m.inductionOn (fun _ distinct => ?_) distinct
   simp only [insertManyIfNewUnit_list_mk]
-  exact Std.DHashMap.Const.size_insertManyIfNewUnit_list distinct
+  exact DHashMap.Const.size_insertManyIfNewUnit_list distinct
 
 theorem size_le_size_insertManyIfNewUnit_list
     {l : List α} :
     m.size ≤ (insertManyIfNewUnit m l).size := by
   refine m.inductionOn fun _ => ?_
   simp only [insertManyIfNewUnit_list_mk]
-  exact Std.DHashMap.Const.size_le_size_insertManyIfNewUnit_list
+  exact DHashMap.Const.size_le_size_insertManyIfNewUnit_list
 
 theorem size_le_size_insertManyIfNewUnit
     {l : ρ} : m.size ≤ (insertManyIfNewUnit m l).size :=
@@ -1578,7 +1578,7 @@ theorem size_insertManyIfNewUnit_list_le
     (insertManyIfNewUnit m l).size ≤ m.size + l.length := by
   refine m.inductionOn fun _ => ?_
   simp only [insertManyIfNewUnit_list_mk]
-  exact Std.DHashMap.Const.size_insertManyIfNewUnit_list_le
+  exact DHashMap.Const.size_insertManyIfNewUnit_list_le
 
 @[simp]
 theorem insertManyIfNewUnit_list_eq_empty_iff {l : List α} :
@@ -1586,7 +1586,7 @@ theorem insertManyIfNewUnit_list_eq_empty_iff {l : List α} :
   refine m.inductionOn fun _ => ?_
   simp only [insertManyIfNewUnit_list_mk, ← isEmpty_iff, ← List.isEmpty_iff,
     Bool.coe_iff_coe, ← Bool.and_eq_true]
-  exact Std.DHashMap.Const.isEmpty_insertManyIfNewUnit_list
+  exact DHashMap.Const.isEmpty_insertManyIfNewUnit_list
 
 theorem eq_empty_of_insertManyIfNewUnit_eq_empty {l : ρ} :
     insertManyIfNewUnit m l = ∅ → m = ∅ :=
@@ -1598,7 +1598,7 @@ theorem get?_insertManyIfNewUnit_list
       if k ∈ m ∨ l.contains k then some () else none := by
   refine m.inductionOn fun _ => ?_
   simp only [insertManyIfNewUnit_list_mk]
-  exact Std.DHashMap.Const.get?_insertManyIfNewUnit_list
+  exact DHashMap.Const.get?_insertManyIfNewUnit_list
 
 theorem get_insertManyIfNewUnit_list
     {l : List α} {k : α} {h} :
@@ -1619,9 +1619,9 @@ end Const
 
 end insertMany
 
-end DHashMap
+end ExtDHashMap
 
-namespace DHashMap
+namespace ExtDHashMap
 
 @[simp]
 theorem ofList_nil :
@@ -1629,14 +1629,14 @@ theorem ofList_nil :
 
 @[simp]
 theorem ofList_singleton {k : α} {v : β k} :
-    ofList [⟨k, v⟩] = (∅ : DHashMap α β).insert k v := rfl
+    ofList [⟨k, v⟩] = (∅ : ExtDHashMap α β).insert k v := rfl
 
 theorem ofList_cons {k : α} {v : β k} {tl : List ((a : α) × β a)} :
-    ofList (⟨k, v⟩ :: tl) = ((∅ : DHashMap α β).insert k v).insertMany tl :=
+    ofList (⟨k, v⟩ :: tl) = ((∅ : ExtDHashMap α β).insert k v).insertMany tl :=
   insertMany_cons
 
 private theorem ofList_eq_mk {l : List ((a : α) × β a)} :
-    (ofList l : DHashMap α β) = Quotient.mk _ (Std.DHashMap.ofList l) := by
+    (ofList l : ExtDHashMap α β) = Quotient.mk _ (DHashMap.ofList l) := by
   change insertMany (Quotient.mk _ _) _ = _
   rw [insertMany_list_mk]
   rfl
@@ -1646,21 +1646,21 @@ theorem contains_ofList
     {l : List ((a : α) × β a)} {k : α} :
     (ofList l).contains k = (l.map Sigma.fst).contains k := by
   simp only [ofList_eq_mk]
-  exact Std.DHashMap.contains_ofList
+  exact DHashMap.contains_ofList
 
 @[simp]
 theorem mem_ofList
     {l : List ((a : α) × β a)} {k : α} :
     k ∈ ofList l ↔ (l.map Sigma.fst).contains k := by
   simp only [ofList_eq_mk]
-  exact Std.DHashMap.mem_ofList
+  exact DHashMap.mem_ofList
 
 theorem get?_ofList_of_contains_eq_false [LawfulBEq α]
     {l : List ((a : α) × β a)} {k : α}
     (contains_eq_false : (l.map Sigma.fst).contains k = false) :
     (ofList l).get? k = none := by
   simp only [ofList_eq_mk]
-  exact Std.DHashMap.get?_ofList_of_contains_eq_false contains_eq_false
+  exact DHashMap.get?_ofList_of_contains_eq_false contains_eq_false
 
 theorem get?_ofList_of_mem [LawfulBEq α]
     {l : List ((a : α) × β a)} {k k' : α} (k_beq : k == k') {v : β k}
@@ -1668,7 +1668,7 @@ theorem get?_ofList_of_mem [LawfulBEq α]
     (mem : ⟨k, v⟩ ∈ l) :
     (ofList l).get? k' = some (cast (by congr; apply LawfulBEq.eq_of_beq k_beq) v) := by
   simp only [ofList_eq_mk]
-  exact Std.DHashMap.get?_ofList_of_mem k_beq distinct mem
+  exact DHashMap.get?_ofList_of_mem k_beq distinct mem
 
 theorem get_ofList_of_mem [LawfulBEq α]
     {l : List ((a : α) × β a)} {k k' : α} (k_beq : k == k') {v : β k}
@@ -1677,14 +1677,14 @@ theorem get_ofList_of_mem [LawfulBEq α]
     {h} :
     (ofList l).get k' h = cast (by congr; apply LawfulBEq.eq_of_beq k_beq) v := by
   simp only [ofList_eq_mk]
-  exact Std.DHashMap.get_ofList_of_mem k_beq distinct mem
+  exact DHashMap.get_ofList_of_mem k_beq distinct mem
 
 theorem get!_ofList_of_contains_eq_false [LawfulBEq α]
     {l : List ((a : α) × β a)} {k : α} [Inhabited (β k)]
     (contains_eq_false : (l.map Sigma.fst).contains k = false) :
     (ofList l).get! k = default := by
   simp only [ofList_eq_mk]
-  exact Std.DHashMap.get!_ofList_of_contains_eq_false contains_eq_false
+  exact DHashMap.get!_ofList_of_contains_eq_false contains_eq_false
 
 theorem get!_ofList_of_mem [LawfulBEq α]
     {l : List ((a : α) × β a)} {k k' : α} (k_beq : k == k') {v : β k} [Inhabited (β k')]
@@ -1692,14 +1692,14 @@ theorem get!_ofList_of_mem [LawfulBEq α]
     (mem : ⟨k, v⟩ ∈ l) :
     (ofList l).get! k' = cast (by congr; apply LawfulBEq.eq_of_beq k_beq) v := by
   simp only [ofList_eq_mk]
-  exact Std.DHashMap.get!_ofList_of_mem k_beq distinct mem
+  exact DHashMap.get!_ofList_of_mem k_beq distinct mem
 
 theorem getD_ofList_of_contains_eq_false [LawfulBEq α]
     {l : List ((a : α) × β a)} {k : α} {fallback : β k}
     (contains_eq_false : (l.map Sigma.fst).contains k = false) :
     (ofList l).getD k fallback = fallback := by
   simp only [ofList_eq_mk]
-  exact Std.DHashMap.getD_ofList_of_contains_eq_false contains_eq_false
+  exact DHashMap.getD_ofList_of_contains_eq_false contains_eq_false
 
 theorem getD_ofList_of_mem [LawfulBEq α]
     {l : List ((a : α) × β a)} {k k' : α} (k_beq : k == k') {v : β k} {fallback : β k'}
@@ -1707,14 +1707,14 @@ theorem getD_ofList_of_mem [LawfulBEq α]
     (mem : ⟨k, v⟩ ∈ l) :
     (ofList l).getD k' fallback = cast (by congr; apply LawfulBEq.eq_of_beq k_beq) v := by
   simp only [ofList_eq_mk]
-  exact Std.DHashMap.getD_ofList_of_mem k_beq distinct mem
+  exact DHashMap.getD_ofList_of_mem k_beq distinct mem
 
 theorem getKey?_ofList_of_contains_eq_false
     {l : List ((a : α) × β a)} {k : α}
     (contains_eq_false : (l.map Sigma.fst).contains k = false) :
     (ofList l).getKey? k = none := by
   simp only [ofList_eq_mk]
-  exact Std.DHashMap.getKey?_ofList_of_contains_eq_false contains_eq_false
+  exact DHashMap.getKey?_ofList_of_contains_eq_false contains_eq_false
 
 theorem getKey?_ofList_of_mem
     {l : List ((a : α) × β a)}
@@ -1723,7 +1723,7 @@ theorem getKey?_ofList_of_mem
     (mem : k ∈ l.map Sigma.fst) :
     (ofList l).getKey? k' = some k := by
   simp only [ofList_eq_mk]
-  exact Std.DHashMap.getKey?_ofList_of_mem k_beq distinct mem
+  exact DHashMap.getKey?_ofList_of_mem k_beq distinct mem
 
 theorem getKey_ofList_of_mem
     {l : List ((a : α) × β a)}
@@ -1733,14 +1733,14 @@ theorem getKey_ofList_of_mem
     {h} :
     (ofList l).getKey k' h = k := by
   simp only [ofList_eq_mk]
-  exact Std.DHashMap.getKey_ofList_of_mem k_beq distinct mem
+  exact DHashMap.getKey_ofList_of_mem k_beq distinct mem
 
 theorem getKey!_ofList_of_contains_eq_false [Inhabited α]
     {l : List ((a : α) × β a)} {k : α}
     (contains_eq_false : (l.map Sigma.fst).contains k = false) :
     (ofList l).getKey! k = default := by
   simp only [ofList_eq_mk]
-  exact Std.DHashMap.getKey!_ofList_of_contains_eq_false contains_eq_false
+  exact DHashMap.getKey!_ofList_of_contains_eq_false contains_eq_false
 
 theorem getKey!_ofList_of_mem [Inhabited α]
     {l : List ((a : α) × β a)}
@@ -1749,14 +1749,14 @@ theorem getKey!_ofList_of_mem [Inhabited α]
     (mem : k ∈ l.map Sigma.fst) :
     (ofList l).getKey! k' = k := by
   simp only [ofList_eq_mk]
-  exact Std.DHashMap.getKey!_ofList_of_mem k_beq distinct mem
+  exact DHashMap.getKey!_ofList_of_mem k_beq distinct mem
 
 theorem getKeyD_ofList_of_contains_eq_false
     {l : List ((a : α) × β a)} {k fallback : α}
     (contains_eq_false : (l.map Sigma.fst).contains k = false) :
     (ofList l).getKeyD k fallback = fallback := by
   simp only [ofList_eq_mk]
-  exact Std.DHashMap.getKeyD_ofList_of_contains_eq_false contains_eq_false
+  exact DHashMap.getKeyD_ofList_of_contains_eq_false contains_eq_false
 
 theorem getKeyD_ofList_of_mem
     {l : List ((a : α) × β a)}
@@ -1765,25 +1765,25 @@ theorem getKeyD_ofList_of_mem
     (mem : k ∈ l.map Sigma.fst) :
     (ofList l).getKeyD k' fallback = k := by
   simp only [ofList_eq_mk]
-  exact Std.DHashMap.getKeyD_ofList_of_mem k_beq distinct mem
+  exact DHashMap.getKeyD_ofList_of_mem k_beq distinct mem
 
 theorem size_ofList
     {l : List ((a : α) × β a)} (distinct : l.Pairwise (fun a b => (a.1 == b.1) = false)) :
     (ofList l).size = l.length := by
   simp only [ofList_eq_mk]
-  exact Std.DHashMap.size_ofList distinct
+  exact DHashMap.size_ofList distinct
 
 theorem size_ofList_le
     {l : List ((a : α) × β a)} :
     (ofList l).size ≤ l.length := by
   simp only [ofList_eq_mk]
-  exact Std.DHashMap.size_ofList_le
+  exact DHashMap.size_ofList_le
 
 @[simp]
 theorem ofList_eq_empty_iff {l : List ((a : α) × β a)} :
     ofList l = ∅ ↔ l = [] := by
   simp only [ofList_eq_mk, ← isEmpty_iff, ← List.isEmpty_iff, Bool.coe_iff_coe]
-  exact Std.DHashMap.isEmpty_ofList
+  exact DHashMap.isEmpty_ofList
 
 namespace Const
 
@@ -1796,15 +1796,15 @@ theorem ofList_nil :
 
 @[simp]
 theorem ofList_singleton {k : α} {v : β} :
-    ofList [⟨k, v⟩] = (∅ : DHashMap α (fun _ => β)).insert k v :=
+    ofList [⟨k, v⟩] = (∅ : ExtDHashMap α (fun _ => β)).insert k v :=
   rfl
 
 theorem ofList_cons {k : α} {v : β} {tl : List (α × β)} :
-    ofList (⟨k, v⟩ :: tl) = insertMany ((∅ : DHashMap α (fun _ => β)).insert k v) tl :=
+    ofList (⟨k, v⟩ :: tl) = insertMany ((∅ : ExtDHashMap α (fun _ => β)).insert k v) tl :=
   insertMany_cons
 
 private theorem ofList_eq_mk {l : List (α × β)} :
-    (ofList l : DHashMap α fun _ => β) = Quotient.mk _ (Std.DHashMap.Const.ofList l) := by
+    (ofList l : ExtDHashMap α fun _ => β) = Quotient.mk _ (DHashMap.Const.ofList l) := by
   change insertMany (Quotient.mk _ _) _ = _
   rw [insertMany_list_mk]
   rfl
@@ -1814,21 +1814,21 @@ theorem contains_ofList
     {l : List (α × β)} {k : α} :
     (ofList l).contains k = (l.map Prod.fst).contains k := by
   simp only [ofList_eq_mk]
-  exact Std.DHashMap.Const.contains_ofList
+  exact DHashMap.Const.contains_ofList
 
 @[simp]
 theorem mem_ofList
     {l : List (α × β)} {k : α} :
     k ∈ ofList l ↔ (l.map Prod.fst).contains k := by
   simp only [ofList_eq_mk]
-  exact Std.DHashMap.Const.mem_ofList
+  exact DHashMap.Const.mem_ofList
 
 theorem get?_ofList_of_contains_eq_false
     {l : List (α × β)} {k : α}
     (contains_eq_false : (l.map Prod.fst).contains k = false) :
     get? (ofList l) k = none := by
   simp only [ofList_eq_mk]
-  exact Std.DHashMap.Const.get?_ofList_of_contains_eq_false contains_eq_false
+  exact DHashMap.Const.get?_ofList_of_contains_eq_false contains_eq_false
 
 theorem get?_ofList_of_mem
     {l : List (α × β)} {k k' : α} (k_beq : k == k') {v : β}
@@ -1836,7 +1836,7 @@ theorem get?_ofList_of_mem
     (mem : ⟨k, v⟩ ∈ l) :
     get? (ofList l) k' = some v := by
   simp only [ofList_eq_mk]
-  exact Std.DHashMap.Const.get?_ofList_of_mem k_beq distinct mem
+  exact DHashMap.Const.get?_ofList_of_mem k_beq distinct mem
 
 theorem get_ofList_of_mem
     {l : List (α × β)} {k k' : α} (k_beq : k == k') {v : β}
@@ -1845,14 +1845,14 @@ theorem get_ofList_of_mem
     {h} :
     get (ofList l) k' h = v := by
   simp only [ofList_eq_mk]
-  exact Std.DHashMap.Const.get_ofList_of_mem k_beq distinct mem
+  exact DHashMap.Const.get_ofList_of_mem k_beq distinct mem
 
 theorem get!_ofList_of_contains_eq_false
     {l : List (α × β)} {k : α} [Inhabited β]
     (contains_eq_false : (l.map Prod.fst).contains k = false) :
     get! (ofList l) k = (default : β) := by
   simp only [ofList_eq_mk]
-  exact Std.DHashMap.Const.get!_ofList_of_contains_eq_false contains_eq_false
+  exact DHashMap.Const.get!_ofList_of_contains_eq_false contains_eq_false
 
 theorem get!_ofList_of_mem
     {l : List (α × β)} {k k' : α} (k_beq : k == k') {v : β} [Inhabited β]
@@ -1860,14 +1860,14 @@ theorem get!_ofList_of_mem
     (mem : ⟨k, v⟩ ∈ l) :
     get! (ofList l) k' = v := by
   simp only [ofList_eq_mk]
-  exact Std.DHashMap.Const.get!_ofList_of_mem k_beq distinct mem
+  exact DHashMap.Const.get!_ofList_of_mem k_beq distinct mem
 
 theorem getD_ofList_of_contains_eq_false
     {l : List (α × β)} {k : α} {fallback : β}
     (contains_eq_false : (l.map Prod.fst).contains k = false) :
     getD (ofList l) k fallback = fallback := by
   simp only [ofList_eq_mk]
-  exact Std.DHashMap.Const.getD_ofList_of_contains_eq_false contains_eq_false
+  exact DHashMap.Const.getD_ofList_of_contains_eq_false contains_eq_false
 
 theorem getD_ofList_of_mem
     {l : List (α × β)} {k k' : α} (k_beq : k == k') {v : β} {fallback : β}
@@ -1875,14 +1875,14 @@ theorem getD_ofList_of_mem
     (mem : ⟨k, v⟩ ∈ l) :
     getD (ofList l) k' fallback = v := by
   simp only [ofList_eq_mk]
-  exact Std.DHashMap.Const.getD_ofList_of_mem k_beq distinct mem
+  exact DHashMap.Const.getD_ofList_of_mem k_beq distinct mem
 
 theorem getKey?_ofList_of_contains_eq_false
     {l : List (α × β)} {k : α}
     (contains_eq_false : (l.map Prod.fst).contains k = false) :
     (ofList l).getKey? k = none := by
   simp only [ofList_eq_mk]
-  exact Std.DHashMap.Const.getKey?_ofList_of_contains_eq_false contains_eq_false
+  exact DHashMap.Const.getKey?_ofList_of_contains_eq_false contains_eq_false
 
 theorem getKey?_ofList_of_mem
     {l : List (α × β)}
@@ -1891,7 +1891,7 @@ theorem getKey?_ofList_of_mem
     (mem : k ∈ l.map Prod.fst) :
     (ofList l).getKey? k' = some k := by
   simp only [ofList_eq_mk]
-  exact Std.DHashMap.Const.getKey?_ofList_of_mem k_beq distinct mem
+  exact DHashMap.Const.getKey?_ofList_of_mem k_beq distinct mem
 
 theorem getKey_ofList_of_mem
     {l : List (α × β)}
@@ -1901,14 +1901,14 @@ theorem getKey_ofList_of_mem
     {h} :
     (ofList l).getKey k' h = k := by
   simp only [ofList_eq_mk]
-  exact Std.DHashMap.Const.getKey_ofList_of_mem k_beq distinct mem
+  exact DHashMap.Const.getKey_ofList_of_mem k_beq distinct mem
 
 theorem getKey!_ofList_of_contains_eq_false
     [Inhabited α] {l : List (α × β)} {k : α}
     (contains_eq_false : (l.map Prod.fst).contains k = false) :
     (ofList l).getKey! k = default := by
   simp only [ofList_eq_mk]
-  exact Std.DHashMap.Const.getKey!_ofList_of_contains_eq_false contains_eq_false
+  exact DHashMap.Const.getKey!_ofList_of_contains_eq_false contains_eq_false
 
 theorem getKey!_ofList_of_mem [Inhabited α]
     {l : List (α × β)}
@@ -1917,14 +1917,14 @@ theorem getKey!_ofList_of_mem [Inhabited α]
     (mem : k ∈ l.map Prod.fst) :
     (ofList l).getKey! k' = k := by
   simp only [ofList_eq_mk]
-  exact Std.DHashMap.Const.getKey!_ofList_of_mem k_beq distinct mem
+  exact DHashMap.Const.getKey!_ofList_of_mem k_beq distinct mem
 
 theorem getKeyD_ofList_of_contains_eq_false
     {l : List (α × β)} {k fallback : α}
     (contains_eq_false : (l.map Prod.fst).contains k = false) :
     (ofList l).getKeyD k fallback = fallback := by
   simp only [ofList_eq_mk]
-  exact Std.DHashMap.Const.getKeyD_ofList_of_contains_eq_false contains_eq_false
+  exact DHashMap.Const.getKeyD_ofList_of_contains_eq_false contains_eq_false
 
 theorem getKeyD_ofList_of_mem
     {l : List (α × β)}
@@ -1933,25 +1933,25 @@ theorem getKeyD_ofList_of_mem
     (mem : k ∈ l.map Prod.fst) :
     (ofList l).getKeyD k' fallback = k := by
   simp only [ofList_eq_mk]
-  exact Std.DHashMap.Const.getKeyD_ofList_of_mem k_beq distinct mem
+  exact DHashMap.Const.getKeyD_ofList_of_mem k_beq distinct mem
 
 theorem size_ofList
     {l : List (α × β)} (distinct : l.Pairwise (fun a b => (a.1 == b.1) = false)) :
     (ofList l).size = l.length := by
   simp only [ofList_eq_mk]
-  exact Std.DHashMap.Const.size_ofList distinct
+  exact DHashMap.Const.size_ofList distinct
 
 theorem size_ofList_le
     {l : List (α × β)} :
     (ofList l).size ≤ l.length := by
   simp only [ofList_eq_mk]
-  exact Std.DHashMap.Const.size_ofList_le
+  exact DHashMap.Const.size_ofList_le
 
 @[simp]
 theorem ofList_eq_empty_iff {l : List (α × β)} :
     ofList l = ∅ ↔ l = [] := by
   simp only [ofList_eq_mk, ← isEmpty_iff, ← List.isEmpty_iff, Bool.coe_iff_coe]
-  exact Std.DHashMap.Const.isEmpty_ofList
+  exact DHashMap.Const.isEmpty_ofList
 
 @[simp]
 theorem unitOfList_nil :
@@ -1960,16 +1960,16 @@ theorem unitOfList_nil :
 
 @[simp]
 theorem unitOfList_singleton {k : α} :
-    unitOfList [k] = (∅ : DHashMap α (fun _ => Unit)).insertIfNew k () :=
+    unitOfList [k] = (∅ : ExtDHashMap α (fun _ => Unit)).insertIfNew k () :=
   rfl
 
 theorem unitOfList_cons {hd : α} {tl : List α} :
     unitOfList (hd :: tl) =
-      insertManyIfNewUnit ((∅ : DHashMap α (fun _ => Unit)).insertIfNew hd ()) tl :=
+      insertManyIfNewUnit ((∅ : ExtDHashMap α (fun _ => Unit)).insertIfNew hd ()) tl :=
   insertManyIfNewUnit_cons
 
 private theorem unitOfList_eq_mk {l : List α} :
-    (unitOfList l : DHashMap α fun _ => Unit) = Quotient.mk _ (Std.DHashMap.Const.unitOfList l) := by
+    (unitOfList l : ExtDHashMap α fun _ => Unit) = Quotient.mk _ (DHashMap.Const.unitOfList l) := by
   change insertManyIfNewUnit (Quotient.mk _ _) _ = _
   rw [insertManyIfNewUnit_list_mk]
   rfl
@@ -1979,27 +1979,27 @@ theorem contains_unitOfList
     {l : List α} {k : α} :
     (unitOfList l).contains k = l.contains k := by
   simp only [unitOfList_eq_mk]
-  exact Std.DHashMap.Const.contains_unitOfList
+  exact DHashMap.Const.contains_unitOfList
 
 @[simp]
 theorem mem_unitOfList
     {l : List α} {k : α} :
     k ∈ unitOfList l ↔ l.contains k := by
   simp only [unitOfList_eq_mk]
-  exact Std.DHashMap.Const.mem_unitOfList
+  exact DHashMap.Const.mem_unitOfList
 
 theorem getKey?_unitOfList_of_contains_eq_false
     {l : List α} {k : α} (contains_eq_false : l.contains k = false) :
     getKey? (unitOfList l) k = none := by
   simp only [unitOfList_eq_mk]
-  exact Std.DHashMap.Const.getKey?_unitOfList_of_contains_eq_false contains_eq_false
+  exact DHashMap.Const.getKey?_unitOfList_of_contains_eq_false contains_eq_false
 
 theorem getKey?_unitOfList_of_mem
     {l : List α} {k k' : α} (k_beq : k == k')
     (distinct : l.Pairwise (fun a b => (a == b) = false)) (mem : k ∈ l) :
     getKey? (unitOfList l) k' = some k := by
   simp only [unitOfList_eq_mk]
-  exact Std.DHashMap.Const.getKey?_unitOfList_of_mem k_beq distinct mem
+  exact DHashMap.Const.getKey?_unitOfList_of_mem k_beq distinct mem
 
 theorem getKey_unitOfList_of_mem
     {l : List α}
@@ -2008,14 +2008,14 @@ theorem getKey_unitOfList_of_mem
     (mem : k ∈ l) {h} :
     getKey (unitOfList l) k' h = k := by
   simp only [unitOfList_eq_mk]
-  exact Std.DHashMap.Const.getKey_unitOfList_of_mem k_beq distinct mem
+  exact DHashMap.Const.getKey_unitOfList_of_mem k_beq distinct mem
 
 theorem getKey!_unitOfList_of_contains_eq_false
     [Inhabited α] {l : List α} {k : α}
     (contains_eq_false : l.contains k = false) :
     getKey! (unitOfList l) k = default := by
   simp only [unitOfList_eq_mk]
-  exact Std.DHashMap.Const.getKey!_unitOfList_of_contains_eq_false contains_eq_false
+  exact DHashMap.Const.getKey!_unitOfList_of_contains_eq_false contains_eq_false
 
 theorem getKey!_unitOfList_of_mem
     [Inhabited α] {l : List α} {k k' : α} (k_beq : k == k')
@@ -2023,14 +2023,14 @@ theorem getKey!_unitOfList_of_mem
     (mem : k ∈ l) :
     getKey! (unitOfList l) k' = k := by
   simp only [unitOfList_eq_mk]
-  exact Std.DHashMap.Const.getKey!_unitOfList_of_mem k_beq distinct mem
+  exact DHashMap.Const.getKey!_unitOfList_of_mem k_beq distinct mem
 
 theorem getKeyD_unitOfList_of_contains_eq_false
     {l : List α} {k fallback : α}
     (contains_eq_false : l.contains k = false) :
     getKeyD (unitOfList l) k fallback = fallback := by
   simp only [unitOfList_eq_mk]
-  exact Std.DHashMap.Const.getKeyD_unitOfList_of_contains_eq_false contains_eq_false
+  exact DHashMap.Const.getKeyD_unitOfList_of_contains_eq_false contains_eq_false
 
 theorem getKeyD_unitOfList_of_mem
     {l : List α} {k k' fallback : α} (k_beq : k == k')
@@ -2038,26 +2038,26 @@ theorem getKeyD_unitOfList_of_mem
     (mem : k ∈ l) :
     getKeyD (unitOfList l) k' fallback = k := by
   simp only [unitOfList_eq_mk]
-  exact Std.DHashMap.Const.getKeyD_unitOfList_of_mem k_beq distinct mem
+  exact DHashMap.Const.getKeyD_unitOfList_of_mem k_beq distinct mem
 
 theorem size_unitOfList
     {l : List α}
     (distinct : l.Pairwise (fun a b => (a == b) = false)) :
     (unitOfList l).size = l.length := by
   simp only [unitOfList_eq_mk]
-  exact Std.DHashMap.Const.size_unitOfList distinct
+  exact DHashMap.Const.size_unitOfList distinct
 
 theorem size_unitOfList_le
     {l : List α} :
     (unitOfList l).size ≤ l.length := by
   simp only [unitOfList_eq_mk]
-  exact Std.DHashMap.Const.size_unitOfList_le
+  exact DHashMap.Const.size_unitOfList_le
 
 @[simp]
 theorem unitOfList_eq_empty_iff {l : List α} :
     unitOfList l = ∅ ↔ l = [] := by
   simp only [unitOfList_eq_mk, ← isEmpty_iff, ← List.isEmpty_iff, Bool.coe_iff_coe]
-  exact Std.DHashMap.Const.isEmpty_unitOfList
+  exact DHashMap.Const.isEmpty_unitOfList
 
 @[simp]
 theorem get?_unitOfList
@@ -2065,7 +2065,7 @@ theorem get?_unitOfList
     get? (unitOfList l) k =
     if l.contains k then some () else none := by
   simp only [unitOfList_eq_mk]
-  exact Std.DHashMap.Const.get?_unitOfList
+  exact DHashMap.Const.get?_unitOfList
 
 @[simp]
 theorem get_unitOfList
@@ -2087,7 +2087,7 @@ theorem getD_unitOfList
 
 end Const
 
-variable {m : DHashMap α β}
+variable {m : ExtDHashMap α β}
 
 section Alter
 
@@ -2096,7 +2096,7 @@ theorem alter_eq_empty_iff_erase_eq_empty [LawfulBEq α] {k : α} {f : Option (�
   rcases m with ⟨m⟩
   simp only [← isEmpty_iff]
   dsimp only [isEmpty, alter, Quotient.lift, Quotient.mk', Quotient.mk]
-  simp only [Std.DHashMap.isEmpty_alter_eq_isEmpty_erase, Bool.and_eq_true, Option.isNone_iff_eq_none]
+  simp only [DHashMap.isEmpty_alter_eq_isEmpty_erase, Bool.and_eq_true, Option.isNone_iff_eq_none]
   rfl
 
 @[simp]
@@ -2106,33 +2106,33 @@ theorem alter_eq_empty_iff [LawfulBEq α] {k : α} {f : Option (β k) → Option
 
 theorem contains_alter [LawfulBEq α] {k k' : α} {f : Option (β k) → Option (β k)} :
     (m.alter k f).contains k' = if k == k' then (f (m.get? k)).isSome else m.contains k' :=
-  m.inductionOn fun _ => Std.DHashMap.contains_alter
+  m.inductionOn fun _ => DHashMap.contains_alter
 
 theorem mem_alter [LawfulBEq α] {k k' : α} {f : Option (β k) → Option (β k)} :
     k' ∈ m.alter k f ↔ if k == k' then (f (m.get? k)).isSome = true else k' ∈ m :=
-  m.inductionOn fun _ => Std.DHashMap.mem_alter
+  m.inductionOn fun _ => DHashMap.mem_alter
 
 theorem mem_alter_of_beq [LawfulBEq α] {k k' : α} {f : Option (β k) → Option (β k)} (h : k == k') :
     k' ∈ m.alter k f ↔ (f (m.get? k)).isSome :=
-  m.inductionOn (fun _ h => Std.DHashMap.mem_alter_of_beq h) h
+  m.inductionOn (fun _ h => DHashMap.mem_alter_of_beq h) h
 
 @[simp]
 theorem contains_alter_self [LawfulBEq α] {k : α} {f : Option (β k) → Option (β k)} :
     (m.alter k f).contains k = (f (m.get? k)).isSome :=
-  m.inductionOn fun _ => Std.DHashMap.contains_alter_self
+  m.inductionOn fun _ => DHashMap.contains_alter_self
 
 @[simp]
 theorem mem_alter_self [LawfulBEq α] {k : α} {f : Option (β k) → Option (β k)} :
     k ∈ m.alter k f ↔ (f (m.get? k)).isSome :=
-  m.inductionOn fun _ => Std.DHashMap.mem_alter_self
+  m.inductionOn fun _ => DHashMap.mem_alter_self
 
 theorem contains_alter_of_beq_eq_false [LawfulBEq α] {k k' : α} {f : Option (β k) → Option (β k)}
     (h : (k == k') = false) : (m.alter k f).contains k' = m.contains k' :=
-  m.inductionOn (fun _ h => Std.DHashMap.contains_alter_of_beq_eq_false h) h
+  m.inductionOn (fun _ h => DHashMap.contains_alter_of_beq_eq_false h) h
 
 theorem mem_alter_of_beq_eq_false [LawfulBEq α] {k k' : α} {f : Option (β k) → Option (β k)}
     (h : (k == k') = false) : k' ∈ m.alter k f ↔ k' ∈ m :=
-  m.inductionOn (fun _ h => Std.DHashMap.mem_alter_of_beq_eq_false h) h
+  m.inductionOn (fun _ h => DHashMap.mem_alter_of_beq_eq_false h) h
 
 theorem size_alter [LawfulBEq α] {k : α} {f : Option (β k) → Option (β k)} :
     (m.alter k f).size =
@@ -2142,33 +2142,33 @@ theorem size_alter [LawfulBEq α] {k : α} {f : Option (β k) → Option (β k)}
         m.size + 1
       else
         m.size :=
-  m.inductionOn fun _ => Std.DHashMap.size_alter
+  m.inductionOn fun _ => DHashMap.size_alter
 
 theorem size_alter_eq_add_one [LawfulBEq α] {k : α} {f : Option (β k) → Option (β k)}
     (h : k ∉ m) (h' : (f (m.get? k)).isSome) :
     (m.alter k f).size = m.size + 1 :=
-  m.inductionOn (fun _ h h' => Std.DHashMap.size_alter_eq_add_one h h') h h'
+  m.inductionOn (fun _ h h' => DHashMap.size_alter_eq_add_one h h') h h'
 
 theorem size_alter_eq_sub_one [LawfulBEq α] {k : α} {f : Option (β k) → Option (β k)}
     (h : k ∈ m) (h' : (f (m.get? k)).isNone) :
     (m.alter k f).size = m.size - 1 :=
-  m.inductionOn (fun _ h h' => Std.DHashMap.size_alter_eq_sub_one h h') h h'
+  m.inductionOn (fun _ h h' => DHashMap.size_alter_eq_sub_one h h') h h'
 
 theorem size_alter_eq_self_of_not_mem [LawfulBEq α] {k : α} {f : Option (β k) → Option (β k)}
     (h : k ∉ m) (h' : (f (m.get? k)).isNone) : (m.alter k f).size = m.size :=
-  m.inductionOn (fun _ h h' => Std.DHashMap.size_alter_eq_self_of_not_mem h h') h h'
+  m.inductionOn (fun _ h h' => DHashMap.size_alter_eq_self_of_not_mem h h') h h'
 
 theorem size_alter_eq_self_of_mem [LawfulBEq α] {k : α} {f : Option (β k) → Option (β k)}
     (h : k ∈ m) (h' : (f (m.get? k)).isSome) : (m.alter k f).size = m.size :=
-  m.inductionOn (fun _ h h' => Std.DHashMap.size_alter_eq_self_of_mem h h') h h'
+  m.inductionOn (fun _ h h' => DHashMap.size_alter_eq_self_of_mem h h') h h'
 
 theorem size_alter_le_size [LawfulBEq α] {k : α} {f : Option (β k) → Option (β k)} :
     (m.alter k f).size ≤ m.size + 1 :=
-  m.inductionOn fun _ => Std.DHashMap.size_alter_le_size
+  m.inductionOn fun _ => DHashMap.size_alter_le_size
 
 theorem size_le_size_alter [LawfulBEq α] {k : α} {f : Option (β k) → Option (β k)} :
     m.size - 1 ≤ (m.alter k f).size :=
-  m.inductionOn fun _ => Std.DHashMap.size_le_size_alter
+  m.inductionOn fun _ => DHashMap.size_le_size_alter
 
 theorem get?_alter [LawfulBEq α] {k k' : α} {f : Option (β k) → Option (β k)} :
     (m.alter k f).get? k' =
@@ -2176,12 +2176,12 @@ theorem get?_alter [LawfulBEq α] {k k' : α} {f : Option (β k) → Option (β 
         (cast (congrArg (Option ∘ β) (eq_of_beq h)) (f (m.get? k)))
       else
         m.get? k' :=
-  m.inductionOn fun _ => Std.DHashMap.get?_alter
+  m.inductionOn fun _ => DHashMap.get?_alter
 
 @[simp]
 theorem get?_alter_self [LawfulBEq α] {k : α} {f : Option (β k) → Option (β k)} :
     (m.alter k f).get? k = f (m.get? k) :=
-  m.inductionOn fun _ => Std.DHashMap.get?_alter_self
+  m.inductionOn fun _ => DHashMap.get?_alter_self
 
 theorem get_alter [LawfulBEq α] {k k' : α} {f : Option (β k) → Option (β k)}
     {h : k' ∈ m.alter k f} :
@@ -2192,14 +2192,14 @@ theorem get_alter [LawfulBEq α] {k k' : α} {f : Option (β k) → Option (β k
       else
         haveI h' : k' ∈ m := mem_alter_of_beq_eq_false (Bool.not_eq_true _ ▸ heq) |>.mp h
         m.get k' h' :=
-  m.inductionOn (fun _ _ => Std.DHashMap.get_alter) h
+  m.inductionOn (fun _ _ => DHashMap.get_alter) h
 
 @[simp]
 theorem get_alter_self [LawfulBEq α] {k : α} {f : Option (β k) → Option (β k)}
     {h : k ∈ m.alter k f} :
     haveI h' : (f (m.get? k)).isSome := mem_alter_self.mp h
     (m.alter k f).get k h = (f (m.get? k)).get h' :=
-  m.inductionOn (fun _ _ => Std.DHashMap.get_alter_self) h
+  m.inductionOn (fun _ _ => DHashMap.get_alter_self) h
 
 theorem get!_alter [LawfulBEq α] {k k' : α} [hi : Inhabited (β k')]
     {f : Option (β k) → Option (β k)} : (m.alter k f).get! k' =
@@ -2207,12 +2207,12 @@ theorem get!_alter [LawfulBEq α] {k k' : α} [hi : Inhabited (β k')]
         (f (m.get? k)).map (cast (congrArg β (eq_of_beq heq))) |>.get!
       else
         m.get! k' :=
-  m.inductionOn fun _ => Std.DHashMap.get!_alter
+  m.inductionOn fun _ => DHashMap.get!_alter
 
 @[simp]
 theorem get!_alter_self [LawfulBEq α] {k : α} [Inhabited (β k)] {f : Option (β k) → Option (β k)} :
     (m.alter k f).get! k = (f (m.get? k)).get! :=
-  m.inductionOn fun _ => Std.DHashMap.get!_alter_self
+  m.inductionOn fun _ => DHashMap.get!_alter_self
 
 theorem getD_alter [LawfulBEq α] {k k' : α} {fallback : β k'} {f : Option (β k) → Option (β k)} :
     (m.alter k f).getD k' fallback =
@@ -2220,12 +2220,12 @@ theorem getD_alter [LawfulBEq α] {k k' : α} {fallback : β k'} {f : Option (β
         f (m.get? k) |>.map (cast (congrArg β <| eq_of_beq heq)) |>.getD fallback
       else
         m.getD k' fallback :=
-  m.inductionOn fun _ => Std.DHashMap.getD_alter
+  m.inductionOn fun _ => DHashMap.getD_alter
 
 @[simp]
 theorem getD_alter_self [LawfulBEq α] {k : α} {fallback : β k} {f : Option (β k) → Option (β k)} :
     (m.alter k f).getD k fallback = (f (m.get? k)).getD fallback :=
-  m.inductionOn fun _ => Std.DHashMap.getD_alter_self
+  m.inductionOn fun _ => DHashMap.getD_alter_self
 
 theorem getKey?_alter [LawfulBEq α] {k k' : α} {f : Option (β k) → Option (β k)} :
     (m.alter k f).getKey? k' =
@@ -2233,11 +2233,11 @@ theorem getKey?_alter [LawfulBEq α] {k k' : α} {f : Option (β k) → Option (
         if (f (m.get? k)).isSome then some k else none
       else
         m.getKey? k' :=
-  m.inductionOn fun _ => Std.DHashMap.getKey?_alter
+  m.inductionOn fun _ => DHashMap.getKey?_alter
 
 theorem getKey?_alter_self [LawfulBEq α] {k : α} {f : Option (β k) → Option (β k)} :
     (m.alter k f).getKey? k = if (f (m.get? k)).isSome then some k else none :=
-  m.inductionOn fun _ => Std.DHashMap.getKey?_alter_self
+  m.inductionOn fun _ => DHashMap.getKey?_alter_self
 
 theorem getKey!_alter [LawfulBEq α] [Inhabited α] {k k' : α} {f : Option (β k) → Option (β k)} :
     (m.alter k f).getKey! k' =
@@ -2245,11 +2245,11 @@ theorem getKey!_alter [LawfulBEq α] [Inhabited α] {k k' : α} {f : Option (β 
         if (f (m.get? k)).isSome then k else default
       else
         m.getKey! k' :=
-  m.inductionOn fun _ => Std.DHashMap.getKey!_alter
+  m.inductionOn fun _ => DHashMap.getKey!_alter
 
 theorem getKey!_alter_self [LawfulBEq α] [Inhabited α] {k : α} {f : Option (β k) → Option (β k)} :
     (m.alter k f).getKey! k = if (f (m.get? k)).isSome then k else default :=
-  m.inductionOn fun _ => Std.DHashMap.getKey!_alter_self
+  m.inductionOn fun _ => DHashMap.getKey!_alter_self
 
 theorem getKey_alter [LawfulBEq α] [Inhabited α] {k k' : α} {f : Option (β k) → Option (β k)}
     {h : k' ∈ m.alter k f} :
@@ -2259,12 +2259,12 @@ theorem getKey_alter [LawfulBEq α] [Inhabited α] {k k' : α} {f : Option (β k
       else
         haveI h' : k' ∈ m := mem_alter_of_beq_eq_false (Bool.not_eq_true _ ▸ heq) |>.mp h
         m.getKey k' h' :=
-  m.inductionOn (fun _ _ => Std.DHashMap.getKey_alter) h
+  m.inductionOn (fun _ _ => DHashMap.getKey_alter) h
 
 @[simp]
 theorem getKey_alter_self [LawfulBEq α] [Inhabited α] {k : α} {f : Option (β k) → Option (β k)}
     {h : k ∈ m.alter k f} : (m.alter k f).getKey k h = k :=
-  m.inductionOn (fun _ _ => Std.DHashMap.getKey_alter_self) h
+  m.inductionOn (fun _ _ => DHashMap.getKey_alter_self) h
 
 theorem getKeyD_alter [LawfulBEq α] {k k' fallback : α} {f : Option (β k) → Option (β k)} :
     (m.alter k f).getKeyD k' fallback =
@@ -2272,24 +2272,24 @@ theorem getKeyD_alter [LawfulBEq α] {k k' fallback : α} {f : Option (β k) →
         if (f (m.get? k)).isSome then k else fallback
       else
         m.getKeyD k' fallback :=
-  m.inductionOn fun _ => Std.DHashMap.getKeyD_alter
+  m.inductionOn fun _ => DHashMap.getKeyD_alter
 
 @[simp]
 theorem getKeyD_alter_self [LawfulBEq α] [Inhabited α] {k : α} {fallback : α}
     {f : Option (β k) → Option (β k)} :
     (m.alter k f).getKeyD k fallback = if (f (m.get? k)).isSome then k else fallback :=
-  m.inductionOn fun _ => Std.DHashMap.getKeyD_alter_self
+  m.inductionOn fun _ => DHashMap.getKeyD_alter_self
 
 namespace Const
 
-variable {β : Type v} {m : DHashMap α (fun _ => β)}
+variable {β : Type v} {m : ExtDHashMap α (fun _ => β)}
 
 theorem alter_eq_empty_iff_erase_eq_empty {k : α} {f : Option β → Option β} :
     alter m k f = ∅ ↔ m.erase k = ∅ ∧ f (get? m k) = none := by
   rcases m with ⟨m⟩
   simp only [← isEmpty_iff]
   dsimp only [isEmpty, alter, Quotient.lift, Quotient.mk', Quotient.mk]
-  simp only [Std.DHashMap.Const.isEmpty_alter_eq_isEmpty_erase, Bool.and_eq_true,
+  simp only [DHashMap.Const.isEmpty_alter_eq_isEmpty_erase, Bool.and_eq_true,
     Option.isNone_iff_eq_none]
   rfl
 
@@ -2301,34 +2301,34 @@ theorem alter_eq_empty_iff {k : α} {f : Option β → Option β} :
 theorem contains_alter {k k': α} {f : Option β → Option β} :
     (Const.alter m k f).contains k' =
       if k == k' then (f (Const.get? m k)).isSome else m.contains k' :=
-  m.inductionOn fun _ => Std.DHashMap.Const.contains_alter
+  m.inductionOn fun _ => DHashMap.Const.contains_alter
 
 theorem mem_alter {k k': α} {f : Option β → Option β} :
     k' ∈ Const.alter m k f ↔ if k == k' then (f (Const.get? m k)).isSome = true else k' ∈ m :=
-  m.inductionOn fun _ => Std.DHashMap.Const.mem_alter
+  m.inductionOn fun _ => DHashMap.Const.mem_alter
 
 theorem mem_alter_of_beq {k k': α} {f : Option β → Option β}
     (h : k == k') : k' ∈ Const.alter m k f ↔ (f (Const.get? m k)).isSome :=
-  m.inductionOn (fun _ h => Std.DHashMap.Const.mem_alter_of_beq h) h
+  m.inductionOn (fun _ h => DHashMap.Const.mem_alter_of_beq h) h
 
 @[simp]
 theorem contains_alter_self {k : α} {f : Option β → Option β} :
     (Const.alter m k f).contains k = (f (Const.get? m k)).isSome :=
-  m.inductionOn fun _ => Std.DHashMap.Const.contains_alter_self
+  m.inductionOn fun _ => DHashMap.Const.contains_alter_self
 
 @[simp]
 theorem mem_alter_self {k : α} {f : Option β → Option β} :
     k ∈ Const.alter m k f ↔ (f (Const.get? m k)).isSome :=
-  m.inductionOn fun _ => Std.DHashMap.Const.mem_alter_self
+  m.inductionOn fun _ => DHashMap.Const.mem_alter_self
 
 theorem contains_alter_of_beq_eq_false {k k' : α}
     {f : Option β → Option β} (h : (k == k') = false) :
     (Const.alter m k f).contains k' = m.contains k' :=
-  m.inductionOn (fun _ h => Std.DHashMap.Const.contains_alter_of_beq_eq_false h) h
+  m.inductionOn (fun _ h => DHashMap.Const.contains_alter_of_beq_eq_false h) h
 
 theorem mem_alter_of_beq_eq_false {k k' : α}
     {f : Option β → Option β} (h : (k == k') = false) : k' ∈ Const.alter m k f ↔ k' ∈ m :=
-  m.inductionOn (fun _ h => Std.DHashMap.Const.mem_alter_of_beq_eq_false h) h
+  m.inductionOn (fun _ h => DHashMap.Const.mem_alter_of_beq_eq_false h) h
 
 theorem size_alter {k : α} {f : Option β → Option β} :
     (Const.alter m k f).size =
@@ -2338,33 +2338,33 @@ theorem size_alter {k : α} {f : Option β → Option β} :
         m.size + 1
       else
         m.size :=
-  m.inductionOn fun _ => Std.DHashMap.Const.size_alter
+  m.inductionOn fun _ => DHashMap.Const.size_alter
 
 theorem size_alter_eq_add_one {k : α} {f : Option β → Option β}
     (h : k ∉ m) (h' : (f (Const.get? m k)).isSome) :
     (Const.alter m k f).size = m.size + 1 :=
-  m.inductionOn (fun _ h h' => Std.DHashMap.Const.size_alter_eq_add_one h h') h h'
+  m.inductionOn (fun _ h h' => DHashMap.Const.size_alter_eq_add_one h h') h h'
 
 theorem size_alter_eq_sub_one {k : α} {f : Option β → Option β}
     (h : k ∈ m) (h' : (f (Const.get? m k)).isNone) :
     (Const.alter m k f).size = m.size - 1 :=
-  m.inductionOn (fun _ h h' => Std.DHashMap.Const.size_alter_eq_sub_one h h') h h'
+  m.inductionOn (fun _ h h' => DHashMap.Const.size_alter_eq_sub_one h h') h h'
 
 theorem size_alter_eq_self_of_not_mem {k : α} {f : Option β → Option β}
     (h : k ∉ m) (h' : (f (Const.get? m k)).isNone) : (Const.alter m k f).size = m.size :=
-  m.inductionOn (fun _ h h' => Std.DHashMap.Const.size_alter_eq_self_of_not_mem h h') h h'
+  m.inductionOn (fun _ h h' => DHashMap.Const.size_alter_eq_self_of_not_mem h h') h h'
 
 theorem size_alter_eq_self_of_mem {k : α} {f : Option β → Option β}
     (h : k ∈ m) (h' : (f (Const.get? m k)).isSome) : (Const.alter m k f).size = m.size :=
-  m.inductionOn (fun _ h h' => Std.DHashMap.Const.size_alter_eq_self_of_mem h h') h h'
+  m.inductionOn (fun _ h h' => DHashMap.Const.size_alter_eq_self_of_mem h h') h h'
 
 theorem size_alter_le_size {k : α} {f : Option β → Option β} :
     (Const.alter m k f).size ≤ m.size + 1 :=
-  m.inductionOn fun _ => Std.DHashMap.Const.size_alter_le_size
+  m.inductionOn fun _ => DHashMap.Const.size_alter_le_size
 
 theorem size_le_size_alter {k : α} {f : Option β → Option β} :
     m.size - 1 ≤ (Const.alter m k f).size :=
-  m.inductionOn fun _ => Std.DHashMap.Const.size_le_size_alter
+  m.inductionOn fun _ => DHashMap.Const.size_le_size_alter
 
 theorem get?_alter {k k' : α} {f : Option β → Option β} :
     Const.get? (Const.alter m k f) k' =
@@ -2372,12 +2372,12 @@ theorem get?_alter {k k' : α} {f : Option β → Option β} :
         f (Const.get? m k)
       else
         Const.get? m k' :=
-  m.inductionOn fun _ => Std.DHashMap.Const.get?_alter
+  m.inductionOn fun _ => DHashMap.Const.get?_alter
 
 @[simp]
 theorem get?_alter_self {k : α} {f : Option β → Option β} :
     Const.get? (Const.alter m k f) k = f (Const.get? m k) :=
-  m.inductionOn fun _ => Std.DHashMap.Const.get?_alter_self
+  m.inductionOn fun _ => DHashMap.Const.get?_alter_self
 
 theorem get_alter {k k' : α} {f : Option β → Option β}
     {h : k' ∈ Const.alter m k f} :
@@ -2388,14 +2388,14 @@ theorem get_alter {k k' : α} {f : Option β → Option β}
       else
         haveI h' : k' ∈ m := mem_alter_of_beq_eq_false (Bool.not_eq_true _ ▸ heq) |>.mp h
         Const.get m k' h' :=
-  m.inductionOn (fun _ _ => Std.DHashMap.Const.get_alter) h
+  m.inductionOn (fun _ _ => DHashMap.Const.get_alter) h
 
 @[simp]
 theorem get_alter_self {k : α} {f : Option β → Option β}
     {h : k ∈ Const.alter m k f} :
     haveI h' : (f (Const.get? m k)).isSome := mem_alter_self.mp h
     Const.get (Const.alter m k f) k h = (f (Const.get? m k)).get h' :=
-  m.inductionOn (fun _ _ => Std.DHashMap.Const.get_alter_self) h
+  m.inductionOn (fun _ _ => DHashMap.Const.get_alter_self) h
 
 theorem get!_alter {k k' : α} [Inhabited β]
     {f : Option β → Option β} : Const.get! (Const.alter m k f) k' =
@@ -2403,12 +2403,12 @@ theorem get!_alter {k k' : α} [Inhabited β]
         f (Const.get? m k) |>.get!
       else
         Const.get! m k' :=
-  m.inductionOn fun _ => Std.DHashMap.Const.get!_alter
+  m.inductionOn fun _ => DHashMap.Const.get!_alter
 
 @[simp]
 theorem get!_alter_self {k : α} [Inhabited β]
     {f : Option β → Option β} : Const.get! (Const.alter m k f) k = (f (Const.get? m k)).get! :=
-  m.inductionOn fun _ => Std.DHashMap.Const.get!_alter_self
+  m.inductionOn fun _ => DHashMap.Const.get!_alter_self
 
 theorem getD_alter {k k' : α} {fallback : β}
     {f : Option β → Option β} :
@@ -2417,13 +2417,13 @@ theorem getD_alter {k k' : α} {fallback : β}
         f (Const.get? m k) |>.getD fallback
       else
         Const.getD m k' fallback :=
-  m.inductionOn fun _ => Std.DHashMap.Const.getD_alter
+  m.inductionOn fun _ => DHashMap.Const.getD_alter
 
 @[simp]
 theorem getD_alter_self {k : α} {fallback : β}
     {f : Option β → Option β} :
     Const.getD (Const.alter m k f) k fallback = (f (Const.get? m k)).getD fallback :=
-  m.inductionOn fun _ => Std.DHashMap.Const.getD_alter_self
+  m.inductionOn fun _ => DHashMap.Const.getD_alter_self
 
 theorem getKey?_alter {k k' : α} {f : Option β → Option β} :
     (Const.alter m k f).getKey? k' =
@@ -2431,11 +2431,11 @@ theorem getKey?_alter {k k' : α} {f : Option β → Option β} :
         if (f (Const.get? m k)).isSome then some k else none
       else
         m.getKey? k' :=
-  m.inductionOn fun _ => Std.DHashMap.Const.getKey?_alter
+  m.inductionOn fun _ => DHashMap.Const.getKey?_alter
 
 theorem getKey?_alter_self {k : α} {f : Option β → Option β} :
     (Const.alter m k f).getKey? k = if (f (Const.get? m k)).isSome then some k else none :=
-  m.inductionOn fun _ => Std.DHashMap.Const.getKey?_alter_self
+  m.inductionOn fun _ => DHashMap.Const.getKey?_alter_self
 
 theorem getKey!_alter [Inhabited α] {k k' : α}
     {f : Option β → Option β} : (Const.alter m k f).getKey! k' =
@@ -2443,12 +2443,12 @@ theorem getKey!_alter [Inhabited α] {k k' : α}
         if (f (Const.get? m k)).isSome then k else default
       else
         m.getKey! k' :=
-  m.inductionOn fun _ => Std.DHashMap.Const.getKey!_alter
+  m.inductionOn fun _ => DHashMap.Const.getKey!_alter
 
 theorem getKey!_alter_self [Inhabited α] {k : α}
     {f : Option β → Option β} :
     (Const.alter m k f).getKey! k = if (f (Const.get? m k)).isSome then k else default :=
-  m.inductionOn fun _ => Std.DHashMap.Const.getKey!_alter_self
+  m.inductionOn fun _ => DHashMap.Const.getKey!_alter_self
 
 theorem getKey_alter [Inhabited α] {k k' : α}
     {f : Option β → Option β} {h : k' ∈ Const.alter m k f} :
@@ -2458,13 +2458,13 @@ theorem getKey_alter [Inhabited α] {k k' : α}
       else
         haveI h' : k' ∈ m := mem_alter_of_beq_eq_false (Bool.not_eq_true _ ▸ heq) |>.mp h
         m.getKey k' h' :=
-  m.inductionOn (fun _ _ => Std.DHashMap.Const.getKey_alter) h
+  m.inductionOn (fun _ _ => DHashMap.Const.getKey_alter) h
 
 @[simp]
 theorem getKey_alter_self [Inhabited α] {k : α}
     {f : Option β → Option β} {h : k ∈ Const.alter m k f} :
     (Const.alter m k f).getKey k h = k :=
-  m.inductionOn (fun _ _ => Std.DHashMap.Const.getKey_alter_self) h
+  m.inductionOn (fun _ _ => DHashMap.Const.getKey_alter_self) h
 
 theorem getKeyD_alter {k k' fallback : α} {f : Option β → Option β} :
     (Const.alter m k f).getKeyD k' fallback =
@@ -2472,13 +2472,13 @@ theorem getKeyD_alter {k k' fallback : α} {f : Option β → Option β} :
         if (f (Const.get? m k)).isSome then k else fallback
       else
         m.getKeyD k' fallback :=
-  m.inductionOn fun _ => Std.DHashMap.Const.getKeyD_alter
+  m.inductionOn fun _ => DHashMap.Const.getKeyD_alter
 
 theorem getKeyD_alter_self [Inhabited α] {k fallback : α}
     {f : Option β → Option β} :
     (Const.alter m k f).getKeyD k fallback =
       if (f (Const.get? m k)).isSome then k else fallback :=
-  m.inductionOn fun _ => Std.DHashMap.Const.getKeyD_alter_self
+  m.inductionOn fun _ => DHashMap.Const.getKeyD_alter_self
 
 end Const
 
@@ -2490,32 +2490,32 @@ section Modify
 theorem modify_eq_empty_iff [LawfulBEq α] {k : α} {f : β k → β k} :
     m.modify k f = ∅ ↔ m = ∅ := by
   simp only [← isEmpty_iff, Bool.coe_iff_coe]
-  exact m.inductionOn fun _ => Std.DHashMap.isEmpty_modify
+  exact m.inductionOn fun _ => DHashMap.isEmpty_modify
 
 @[simp]
 theorem contains_modify [LawfulBEq α] {k k': α} {f : β k → β k} :
     (m.modify k f).contains k' = m.contains k' :=
-  m.inductionOn fun _ => Std.DHashMap.contains_modify
+  m.inductionOn fun _ => DHashMap.contains_modify
 
 @[simp]
 theorem mem_modify [LawfulBEq α] {k k': α} {f : β k → β k} : k' ∈ m.modify k f ↔ k' ∈ m :=
-  m.inductionOn fun _ => Std.DHashMap.mem_modify
+  m.inductionOn fun _ => DHashMap.mem_modify
 
 @[simp]
 theorem size_modify [LawfulBEq α] {k : α} {f : β k → β k} : (m.modify k f).size = m.size :=
-  m.inductionOn fun _ => Std.DHashMap.size_modify
+  m.inductionOn fun _ => DHashMap.size_modify
 
 theorem get?_modify [LawfulBEq α] {k k' : α} {f : β k → β k} :
     (m.modify k f).get? k' = if h : k == k' then
       (cast (congrArg (Option ∘ β) (eq_of_beq h)) ((m.get? k).map f))
     else
       m.get? k' :=
-  m.inductionOn fun _ => Std.DHashMap.get?_modify
+  m.inductionOn fun _ => DHashMap.get?_modify
 
 @[simp]
 theorem get?_modify_self [LawfulBEq α] {k : α} {f : β k → β k} :
     (m.modify k f).get? k = (m.get? k).map f :=
-  m.inductionOn fun _ => Std.DHashMap.get?_modify_self
+  m.inductionOn fun _ => DHashMap.get?_modify_self
 
 theorem get_modify [LawfulBEq α] {k k' : α} {f : β k → β k}
     (h : k' ∈ m.modify k f) :
@@ -2526,13 +2526,13 @@ theorem get_modify [LawfulBEq α] {k k' : α} {f : β k → β k}
       else
         haveI h' : k' ∈ m := mem_modify.mp h
         m.get k' h' :=
-  m.inductionOn (fun _ h => Std.DHashMap.get_modify h) h
+  m.inductionOn (fun _ h => DHashMap.get_modify h) h
 
 @[simp]
 theorem get_modify_self [LawfulBEq α] {k : α} {f : β k → β k} {h : k ∈ m.modify k f} :
     haveI h' : k ∈ m := mem_modify.mp h
     (m.modify k f).get k h = f (m.get k h') :=
-  m.inductionOn (fun _ _ => Std.DHashMap.get_modify_self) h
+  m.inductionOn (fun _ _ => DHashMap.get_modify_self) h
 
 theorem get!_modify [LawfulBEq α] {k k' : α} [hi : Inhabited (β k')] {f : β k → β k} :
     (m.modify k f).get! k' =
@@ -2540,12 +2540,12 @@ theorem get!_modify [LawfulBEq α] {k k' : α} [hi : Inhabited (β k')] {f : β 
         m.get? k |>.map f |>.map (cast (congrArg β (eq_of_beq heq))) |>.get!
       else
         m.get! k' :=
-  m.inductionOn fun _ => Std.DHashMap.get!_modify
+  m.inductionOn fun _ => DHashMap.get!_modify
 
 @[simp]
 theorem get!_modify_self [LawfulBEq α] {k : α} [Inhabited (β k)] {f : β k → β k} :
     (m.modify k f).get! k = ((m.get? k).map f).get! :=
-  m.inductionOn fun _ => Std.DHashMap.get!_modify_self
+  m.inductionOn fun _ => DHashMap.get!_modify_self
 
 theorem getD_modify [LawfulBEq α] {k k' : α} {fallback : β k'} {f : β k → β k} :
     (m.modify k f).getD k' fallback =
@@ -2553,12 +2553,12 @@ theorem getD_modify [LawfulBEq α] {k k' : α} {fallback : β k'} {f : β k → 
         m.get? k |>.map f |>.map (cast (congrArg β <| eq_of_beq heq)) |>.getD fallback
       else
         m.getD k' fallback :=
-  m.inductionOn fun _ => Std.DHashMap.getD_modify
+  m.inductionOn fun _ => DHashMap.getD_modify
 
 @[simp]
 theorem getD_modify_self [LawfulBEq α] {k : α} {fallback : β k} {f : β k → β k} :
     (m.modify k f).getD k fallback = ((m.get? k).map f).getD fallback :=
-  m.inductionOn fun _ => Std.DHashMap.getD_modify_self
+  m.inductionOn fun _ => DHashMap.getD_modify_self
 
 theorem getKey?_modify [LawfulBEq α] {k k' : α} {f : β k → β k} :
     (m.modify k f).getKey? k' =
@@ -2566,11 +2566,11 @@ theorem getKey?_modify [LawfulBEq α] {k k' : α} {f : β k → β k} :
         if k ∈ m then some k else none
       else
         m.getKey? k' :=
-  m.inductionOn fun _ => Std.DHashMap.getKey?_modify
+  m.inductionOn fun _ => DHashMap.getKey?_modify
 
 theorem getKey?_modify_self [LawfulBEq α] {k : α} {f : β k → β k} :
     (m.modify k f).getKey? k = if k ∈ m then some k else none :=
-  m.inductionOn fun _ => Std.DHashMap.getKey?_modify_self
+  m.inductionOn fun _ => DHashMap.getKey?_modify_self
 
 theorem getKey!_modify [LawfulBEq α] [Inhabited α] {k k' : α} {f : β k → β k} :
     (m.modify k f).getKey! k' =
@@ -2578,11 +2578,11 @@ theorem getKey!_modify [LawfulBEq α] [Inhabited α] {k k' : α} {f : β k → �
         if k ∈ m then k else default
       else
         m.getKey! k' :=
-  m.inductionOn fun _ => Std.DHashMap.getKey!_modify
+  m.inductionOn fun _ => DHashMap.getKey!_modify
 
 theorem getKey!_modify_self [LawfulBEq α] [Inhabited α] {k : α} {f : β k → β k} :
     (m.modify k f).getKey! k = if k ∈ m then k else default :=
-  m.inductionOn fun _ => Std.DHashMap.getKey!_modify_self
+  m.inductionOn fun _ => DHashMap.getKey!_modify_self
 
 theorem getKey_modify [LawfulBEq α] [Inhabited α] {k k' : α} {f : β k → β k}
     {h : k' ∈ m.modify k f} :
@@ -2592,12 +2592,12 @@ theorem getKey_modify [LawfulBEq α] [Inhabited α] {k k' : α} {f : β k → β
       else
         haveI h' : k' ∈ m := mem_modify.mp h
         m.getKey k' h' :=
-  m.inductionOn (fun _ _ => Std.DHashMap.getKey_modify) h
+  m.inductionOn (fun _ _ => DHashMap.getKey_modify) h
 
 @[simp]
 theorem getKey_modify_self [LawfulBEq α] [Inhabited α] {k : α} {f : β k → β k}
     {h : k ∈ m.modify k f} : (m.modify k f).getKey k h = k :=
-  m.inductionOn (fun _ _ => Std.DHashMap.getKey_modify_self) h
+  m.inductionOn (fun _ _ => DHashMap.getKey_modify_self) h
 
 theorem getKeyD_modify [LawfulBEq α] {k k' fallback : α} {f : β k → β k} :
     (m.modify k f).getKeyD k' fallback =
@@ -2605,48 +2605,48 @@ theorem getKeyD_modify [LawfulBEq α] {k k' fallback : α} {f : β k → β k} :
         if k ∈ m then k else fallback
       else
         m.getKeyD k' fallback :=
-  m.inductionOn fun _ => Std.DHashMap.getKeyD_modify
+  m.inductionOn fun _ => DHashMap.getKeyD_modify
 
 theorem getKeyD_modify_self [LawfulBEq α] [Inhabited α] {k fallback : α} {f : β k → β k} :
     (m.modify k f).getKeyD k fallback = if k ∈ m then k else fallback :=
-  m.inductionOn fun _ => Std.DHashMap.getKeyD_modify_self
+  m.inductionOn fun _ => DHashMap.getKeyD_modify_self
 
 namespace Const
 
-variable {β : Type v} {m : DHashMap α (fun _ => β)}
+variable {β : Type v} {m : ExtDHashMap α (fun _ => β)}
 
 @[simp]
 theorem modify_eq_empty_iff {k : α} {f : β → β} :
     Const.modify m k f = ∅ ↔ m = ∅ := by
   simp only [← isEmpty_iff, Bool.coe_iff_coe]
-  exact m.inductionOn fun _ => Std.DHashMap.Const.isEmpty_modify
+  exact m.inductionOn fun _ => DHashMap.Const.isEmpty_modify
 
 @[simp]
 theorem contains_modify {k k': α} {f : β → β} :
     (Const.modify m k f).contains k' = m.contains k' :=
-  m.inductionOn fun _ => Std.DHashMap.Const.contains_modify
+  m.inductionOn fun _ => DHashMap.Const.contains_modify
 
 @[simp]
 theorem mem_modify {k k': α} {f : β → β} :
     k' ∈ Const.modify m k f ↔ k' ∈ m :=
-  m.inductionOn fun _ => Std.DHashMap.Const.mem_modify
+  m.inductionOn fun _ => DHashMap.Const.mem_modify
 
 @[simp]
 theorem size_modify {k : α} {f : β → β} :
     (Const.modify m k f).size = m.size :=
-  m.inductionOn fun _ => Std.DHashMap.Const.size_modify
+  m.inductionOn fun _ => DHashMap.Const.size_modify
 
 theorem get?_modify {k k' : α} {f : β → β} :
     Const.get? (Const.modify m k f) k' = if k == k' then
       Const.get? m k |>.map f
     else
       Const.get? m k' :=
-  m.inductionOn fun _ => Std.DHashMap.Const.get?_modify
+  m.inductionOn fun _ => DHashMap.Const.get?_modify
 
 @[simp]
 theorem get?_modify_self {k : α} {f : β → β} :
     Const.get? (Const.modify m k f) k = (Const.get? m k).map f :=
-  m.inductionOn fun _ => Std.DHashMap.Const.get?_modify_self
+  m.inductionOn fun _ => DHashMap.Const.get?_modify_self
 
 theorem get_modify {k k' : α} {f : β → β}
     {h : k' ∈ Const.modify m k f} :
@@ -2657,14 +2657,14 @@ theorem get_modify {k k' : α} {f : β → β}
       else
         haveI h' : k' ∈ m := mem_modify.mp h
         Const.get m k' h' :=
-  m.inductionOn (fun _ _ => Std.DHashMap.Const.get_modify) h
+  m.inductionOn (fun _ _ => DHashMap.Const.get_modify) h
 
 @[simp]
 theorem get_modify_self {k : α} {f : β → β}
     {h : k ∈ Const.modify m k f} :
     haveI h' : k ∈ m := mem_modify.mp h
     Const.get (Const.modify m k f) k h = f (Const.get m k h') :=
-  m.inductionOn (fun _ _ => Std.DHashMap.Const.get_modify_self) h
+  m.inductionOn (fun _ _ => DHashMap.Const.get_modify_self) h
 
 theorem get!_modify {k k' : α} [Inhabited β] {f : β → β} :
     Const.get! (Const.modify m k f) k' =
@@ -2672,12 +2672,12 @@ theorem get!_modify {k k' : α} [Inhabited β] {f : β → β} :
         Const.get? m k |>.map f |>.get!
       else
         Const.get! m k' :=
-  m.inductionOn fun _ => Std.DHashMap.Const.get!_modify
+  m.inductionOn fun _ => DHashMap.Const.get!_modify
 
 @[simp]
 theorem get!_modify_self {k : α} [Inhabited β] {f : β → β} :
     Const.get! (Const.modify m k f) k = ((Const.get? m k).map f).get! :=
-  m.inductionOn fun _ => Std.DHashMap.Const.get!_modify_self
+  m.inductionOn fun _ => DHashMap.Const.get!_modify_self
 
 theorem getD_modify {k k' : α} {fallback : β} {f : β → β} :
     Const.getD (Const.modify m k f) k' fallback =
@@ -2685,12 +2685,12 @@ theorem getD_modify {k k' : α} {fallback : β} {f : β → β} :
         Const.get? m k |>.map f |>.getD fallback
       else
         Const.getD m k' fallback :=
-  m.inductionOn fun _ => Std.DHashMap.Const.getD_modify
+  m.inductionOn fun _ => DHashMap.Const.getD_modify
 
 @[simp]
 theorem getD_modify_self {k : α} {fallback : β} {f : β → β} :
     Const.getD (Const.modify m k f) k fallback = ((Const.get? m k).map f).getD fallback :=
-  m.inductionOn fun _ => Std.DHashMap.Const.getD_modify_self
+  m.inductionOn fun _ => DHashMap.Const.getD_modify_self
 
 theorem getKey?_modify {k k' : α} {f : β → β} :
     (Const.modify m k f).getKey? k' =
@@ -2698,11 +2698,11 @@ theorem getKey?_modify {k k' : α} {f : β → β} :
         if k ∈ m then some k else none
       else
         m.getKey? k' :=
-  m.inductionOn fun _ => Std.DHashMap.Const.getKey?_modify
+  m.inductionOn fun _ => DHashMap.Const.getKey?_modify
 
 theorem getKey?_modify_self {k : α} {f : β → β} :
     (Const.modify m k f).getKey? k = if k ∈ m then some k else none :=
-  m.inductionOn fun _ => Std.DHashMap.Const.getKey?_modify_self
+  m.inductionOn fun _ => DHashMap.Const.getKey?_modify_self
 
 theorem getKey!_modify [Inhabited α] {k k' : α} {f : β → β} :
     (Const.modify m k f).getKey! k' =
@@ -2710,11 +2710,11 @@ theorem getKey!_modify [Inhabited α] {k k' : α} {f : β → β} :
         if k ∈ m then k else default
       else
         m.getKey! k' :=
-  m.inductionOn fun _ => Std.DHashMap.Const.getKey!_modify
+  m.inductionOn fun _ => DHashMap.Const.getKey!_modify
 
 theorem getKey!_modify_self [Inhabited α] {k : α} {f : β → β} :
     (Const.modify m k f).getKey! k = if k ∈ m then k else default :=
-  m.inductionOn fun _ => Std.DHashMap.Const.getKey!_modify_self
+  m.inductionOn fun _ => DHashMap.Const.getKey!_modify_self
 
 theorem getKey_modify [Inhabited α] {k k' : α} {f : β → β}
     {h : k' ∈ Const.modify m k f} :
@@ -2724,12 +2724,12 @@ theorem getKey_modify [Inhabited α] {k k' : α} {f : β → β}
       else
         haveI h' : k' ∈ m := mem_modify.mp h
         m.getKey k' h' :=
-  m.inductionOn (fun _ _ => Std.DHashMap.Const.getKey_modify) h
+  m.inductionOn (fun _ _ => DHashMap.Const.getKey_modify) h
 
 @[simp]
 theorem getKey_modify_self [Inhabited α] {k : α} {f : β → β}
     {h : k ∈ Const.modify m k f} : (Const.modify m k f).getKey k h = k :=
-  m.inductionOn (fun _ _ => Std.DHashMap.Const.getKey_modify_self) h
+  m.inductionOn (fun _ _ => DHashMap.Const.getKey_modify_self) h
 
 theorem getKeyD_modify {k k' fallback : α} {f : β → β} :
     (Const.modify m k f).getKeyD k' fallback =
@@ -2737,11 +2737,11 @@ theorem getKeyD_modify {k k' fallback : α} {f : β → β} :
         if k ∈ m then k else fallback
       else
         m.getKeyD k' fallback :=
-  m.inductionOn fun _ => Std.DHashMap.Const.getKeyD_modify
+  m.inductionOn fun _ => DHashMap.Const.getKeyD_modify
 
 theorem getKeyD_modify_self [Inhabited α] {k fallback : α} {f : β → β} :
     (Const.modify m k f).getKeyD k fallback = if k ∈ m then k else fallback :=
-  m.inductionOn fun _ => Std.DHashMap.Const.getKeyD_modify_self
+  m.inductionOn fun _ => DHashMap.Const.getKeyD_modify_self
 
 end Const
 
@@ -2749,29 +2749,29 @@ end Modify
 
 section Equiv
 
-variable {m₁ m₂ : DHashMap α β}
+variable {m₁ m₂ m₃ : Std.ExtDHashMap α β}
 
 theorem ext_get? [LawfulBEq α] (h : ∀ k, m₁.get? k = m₂.get? k) : m₁ = m₂ :=
   m₁.inductionOn₂ m₂ (fun _ _ h => Quotient.sound (.of_forall_get?_eq h)) h
 
 namespace Const
 
-variable {β : Type v} {m₁ m₂ : DHashMap α fun _ => β}
+variable {β : Type v} {m₁ m₂ : ExtDHashMap α fun _ => β}
 
 theorem ext_getKey?_get? (hk : ∀ k, m₁.getKey? k = m₂.getKey? k)
     (hv : ∀ k, Const.get? m₁ k = Const.get? m₂ k) : m₁ = m₂ :=
   m₁.inductionOn₂ m₂ (fun _ _ hk hv => Quotient.sound
     (.of_forall_getKey?_eq_of_forall_constGet?_eq hk hv)) hk hv
 
-theorem ext_getKey?_unit {m₁ m₂ : DHashMap α fun _ => Unit}
+theorem ext_getKey?_unit {m₁ m₂ : ExtDHashMap α fun _ => Unit}
     (h : ∀ k, m₁.getKey? k = m₂.getKey? k) : m₁ = m₂ :=
   m₁.inductionOn₂ m₂ (fun _ _ h => Quotient.sound (.of_forall_getKey?_unit_eq h)) h
 
-theorem ext_contains_unit [LawfulBEq α] {m₁ m₂ : DHashMap α fun _ => Unit}
+theorem ext_contains_unit [LawfulBEq α] {m₁ m₂ : ExtDHashMap α fun _ => Unit}
     (h : ∀ k, m₁.contains k = m₂.contains k) : m₁ = m₂ :=
   m₁.inductionOn₂ m₂ (fun _ _ h => Quotient.sound (.of_forall_contains_unit_eq h)) h
 
-theorem ext_mem_unit [LawfulBEq α] {m₁ m₂ : DHashMap α fun _ => Unit}
+theorem ext_mem_unit [LawfulBEq α] {m₁ m₂ : ExtDHashMap α fun _ => Unit}
     (h : ∀ k, k ∈ m₁ ↔ k ∈ m₂) : m₁ = m₂ :=
   m₁.inductionOn₂ m₂ (fun _ _ h => Quotient.sound (.of_forall_mem_unit_iff h)) h
 
@@ -2786,49 +2786,49 @@ variable {γ : α → Type w}
 theorem filterMap_eq_empty_iff [LawfulBEq α]
     {f : (a : α) → β a → Option (γ a)} :
     m.filterMap f = ∅ ↔ ∀ k h, f k (m.get k h) = none :=
-  isEmpty_iff.symm.trans <| m.inductionOn fun _ => Std.DHashMap.isEmpty_filterMap_iff
+  isEmpty_iff.symm.trans <| m.inductionOn fun _ => DHashMap.isEmpty_filterMap_iff
 
 theorem contains_filterMap [LawfulBEq α]
     {f : (a : α) → β a → Option (γ a)} {k : α} :
     (m.filterMap f).contains k = (m.get? k).any (f k · |>.isSome) :=
-  m.inductionOn fun _ => Std.DHashMap.contains_filterMap
+  m.inductionOn fun _ => DHashMap.contains_filterMap
 
 theorem mem_filterMap [LawfulBEq α]
     {f : (a : α) → β a → Option (γ a)} {k : α} :
     k ∈ m.filterMap f ↔ ∃ h, (f k (m.get k h)).isSome :=
-  m.inductionOn fun _ => Std.DHashMap.mem_filterMap
+  m.inductionOn fun _ => DHashMap.mem_filterMap
 
 theorem contains_of_contains_filterMap
     {f : (a : α) → β a → Option (γ a)} {k : α} :
     (m.filterMap f).contains k = true → m.contains k = true :=
-  m.inductionOn fun _ => Std.DHashMap.contains_of_contains_filterMap
+  m.inductionOn fun _ => DHashMap.contains_of_contains_filterMap
 
 theorem mem_of_mem_filterMap
     {f : (a : α) → β a → Option (γ a)} {k : α} :
     k ∈ m.filterMap f → k ∈ m :=
-  m.inductionOn fun _ => Std.DHashMap.mem_of_mem_filterMap
+  m.inductionOn fun _ => DHashMap.mem_of_mem_filterMap
 
 theorem size_filterMap_le_size
     {f : (a : α) → β a → Option (γ a)} :
     (m.filterMap f).size ≤ m.size :=
-  m.inductionOn fun _ => Std.DHashMap.size_filterMap_le_size
+  m.inductionOn fun _ => DHashMap.size_filterMap_le_size
 
 theorem size_filterMap_eq_size_iff [LawfulBEq α]
     {f : (a : α) → β a → Option (γ a)} :
     (m.filterMap f).size = m.size ↔ ∀ (a : α) (h : a ∈ m), (f a (m.get a h)).isSome :=
-  m.inductionOn fun _ => Std.DHashMap.size_filterMap_eq_size_iff
+  m.inductionOn fun _ => DHashMap.size_filterMap_eq_size_iff
 
 @[simp]
 theorem get?_filterMap [LawfulBEq α]
     {f : (a : α) → β a → Option (γ a)} {k : α} :
     (m.filterMap f).get? k = (m.get? k).bind (f k) :=
-  m.inductionOn fun _ => Std.DHashMap.get?_filterMap
+  m.inductionOn fun _ => DHashMap.get?_filterMap
 
 theorem isSome_apply_of_mem_filterMap [LawfulBEq α]
     {f : (a : α) → β a → Option (γ a)} {k : α} :
     ∀ (h' : k ∈ m.filterMap f),
       (f k (m.get k (mem_of_mem_filterMap h'))).isSome :=
-  m.inductionOn fun _ => Std.DHashMap.isSome_apply_of_mem_filterMap
+  m.inductionOn fun _ => DHashMap.isSome_apply_of_mem_filterMap
 
 @[simp]
 theorem get_filterMap [LawfulBEq α]
@@ -2836,80 +2836,80 @@ theorem get_filterMap [LawfulBEq α]
     (m.filterMap f).get k h' =
       (f k (m.get k (mem_of_mem_filterMap h'))).get
         (isSome_apply_of_mem_filterMap h') :=
-  m.inductionOn (fun _ _ => Std.DHashMap.get_filterMap) h'
+  m.inductionOn (fun _ _ => DHashMap.get_filterMap) h'
 
 theorem get!_filterMap [LawfulBEq α]
     {f : (a : α) → β a → Option (γ a)} {k : α} [Inhabited (γ k)] :
     (m.filterMap f).get! k = ((m.get? k).bind (f k)).get! :=
-  m.inductionOn fun _ => Std.DHashMap.get!_filterMap
+  m.inductionOn fun _ => DHashMap.get!_filterMap
 
 theorem getD_filterMap [LawfulBEq α]
     {f : (a : α) → β a → Option (γ a)} {k : α} {fallback : γ k} :
     (m.filterMap f).getD k fallback = ((m.get? k).bind (f k)).getD fallback :=
-  m.inductionOn fun _ => Std.DHashMap.getD_filterMap
+  m.inductionOn fun _ => DHashMap.getD_filterMap
 
 theorem getKey?_filterMap [LawfulBEq α]
     {f : (a : α) → β a → Option (γ a)} {k : α} :
     (m.filterMap f).getKey? k =
     (m.getKey? k).pfilter (fun x h' =>
       (f x (m.get x (mem_of_getKey?_eq_some h'))).isSome) :=
-  m.inductionOn fun _ => Std.DHashMap.getKey?_filterMap
+  m.inductionOn fun _ => DHashMap.getKey?_filterMap
 
 @[simp]
 theorem getKey_filterMap
     {f : (a : α) → β a → Option (γ a)} {k : α} {h'} :
     (m.filterMap f).getKey k h' = m.getKey k (mem_of_mem_filterMap h') :=
-  m.inductionOn (fun _ _ => Std.DHashMap.getKey_filterMap) h'
+  m.inductionOn (fun _ _ => DHashMap.getKey_filterMap) h'
 
 theorem getKey!_filterMap [LawfulBEq α] [Inhabited α]
     {f : (a : α) → β a → Option (γ a)} {k : α} :
     (m.filterMap f).getKey! k =
     ((m.getKey? k).pfilter (fun x h' =>
       (f x (m.get x (mem_of_getKey?_eq_some h'))).isSome)).get! :=
-  m.inductionOn fun _ => Std.DHashMap.getKey!_filterMap
+  m.inductionOn fun _ => DHashMap.getKey!_filterMap
 
 theorem getKeyD_filterMap [LawfulBEq α]
     {f : (a : α) → β a → Option (γ a)} {k fallback : α} :
     (m.filterMap f).getKeyD k fallback =
     ((m.getKey? k).pfilter (fun x h' =>
       (f x (m.get x (mem_of_getKey?_eq_some h'))).isSome)).getD fallback :=
-  m.inductionOn fun _ => Std.DHashMap.getKeyD_filterMap
+  m.inductionOn fun _ => DHashMap.getKeyD_filterMap
 
 namespace Const
 
-variable {β : Type v} {γ : Type w} {m : DHashMap α (fun _ => β)}
+variable {β : Type v} {γ : Type w} {m : ExtDHashMap α (fun _ => β)}
 
 theorem filterMap_eq_empty_iff {f : α → β → Option γ} :
     m.filterMap f = ∅ ↔ ∀ k h, f (m.getKey k h) (get m k h) = none :=
-  isEmpty_iff.symm.trans <| m.inductionOn fun _ => Std.DHashMap.Const.isEmpty_filterMap_iff
+  isEmpty_iff.symm.trans <| m.inductionOn fun _ => DHashMap.Const.isEmpty_filterMap_iff
 
 theorem mem_filterMap
     {f : α → β → Option γ} {k : α} :
     k ∈ m.filterMap f ↔ ∃ h, (f (m.getKey k h) (Const.get m k h)).isSome :=
-  m.inductionOn fun _ => Std.DHashMap.Const.mem_filterMap
+  m.inductionOn fun _ => DHashMap.Const.mem_filterMap
 
 theorem size_filterMap_eq_size_iff
     {f : α → β → Option γ} :
     (m.filterMap f).size = m.size ↔ ∀ k h, (f (m.getKey k h) (Const.get m k h)).isSome :=
-  m.inductionOn fun _ => Std.DHashMap.Const.size_filterMap_eq_size_iff
+  m.inductionOn fun _ => DHashMap.Const.size_filterMap_eq_size_iff
 
 theorem get?_filterMap
     {f : α → β → Option γ} {k : α} :
     Const.get? (m.filterMap f) k = (Const.get? m k).pbind (fun x h' =>
       f (m.getKey k (mem_iff_isSome_get?.mpr (Option.isSome_of_eq_some h'))) x) :=
-  m.inductionOn fun _ => Std.DHashMap.Const.get?_filterMap
+  m.inductionOn fun _ => DHashMap.Const.get?_filterMap
 
 theorem get?_filterMap_of_getKey?_eq_some
     {f : α → β → Option γ} {k k' : α} (h : m.getKey? k = some k') :
     Const.get? (m.filterMap f) k = (Const.get? m k).bind (f k') :=
-  m.inductionOn (fun _ h => Std.DHashMap.Const.get?_filterMap_of_getKey?_eq_some h) h
+  m.inductionOn (fun _ h => DHashMap.Const.get?_filterMap_of_getKey?_eq_some h) h
 
 theorem isSome_apply_of_mem_filterMap
     {f : α → β → Option γ} {k : α} :
     ∀ (h : k ∈ m.filterMap f),
       (f (m.getKey k (mem_of_mem_filterMap h))
         (Const.get m k (mem_of_mem_filterMap h))).isSome :=
-  m.inductionOn fun _ => Std.DHashMap.Const.isSome_apply_of_mem_filterMap
+  m.inductionOn fun _ => DHashMap.Const.isSome_apply_of_mem_filterMap
 
 @[simp]
 theorem get_filterMap
@@ -2918,52 +2918,52 @@ theorem get_filterMap
       (f (m.getKey k (mem_of_mem_filterMap h))
         (Const.get m k (mem_of_mem_filterMap h))).get
           (isSome_apply_of_mem_filterMap h) :=
-  m.inductionOn (fun _ _ => Std.DHashMap.Const.get_filterMap) h
+  m.inductionOn (fun _ _ => DHashMap.Const.get_filterMap) h
 
 theorem get!_filterMap [Inhabited γ]
     {f : α → β → Option γ} {k : α} :
     Const.get! (m.filterMap f) k =
       ((Const.get? m k).pbind (fun x h' =>
         f (m.getKey k (mem_iff_isSome_get?.mpr (Option.isSome_of_eq_some h'))) x)).get! :=
-  m.inductionOn fun _ => Std.DHashMap.Const.get!_filterMap
+  m.inductionOn fun _ => DHashMap.Const.get!_filterMap
 
 theorem get!_filterMap_of_getKey?_eq_some [Inhabited γ]
     {f : α → β → Option γ} {k k' : α} (h : m.getKey? k = some k') :
     Const.get! (m.filterMap f) k = ((Const.get? m k).bind (f k')).get! :=
-  m.inductionOn (fun _ h => Std.DHashMap.Const.get!_filterMap_of_getKey?_eq_some h) h
+  m.inductionOn (fun _ h => DHashMap.Const.get!_filterMap_of_getKey?_eq_some h) h
 
 theorem getD_filterMap
     {f : α → β → Option γ} {k : α} {fallback : γ} :
     Const.getD (m.filterMap f) k fallback =
       ((Const.get? m k).pbind (fun x h' =>
       f (m.getKey k (mem_iff_isSome_get?.mpr (Option.isSome_of_eq_some h'))) x)).getD fallback :=
-  m.inductionOn fun _ => Std.DHashMap.Const.getD_filterMap
+  m.inductionOn fun _ => DHashMap.Const.getD_filterMap
 
 theorem getD_filterMap_of_getKey?_eq_some
     {f : α → β → Option γ} {k k' : α} {fallback : γ} (h : m.getKey? k = some k') :
     Const.getD (m.filterMap f) k fallback = ((Const.get? m k).bind (f k')).getD fallback :=
-  m.inductionOn (fun _ h => Std.DHashMap.Const.getD_filterMap_of_getKey?_eq_some h) h
+  m.inductionOn (fun _ h => DHashMap.Const.getD_filterMap_of_getKey?_eq_some h) h
 
 theorem getKey?_filterMap
     {f : α → β → Option γ} {k : α} :
     (m.filterMap f).getKey? k =
     (m.getKey? k).pfilter (fun x h' =>
       (f x (Const.get m x (mem_of_getKey?_eq_some h'))).isSome) :=
-  m.inductionOn fun _ => Std.DHashMap.Const.getKey?_filterMap
+  m.inductionOn fun _ => DHashMap.Const.getKey?_filterMap
 
 theorem getKey!_filterMap [Inhabited α]
     {f : α → β → Option γ} {k : α} :
     (m.filterMap f).getKey! k =
     ((m.getKey? k).pfilter (fun x h' =>
       (f x (Const.get m x (mem_of_getKey?_eq_some h'))).isSome)).get! :=
-  m.inductionOn fun _ => Std.DHashMap.Const.getKey!_filterMap
+  m.inductionOn fun _ => DHashMap.Const.getKey!_filterMap
 
 theorem getKeyD_filterMap
     {f : α → β → Option γ} {k fallback : α} :
     (m.filterMap f).getKeyD k fallback =
     ((m.getKey? k).pfilter (fun x h' =>
       (f x (Const.get m x (mem_of_getKey?_eq_some h'))).isSome)).getD fallback :=
-  m.inductionOn fun _ => Std.DHashMap.Const.getKeyD_filterMap
+  m.inductionOn fun _ => DHashMap.Const.getKeyD_filterMap
 
 end Const
 
@@ -2973,215 +2973,215 @@ section filter
 
 theorem filterMap_eq_filter {f : (a : α) → β a → Bool} :
     m.filterMap (fun k => Option.guard (fun v => f k v)) = m.filter f :=
-  m.inductionOn fun _ => Quotient.sound Std.DHashMap.filterMap_equiv_filter
+  m.inductionOn fun _ => Quotient.sound DHashMap.filterMap_equiv_filter
 
 @[simp]
 theorem filter_eq_empty_iff [LawfulBEq α]
     {f : (a : α) → β a → Bool} :
     m.filter f = ∅ ↔ ∀ k h, f k (m.get k h) = false :=
-  isEmpty_iff.symm.trans <| m.inductionOn fun _ => Std.DHashMap.isEmpty_filter_iff
+  isEmpty_iff.symm.trans <| m.inductionOn fun _ => DHashMap.isEmpty_filter_iff
 
 theorem filter_key_eq_empty_iff {f : α → Bool} :
     m.filter (fun a _ => f a) = ∅ ↔ ∀ k h, f (m.getKey k h) = false :=
-  isEmpty_iff.symm.trans <| m.inductionOn fun _ => Std.DHashMap.isEmpty_filter_key_iff
+  isEmpty_iff.symm.trans <| m.inductionOn fun _ => DHashMap.isEmpty_filter_key_iff
 
 theorem contains_filter [LawfulBEq α] {f : (a : α) → β a → Bool} {k : α} :
     (m.filter f).contains k = (m.get? k).any (f k) :=
-  m.inductionOn fun _ => Std.DHashMap.contains_filter
+  m.inductionOn fun _ => DHashMap.contains_filter
 
 theorem mem_filter [LawfulBEq α] {f : (a : α) → β a → Bool} {k : α} :
     k ∈ m.filter f ↔ ∃ h, f k (m.get k h) :=
-  m.inductionOn fun _ => Std.DHashMap.mem_filter
+  m.inductionOn fun _ => DHashMap.mem_filter
 
 theorem mem_filter_key {f : α → Bool} {k : α} :
     k ∈ m.filter (fun a _ => f a) ↔ ∃ h, f (m.getKey k h) :=
-  m.inductionOn fun _ => Std.DHashMap.mem_filter_key
+  m.inductionOn fun _ => DHashMap.mem_filter_key
 
 theorem contains_of_contains_filter {f : (a : α) → β a → Bool} {k : α} :
     (m.filter f).contains k = true → m.contains k = true :=
-  m.inductionOn fun _ => Std.DHashMap.contains_of_contains_filter
+  m.inductionOn fun _ => DHashMap.contains_of_contains_filter
 
 theorem mem_of_mem_filter {f : (a : α) → β a → Bool} {k : α} :
     k ∈ (m.filter f) → k ∈ m :=
-  m.inductionOn fun _ => Std.DHashMap.mem_of_mem_filter
+  m.inductionOn fun _ => DHashMap.mem_of_mem_filter
 
 theorem size_filter_le_size {f : (a : α) → β a → Bool} :
     (m.filter f).size ≤ m.size :=
-  m.inductionOn fun _ => Std.DHashMap.size_filter_le_size
+  m.inductionOn fun _ => DHashMap.size_filter_le_size
 
 theorem size_filter_eq_size_iff [LawfulBEq α] {f : (a : α) → β a → Bool} :
     (m.filter f).size = m.size ↔ ∀ k h, f k (m.get k h) :=
-  m.inductionOn fun _ => Std.DHashMap.size_filter_eq_size_iff
+  m.inductionOn fun _ => DHashMap.size_filter_eq_size_iff
 
 theorem filter_eq_self_iff [LawfulBEq α] {f : (a : α) → β a → Bool} :
     m.filter f = m ↔ ∀ k h, f k (m.get k h) :=
-  m.inductionOn fun _ => Iff.trans ⟨Quotient.exact, Quotient.sound⟩ Std.DHashMap.filter_equiv_self_iff
+  m.inductionOn fun _ => Iff.trans ⟨Quotient.exact, Quotient.sound⟩ DHashMap.filter_equiv_self_iff
 
 theorem filter_key_equiv_self_iff {f : (a : α) → Bool} :
     m.filter (fun k _ => f k) = m ↔ ∀ k h, f (m.getKey k h) :=
-  m.inductionOn fun _ => Iff.trans ⟨Quotient.exact, Quotient.sound⟩ Std.DHashMap.filter_key_equiv_self_iff
+  m.inductionOn fun _ => Iff.trans ⟨Quotient.exact, Quotient.sound⟩ DHashMap.filter_key_equiv_self_iff
 
 theorem size_filter_key_eq_size_iff {f : α → Bool} :
     (m.filter fun k _ => f k).size = m.size ↔ ∀ k h, f (m.getKey k h) :=
-  m.inductionOn fun _ => Std.DHashMap.size_filter_key_eq_size_iff
+  m.inductionOn fun _ => DHashMap.size_filter_key_eq_size_iff
 
 @[simp]
 theorem get?_filter [LawfulBEq α]
     {f : (a : α) → β a → Bool} {k : α} :
     (m.filter f).get? k = (m.get? k).filter (f k) :=
-  m.inductionOn fun _ => Std.DHashMap.get?_filter
+  m.inductionOn fun _ => DHashMap.get?_filter
 
 @[simp]
 theorem get_filter [LawfulBEq α]
     {f : (a : α) → β a → Bool} {k : α} {h'} :
     (m.filter f).get k h' = m.get k (mem_of_mem_filter h') :=
-  m.inductionOn (fun _ _ => Std.DHashMap.get_filter) h'
+  m.inductionOn (fun _ _ => DHashMap.get_filter) h'
 
 theorem get!_filter [LawfulBEq α]
     {f : (a : α) → β a → Bool} {k : α} [Inhabited (β k)] :
     (m.filter f).get! k = ((m.get? k).filter (f k)).get! :=
-  m.inductionOn fun _ => Std.DHashMap.get!_filter
+  m.inductionOn fun _ => DHashMap.get!_filter
 
 theorem getD_filter [LawfulBEq α]
     {f : (a : α) → β a → Bool} {k : α} {fallback : β k} :
     (m.filter f).getD k fallback = ((m.get? k).filter (f k)).getD fallback :=
-  m.inductionOn fun _ => Std.DHashMap.getD_filter
+  m.inductionOn fun _ => DHashMap.getD_filter
 
 theorem getKey?_filter [LawfulBEq α]
     {f : (a : α) → β a → Bool} {k : α} :
     (m.filter f).getKey? k =
     (m.getKey? k).pfilter (fun x h' =>
       f x (m.get x (mem_of_getKey?_eq_some h'))) :=
-  m.inductionOn fun _ => Std.DHashMap.getKey?_filter
+  m.inductionOn fun _ => DHashMap.getKey?_filter
 
 theorem getKey?_filter_key
     {f : α → Bool} {k : α} :
     (m.filter fun k _ => f k).getKey? k = (m.getKey? k).filter f :=
-  m.inductionOn fun _ => Std.DHashMap.getKey?_filter_key
+  m.inductionOn fun _ => DHashMap.getKey?_filter_key
 
 @[simp]
 theorem getKey_filter
     {f : (a : α) → β a → Bool} {k : α} {h'} :
     (m.filter f).getKey k h' = m.getKey k (mem_of_mem_filter h') :=
-  m.inductionOn (fun _ _ => Std.DHashMap.getKey_filter) h'
+  m.inductionOn (fun _ _ => DHashMap.getKey_filter) h'
 
 theorem getKey!_filter [LawfulBEq α] [Inhabited α]
     {f : (a : α) → β a → Bool} {k : α} :
     (m.filter f).getKey! k =
     ((m.getKey? k).pfilter (fun x h' =>
       f x (m.get x (mem_of_getKey?_eq_some h')))).get! :=
-  m.inductionOn fun _ => Std.DHashMap.getKey!_filter
+  m.inductionOn fun _ => DHashMap.getKey!_filter
 
 theorem getKey!_filter_key [Inhabited α]
     {f : α → Bool} {k : α} :
     (m.filter fun k _ => f k).getKey! k = ((m.getKey? k).filter f).get! :=
-  m.inductionOn fun _ => Std.DHashMap.getKey!_filter_key
+  m.inductionOn fun _ => DHashMap.getKey!_filter_key
 
 theorem getKeyD_filter [LawfulBEq α]
     {f : (a : α) → β a → Bool} {k fallback : α} :
     (m.filter f).getKeyD k fallback =
     ((m.getKey? k).pfilter (fun x h' =>
       f x (m.get x (mem_of_getKey?_eq_some h')))).getD fallback :=
-  m.inductionOn fun _ => Std.DHashMap.getKeyD_filter
+  m.inductionOn fun _ => DHashMap.getKeyD_filter
 
 theorem getKeyD_filter_key
     {f : α → Bool} {k fallback : α} :
     (m.filter fun k _ => f k).getKeyD k fallback = ((m.getKey? k).filter f).getD fallback :=
-  m.inductionOn fun _ => Std.DHashMap.getKeyD_filter_key
+  m.inductionOn fun _ => DHashMap.getKeyD_filter_key
 
 namespace Const
 
-variable {β : Type v} {γ : Type w} {m : DHashMap α (fun _ => β)}
+variable {β : Type v} {γ : Type w} {m : ExtDHashMap α (fun _ => β)}
 
 theorem filter_eq_empty_iff {f : α → β → Bool} :
     m.filter f = ∅ ↔ ∀ k h, f (m.getKey k h) (Const.get m k h) = false :=
-  isEmpty_iff.symm.trans <| m.inductionOn fun _ => Std.DHashMap.Const.isEmpty_filter_iff
+  isEmpty_iff.symm.trans <| m.inductionOn fun _ => DHashMap.Const.isEmpty_filter_iff
 
 theorem mem_filter
     {f : α → β → Bool} {k : α} :
     k ∈ m.filter f ↔ ∃ (h' : k ∈ m),
       f (m.getKey k h') (Const.get m k h') :=
-  m.inductionOn fun _ => Std.DHashMap.Const.mem_filter
+  m.inductionOn fun _ => DHashMap.Const.mem_filter
 
 theorem size_filter_le_size
     {f : α → β → Bool} :
     (m.filter f).size ≤ m.size :=
-  m.inductionOn fun _ => Std.DHashMap.Const.size_filter_le_size
+  m.inductionOn fun _ => DHashMap.Const.size_filter_le_size
 
 theorem size_filter_eq_size_iff
     {f : α → β → Bool} :
     (m.filter f).size = m.size ↔ ∀ (a : α) (h : a ∈ m),
       f (m.getKey a h) (Const.get m a h) :=
-  m.inductionOn fun _ => Std.DHashMap.Const.size_filter_eq_size_iff
+  m.inductionOn fun _ => DHashMap.Const.size_filter_eq_size_iff
 
 theorem filter_eq_self_iff {f : α → β → Bool} :
     m.filter f = m ↔ ∀ k h, f (m.getKey k h) (Const.get m k h) :=
-  m.inductionOn fun _ => Iff.trans ⟨Quotient.exact, Quotient.sound⟩ Std.DHashMap.Const.filter_equiv_self_iff
+  m.inductionOn fun _ => Iff.trans ⟨Quotient.exact, Quotient.sound⟩ DHashMap.Const.filter_equiv_self_iff
 
 theorem get?_filter
     {f : α → β → Bool} {k : α} :
     Const.get? (m.filter f) k = (Const.get? m k).pfilter (fun x h' =>
       f (m.getKey k (mem_iff_isSome_get?.mpr (Option.isSome_of_eq_some h'))) x) :=
-  m.inductionOn fun _ => Std.DHashMap.Const.get?_filter
+  m.inductionOn fun _ => DHashMap.Const.get?_filter
 
 theorem get?_filter_of_getKey?_eq_some
     {f : α → β → Bool} {k k' : α} :
     m.getKey? k = some k' →
       Const.get? (m.filter f) k = (Const.get? m k).filter (fun x => f k' x) :=
-  m.inductionOn fun _ => Std.DHashMap.Const.get?_filter_of_getKey?_eq_some
+  m.inductionOn fun _ => DHashMap.Const.get?_filter_of_getKey?_eq_some
 
 @[simp]
 theorem get_filter
     {f : α → β → Bool} {k : α} {h'} :
     Const.get (m.filter f) k h' = Const.get m k (mem_of_mem_filter h') :=
-  m.inductionOn (fun _ _ => Std.DHashMap.Const.get_filter) h'
+  m.inductionOn (fun _ _ => DHashMap.Const.get_filter) h'
 
 theorem get!_filter [Inhabited β]
     {f : α → β → Bool} {k : α} :
     Const.get! (m.filter f) k =
       ((Const.get? m k).pfilter (fun x h' =>
       f (m.getKey k (mem_iff_isSome_get?.mpr (Option.isSome_of_eq_some h'))) x)).get! :=
-  m.inductionOn fun _ => Std.DHashMap.Const.get!_filter
+  m.inductionOn fun _ => DHashMap.Const.get!_filter
 
 theorem get!_filter_of_getKey?_eq_some [Inhabited β]
     {f : α → β → Bool} {k k' : α} :
     m.getKey? k = some k' →
       Const.get! (m.filter f) k = ((Const.get? m k).filter (fun x => f k' x)).get! :=
-  m.inductionOn fun _ => Std.DHashMap.Const.get!_filter_of_getKey?_eq_some
+  m.inductionOn fun _ => DHashMap.Const.get!_filter_of_getKey?_eq_some
 
 theorem getD_filter
     {f : α → β → Bool} {k : α} {fallback : β} :
     Const.getD (m.filter f) k fallback = ((Const.get? m k).pfilter (fun x h' =>
       f (m.getKey k (mem_iff_isSome_get?.mpr (Option.isSome_of_eq_some h'))) x)).getD fallback :=
-  m.inductionOn fun _ => Std.DHashMap.Const.getD_filter
+  m.inductionOn fun _ => DHashMap.Const.getD_filter
 
 theorem getD_filter_of_getKey?_eq_some
     {f : α → β → Bool} {k k' : α} {fallback : β} :
     m.getKey? k = some k' →
       Const.getD (m.filter f) k fallback =
         ((Const.get? m k).filter (fun x => f k' x)).getD fallback :=
-  m.inductionOn fun _ => Std.DHashMap.Const.getD_filter_of_getKey?_eq_some
+  m.inductionOn fun _ => DHashMap.Const.getD_filter_of_getKey?_eq_some
 
 theorem getKey?_filter
     {f : α → β → Bool} {k : α} :
     (m.filter f).getKey? k =
     (m.getKey? k).pfilter (fun x h' =>
       (f x (Const.get m x (mem_of_getKey?_eq_some h')))) :=
-  m.inductionOn fun _ => Std.DHashMap.Const.getKey?_filter
+  m.inductionOn fun _ => DHashMap.Const.getKey?_filter
 
 theorem getKey!_filter [Inhabited α]
     {f : α → β → Bool} {k : α} :
     (m.filter f).getKey! k =
     ((m.getKey? k).pfilter (fun x h' =>
       (f x (Const.get m x (mem_of_getKey?_eq_some h'))))).get! :=
-  m.inductionOn fun _ => Std.DHashMap.Const.getKey!_filter
+  m.inductionOn fun _ => DHashMap.Const.getKey!_filter
 
 theorem getKeyD_filter
     {f : α → β → Bool} {k fallback : α} :
     (m.filter f).getKeyD k fallback =
     ((m.getKey? k).pfilter (fun x h' =>
       (f x (Const.get m x (mem_of_getKey?_eq_some h'))))).getD fallback :=
-  m.inductionOn fun _ => Std.DHashMap.Const.getKeyD_filter
+  m.inductionOn fun _ => DHashMap.Const.getKeyD_filter
 
 end Const
 
@@ -3193,144 +3193,144 @@ variable {γ : α → Type w} {δ : α → Type w'}
 
 @[simp]
 theorem map_id_fun : m.map (fun _ v => v) = m :=
-  m.inductionOn fun _ => Quotient.sound Std.DHashMap.map_id_equiv
+  m.inductionOn fun _ => Quotient.sound DHashMap.map_id_equiv
 
 @[simp]
 theorem map_map {f : (a : α) → β a → γ a} {g : (a : α) → γ a → δ a} :
     (m.map f).map g = m.map fun k v => g k (f k v) :=
-  m.inductionOn fun _ => Quotient.sound Std.DHashMap.map_map_equiv
+  m.inductionOn fun _ => Quotient.sound DHashMap.map_map_equiv
 
 theorem filterMap_eq_map {f : (a : α) → β a → γ a} :
     (m.filterMap (fun k v => some (f k v))) = m.map f :=
-  m.inductionOn fun _ => Quotient.sound Std.DHashMap.filterMap_equiv_map
+  m.inductionOn fun _ => Quotient.sound DHashMap.filterMap_equiv_map
 
 @[simp]
 theorem map_eq_empty_iff {f : (a : α) → β a → γ a} :
     m.map f = ∅ ↔ m = ∅ := by
   simp only [← isEmpty_iff, Bool.coe_iff_coe]
-  exact m.inductionOn fun _ => Std.DHashMap.isEmpty_map
+  exact m.inductionOn fun _ => DHashMap.isEmpty_map
 
 theorem contains_map
     {f : (a : α) → β a → γ a} {k : α} :
     (m.map f).contains k = m.contains k :=
-  m.inductionOn fun _ => Std.DHashMap.contains_map
+  m.inductionOn fun _ => DHashMap.contains_map
 
 theorem contains_of_contains_map
     {f : (a : α) → β a → γ a} {k : α} :
     (m.map f).contains k = true → m.contains k = true :=
-  m.inductionOn fun _ => Std.DHashMap.contains_of_contains_map
+  m.inductionOn fun _ => DHashMap.contains_of_contains_map
 
 @[simp]
 theorem mem_map
     {f : (a : α) → β a → γ a} {k : α} :
     k ∈ m.map f ↔ k ∈ m :=
-  m.inductionOn fun _ => Std.DHashMap.mem_map
+  m.inductionOn fun _ => DHashMap.mem_map
 
 theorem mem_of_mem_map
     {f : (a : α) → β a → γ a} {k : α} :
     k ∈ m.map f → k ∈ m :=
-  m.inductionOn fun _ => Std.DHashMap.mem_of_mem_map
+  m.inductionOn fun _ => DHashMap.mem_of_mem_map
 
 @[simp]
 theorem size_map
     {f : (a : α) → β a → γ a} :
     (m.map f).size = m.size :=
-  m.inductionOn fun _ => Std.DHashMap.size_map
+  m.inductionOn fun _ => DHashMap.size_map
 
 @[simp]
 theorem get?_map [LawfulBEq α]
     {f : (a : α) → β a → γ a} {k : α} :
     (m.map f).get? k = (m.get? k).map (f k) :=
-  m.inductionOn fun _ => Std.DHashMap.get?_map
+  m.inductionOn fun _ => DHashMap.get?_map
 
 @[simp]
 theorem get_map [LawfulBEq α]
     {f : (a : α) → β a → γ a} {k : α} {h'} :
     (m.map f).get k h' = f k (m.get k (mem_of_mem_map h')) :=
-  m.inductionOn (fun _ _ => Std.DHashMap.get_map) h'
+  m.inductionOn (fun _ _ => DHashMap.get_map) h'
 
 theorem get!_map [LawfulBEq α]
     {f : (a : α) → β a → γ a} {k : α} [Inhabited (γ k)] :
     (m.map f).get! k = ((m.get? k).map (f k)).get! :=
-  m.inductionOn fun _ => Std.DHashMap.get!_map
+  m.inductionOn fun _ => DHashMap.get!_map
 
 theorem getD_map [LawfulBEq α]
     {f : (a : α) → β a → γ a} {k : α} {fallback : γ k} :
     (m.map f).getD k fallback = ((m.get? k).map (f k)).getD fallback :=
-  m.inductionOn fun _ => Std.DHashMap.getD_map
+  m.inductionOn fun _ => DHashMap.getD_map
 
 @[simp]
 theorem getKey?_map
     {f : (a : α) → β a → γ a} {k : α} :
     (m.map f).getKey? k = m.getKey? k :=
-  m.inductionOn fun _ => Std.DHashMap.getKey?_map
+  m.inductionOn fun _ => DHashMap.getKey?_map
 
 @[simp]
 theorem getKey_map
     {f : (a : α) → β a → γ a} {k : α} {h'} :
     (m.map f).getKey k h' = m.getKey k (mem_of_mem_map h') :=
-  m.inductionOn (fun _ _ => Std.DHashMap.getKey_map) h'
+  m.inductionOn (fun _ _ => DHashMap.getKey_map) h'
 
 @[simp]
 theorem getKey!_map [Inhabited α]
     {f : (a : α) → β a → γ a} {k : α} :
     (m.map f).getKey! k = m.getKey! k :=
-  m.inductionOn fun _ => Std.DHashMap.getKey!_map
+  m.inductionOn fun _ => DHashMap.getKey!_map
 
 @[simp]
 theorem getKeyD_map
     {f : (a : α) → β a → γ a} {k fallback : α} :
     (m.map f).getKeyD k fallback = m.getKeyD k fallback :=
-  m.inductionOn fun _ => Std.DHashMap.getKeyD_map
+  m.inductionOn fun _ => DHashMap.getKeyD_map
 
 namespace Const
 
-variable {β : Type v} {γ : Type w} {m : DHashMap α fun _ => β}
+variable {β : Type v} {γ : Type w} {m : ExtDHashMap α fun _ => β}
 
 theorem get?_map
     {f : α → β → γ} {k : α} :
     Const.get? (m.map f) k = (Const.get? m k).pmap (fun v h' => f (m.getKey k h') v)
       (fun _ h' => mem_iff_isSome_get?.mpr (Option.isSome_of_eq_some h')) :=
-  m.inductionOn fun _ => Std.DHashMap.Const.get?_map
+  m.inductionOn fun _ => DHashMap.Const.get?_map
 
 theorem get?_map_of_getKey?_eq_some
     {f : α → β → γ} {k k' : α} (h : m.getKey? k = some k') :
     Const.get? (m.map f) k = (Const.get? m k).map (f k') :=
-  m.inductionOn (fun _ h => Std.DHashMap.Const.get?_map_of_getKey?_eq_some h) h
+  m.inductionOn (fun _ h => DHashMap.Const.get?_map_of_getKey?_eq_some h) h
 
 @[simp]
 theorem get_map
     {f : α → β → γ} {k : α} {h'} :
     Const.get (m.map f) k h' =
       f (m.getKey k (mem_of_mem_map h')) (Const.get m k (mem_of_mem_map h')) :=
-  m.inductionOn (fun _ _ => Std.DHashMap.Const.get_map) h'
+  m.inductionOn (fun _ _ => DHashMap.Const.get_map) h'
 
 theorem get!_map [Inhabited γ]
     {f : α → β → γ} {k : α} :
     Const.get! (m.map f) k =
       ((get? m k).pmap (fun v h => f (m.getKey k h) v)
         (fun _ h' => mem_iff_isSome_get?.mpr (Option.isSome_of_mem h'))).get! :=
-  m.inductionOn fun _ => Std.DHashMap.Const.get!_map
+  m.inductionOn fun _ => DHashMap.Const.get!_map
 
 theorem get!_map_of_getKey?_eq_some [Inhabited γ]
     {f : α → β → γ} {k k' : α} (h : m.getKey? k = some k') :
     Const.get! (m.map f) k = ((Const.get? m k).map (f k')).get! :=
-  m.inductionOn (fun _ h => Std.DHashMap.Const.get!_map_of_getKey?_eq_some h) h
+  m.inductionOn (fun _ h => DHashMap.Const.get!_map_of_getKey?_eq_some h) h
 
 theorem getD_map
     {f : α → β → γ} {k : α} {fallback : γ} :
     Const.getD (m.map f) k fallback =
       ((get? m k).pmap (fun v h => f (m.getKey k h) v)
         (fun _ h' => mem_iff_isSome_get?.mpr (Option.isSome_of_eq_some h'))).getD fallback :=
-  m.inductionOn fun _ => Std.DHashMap.Const.getD_map
+  m.inductionOn fun _ => DHashMap.Const.getD_map
 
 theorem getD_map_of_getKey?_eq_some [Inhabited γ]
     {f : α → β → γ} {k k' : α} {fallback : γ} (h : m.getKey? k = some k') :
     Const.getD (m.map f) k fallback = ((Const.get? m k).map (f k')).getD fallback :=
-  m.inductionOn (fun _ h => Std.DHashMap.Const.getD_map_of_getKey?_eq_some h) h
+  m.inductionOn (fun _ h => DHashMap.Const.getD_map_of_getKey?_eq_some h) h
 
 end Const
 
 end map
 
-end Std.Extensional.DHashMap
+end Std.ExtDHashMap
